<http://datashapes.org/dash#GraphUpdate> <http://www.w3.org/2000/01/rdf-schema#comment> "A suggestion consisting of added and/or deleted triples, represented as rdf:Statements via dash:addedTriple and dash:deletedTriple." .
<http://datashapes.org/dash#fixed> <http://www.w3.org/2000/01/rdf-schema#comment> "Can be used to mark that certain validation results have already been fixed." .
<http://datashapes.org/dash#width> <http://www.w3.org/2000/01/rdf-schema#range> <http://www.w3.org/2001/XMLSchema#integer> .
_:B6df3b0d09d638883ddc7eaf55d1a9646 <http://www.w3.org/ns/shacl#name> "test graph" .
<http://datashapes.org/dash#TextAreaWithLangEditor> <http://www.w3.org/2000/01/rdf-schema#comment> "A multi-line text area to enter the value of a literal and a drop down to select a language." .
<http://datashapes.org/dash#JSTestCase> <http://www.w3.org/2000/01/rdf-schema#subClassOf> <http://datashapes.org/dash#TestCase> .
<http://datashapes.org/dash#addedTriple> <http://www.w3.org/1999/02/22-rdf-syntax-ns#type> <http://www.w3.org/1999/02/22-rdf-syntax-ns#Property> .
<http://datashapes.org/dash#shape> <http://www.w3.org/2000/01/rdf-schema#comment> "States that a subject resource has a given shape. This property can, for example, be used to capture results of SHACL validation on static data." .
<http://datashapes.org/dash#singleLine> <http://www.w3.org/2000/01/rdf-schema#range> <http://www.w3.org/2001/XMLSchema#boolean> .
_:B8791b3a24b8675de3fe6cea3980f416f <http://www.w3.org/ns/shacl#prefixes> <http://datashapes.org/dash> .
<http://datashapes.org/dash#TextFieldEditor> <http://www.w3.org/1999/02/22-rdf-syntax-ns#type> <http://datashapes.org/dash#Editor> .
<http://www.w3.org/ns/shacl#NodeKindConstraintComponent> <http://www.w3.org/ns/shacl#message> "Value does not have node kind {$nodeKind}" .
<http://datashapes.org/dash#isDeactivated> <http://www.w3.org/1999/02/22-rdf-syntax-ns#type> <http://www.w3.org/ns/shacl#SPARQLFunction> .
<http://www.w3.org/ns/shacl#QualifiedMinCountConstraintComponent> <http://www.w3.org/ns/shacl#message> "Fewer than {$qualifiedMinCount} values have shape {$qualifiedValueShape}" .
<http://datashapes.org/dash#StringOrLangString> <http://www.w3.org/1999/02/22-rdf-syntax-ns#type> <http://www.w3.org/1999/02/22-rdf-syntax-ns#List> .
<http://datashapes.org/dash#SPARQLUpdateSuggestionGenerator> <http://www.w3.org/2000/01/rdf-schema#comment> "A SuggestionGenerator based on a SPARQL UPDATE query (sh:update), producing an instance of dash:GraphUpdate. The INSERTs become dash:addedTriple and the DELETEs become dash:deletedTriple. The WHERE clause operates on the data graph with the pre-bound variables $subject, $predicate and $object, as well as the other pre-bound variables for the parameters of the constraint.\n\nIn many cases, there may be multiple possible suggestions to fix a problem. For example, with sh:maxLength there are many ways to slice a string. In those cases, the system will first iterate through the result variables from a SELECT query (sh:select) and apply these results as pre-bound variables into the UPDATE query." .
<http://datashapes.org/dash#isNodeKindBlankNode> <http://www.w3.org/ns/shacl#ask> "ASK {\n\tFILTER ($nodeKind IN ( sh:BlankNode, sh:BlankNodeOrIRI, sh:BlankNodeOrLiteral ))\n}" .
_:Bcfe9344fc73c29171f67ab7f8d807e68 <http://www.w3.org/ns/shacl#oneOrMorePath> <http://www.w3.org/1999/02/22-rdf-syntax-ns#rest> .
<http://datashapes.org/dash#URIEditor> <http://www.w3.org/2000/01/rdf-schema#label> "URI editor" .
_:Bff9ecbe5a61b70becac46f6b4ddfdb03 <http://www.w3.org/ns/shacl#maxCount> "1"^^<http://www.w3.org/2001/XMLSchema#integer> .
<http://datashapes.org/dash#suggestion> <http://www.w3.org/2000/01/rdf-schema#range> <http://datashapes.org/dash#Suggestion> .
<http://datashapes.org/dash#suggestionConfidence> <http://www.w3.org/1999/02/22-rdf-syntax-ns#type> <http://www.w3.org/1999/02/22-rdf-syntax-ns#Property> .
<http://datashapes.org/dash#y> <http://www.w3.org/2000/01/rdf-schema#comment> "The y position." .
<http://datashapes.org/dash#isNodeKindIRI> <http://www.w3.org/2000/01/rdf-schema#label> "is NodeKind IRI" .
<http://datashapes.org/dash#Suggestion> <http://www.w3.org/1999/02/22-rdf-syntax-ns#type> <http://www.w3.org/2000/01/rdf-schema#Class> .
<http://datashapes.org/dash#SPARQLUpdateSuggestionGenerator> <http://www.w3.org/2000/01/rdf-schema#subClassOf> <http://www.w3.org/ns/shacl#SPARQLSelectExecutable> .
<http://datashapes.org/dash#FailureResult> <http://www.w3.org/2000/01/rdf-schema#label> "Failure result" .
_:B8911ff43e060d96ba77f70561fffd26e <http://www.w3.org/1999/02/22-rdf-syntax-ns#type> <http://www.w3.org/ns/shacl#JSValidator> .
<http://datashapes.org/dash#height> <http://www.w3.org/1999/02/22-rdf-syntax-ns#type> <http://www.w3.org/1999/02/22-rdf-syntax-ns#Property> .
_:Bf87fbb2c21e07adfb80e0445145d23a6 <http://www.w3.org/ns/shacl#jsFunctionName> "validateStem" .
_:B9e11ce9adf350d1895c6096c2ef7444d <http://www.w3.org/1999/02/22-rdf-syntax-ns#type> <http://www.w3.org/ns/shacl#JSValidator> .
<http://datashapes.org/dash#TestCase> <http://www.w3.org/2000/01/rdf-schema#label> "Test case" .
<http://datashapes.org/dash#FunctionTestCase> <http://www.w3.org/2000/01/rdf-schema#subClassOf> <http://datashapes.org/dash#TestCase> .
<http://datashapes.org/dash#AllObjectsTarget> <http://www.w3.org/2000/01/rdf-schema#label> "All objects target" .
<http://datashapes.org/dash#requiredExecutionPlatform> <http://www.w3.org/2000/01/rdf-schema#range> <http://datashapes.org/dash#ExecutionPlatform> .
_:Beb225391b5ff8fb10e272118f430ade4 <http://www.w3.org/1999/02/22-rdf-syntax-ns#type> <http://www.w3.org/ns/shacl#JSValidator> .
<http://datashapes.org/dash#ListShape> <http://www.w3.org/1999/02/22-rdf-syntax-ns#type> <http://www.w3.org/ns/shacl#NodeShape> .
<http://datashapes.org/dash#staticConstraint> <http://www.w3.org/1999/02/22-rdf-syntax-ns#type> <http://www.w3.org/1999/02/22-rdf-syntax-ns#Property> .
<http://datashapes.org/dash#BooleanSelectEditor> <http://www.w3.org/1999/02/22-rdf-syntax-ns#type> <http://datashapes.org/dash#Editor> .
<http://datashapes.org/dash#PrimaryKeyConstraintComponent> <http://www.w3.org/ns/shacl#propertyValidator> _:B517776987b29b83bb92acd7f611fa440 .
_:B9f5ec4ceX2D5991X2D4a1dX2Da81aX2D237da79bf345 <http://www.w3.org/1999/02/22-rdf-syntax-ns#rest> _:B817d3310X2D8c48X2D4ff6X2Da801X2D06febce45863 .
<http://datashapes.org/dash#coExistsWith> <http://www.w3.org/1999/02/22-rdf-syntax-ns#type> <http://www.w3.org/1999/02/22-rdf-syntax-ns#Property> .
<http://datashapes.org/dash#SPARQLUpdateSuggestionGenerator> <http://www.w3.org/2000/01/rdf-schema#label> "SPARQL UPDATE suggestion generator" .
_:B817d3310X2D8c48X2D4ff6X2Da801X2D06febce45863 <http://www.w3.org/1999/02/22-rdf-syntax-ns#rest> <http://www.w3.org/1999/02/22-rdf-syntax-ns#nil> .
<http://datashapes.org/dash#abstract> <http://www.w3.org/2000/01/rdf-schema#range> <http://www.w3.org/2001/XMLSchema#boolean> .
<http://datashapes.org/dash#NonRecursiveConstraintComponent> <http://www.w3.org/2000/01/rdf-schema#comment> "Used to state that a property or path must not point back to itself.\n\nFor example, \"a person cannot have itself as parent\" can be expressed by setting dash:nonRecursive=true for a given sh:path.\n\nTo express that a person cannot have itself among any of its (recursive) parents, use a sh:path with the + operator such as ex:parent+." .
<http://datashapes.org/dash#GraphStoreTestCase> <http://www.w3.org/2000/01/rdf-schema#subClassOf> <http://datashapes.org/dash#TestCase> .
_:Bd2820cd0X2D1befX2D4fb9X2D934fX2Dd31b1666ea53 <http://www.w3.org/1999/02/22-rdf-syntax-ns#rest> _:Ba2d95b06X2D9e54X2D48f4X2Db71bX2D49bde683055d .
_:B517776987b29b83bb92acd7f611fa440 <http://www.w3.org/1999/02/22-rdf-syntax-ns#type> <http://www.w3.org/ns/shacl#JSValidator> .
<http://www.w3.org/ns/shacl#InConstraintComponent> <http://www.w3.org/ns/shacl#validator> _:B3dc0d1acdae51f4d90e61301d771976f .
<http://datashapes.org/dash#CoExistsWithConstraintComponent> <http://datashapes.org/dash#localConstraint> "true"^^<http://www.w3.org/2001/XMLSchema#boolean> .
<http://datashapes.org/dash#hasNodeKind> <http://www.w3.org/2000/01/rdf-schema#comment> "Checks whether a given node (?value) has a given sh:NodeKind (?nodeKind). For example, sh:hasNodeKind(42, sh:Literal) = true." .
_:B23e1001b72de7da857c5cf60a846810f <http://www.w3.org/1999/02/22-rdf-syntax-ns#type> <http://www.w3.org/ns/shacl#JSValidator> .
<http://www.w3.org/ns/shacl#MaxCountConstraintComponent> <http://datashapes.org/dash#localConstraint> "true"^^<http://www.w3.org/2001/XMLSchema#boolean> .
<http://datashapes.org/dash#ListShape> <http://www.w3.org/2000/01/rdf-schema#comment> "Defines constraints on what it means for a node to be a well-formed RDF list.\n\nThe focus node must either be rdf:nil or not recursive. Furthermore, this shape uses dash:ListNodeShape as a \"helper\" to walk through all members of the whole list (including itself)." .
<http://datashapes.org/dash#QueryTestCase> <http://www.w3.org/2000/01/rdf-schema#label> "Query test case" .
<http://datashapes.org/dash#coExistsWith> <http://www.w3.org/2000/01/rdf-schema#range> <http://www.w3.org/1999/02/22-rdf-syntax-ns#Property> .
<http://datashapes.org/dash#URIEditor> <http://www.w3.org/2000/01/rdf-schema#comment> "An input field to enter the URI of a resource, e.g. rdfs:seeAlso links or images." .
<http://datashapes.org/dash#addedTriple> <http://www.w3.org/2000/01/rdf-schema#domain> <http://datashapes.org/dash#GraphUpdate> .
<http://datashapes.org/dash#SingleLineConstraintComponent> <http://www.w3.org/2000/01/rdf-schema#label> "Single line constraint component" .
<http://datashapes.org/dash#hidden> <http://www.w3.org/2000/01/rdf-schema#domain> <http://www.w3.org/ns/shacl#PropertyShape> .
<http://datashapes.org/dash#suggestionGroup> <http://www.w3.org/1999/02/22-rdf-syntax-ns#type> <http://www.w3.org/1999/02/22-rdf-syntax-ns#Property> .
<http://datashapes.org/dash#requiredExecutionPlatform> <http://www.w3.org/2000/01/rdf-schema#label> "required execution platform" .
<http://datashapes.org/dash#expectedResultIsTTL> <http://www.w3.org/2000/01/rdf-schema#range> <http://www.w3.org/2001/XMLSchema#boolean> .
<http://datashapes.org/dash#StemConstraintComponent> <http://www.w3.org/ns/shacl#message> "Value does not have stem {$stem}" .
<http://datashapes.org/dash> <http://www.w3.org/ns/shacl#declare> _:Bf0ecfeb376963097d84d425af13c3875 .
<http://datashapes.org/dash#HasValueWithClassConstraintComponent> <http://www.w3.org/2000/01/rdf-schema#label> "Has value with class constraint component" .
<http://datashapes.org/dash#DefaultValueTypeRule> <http://www.w3.org/2000/01/rdf-schema#comment> "\n\t\tA resource encapsulating a query that can be used to construct rdf:type triples for certain untyped nodes\n\t\tthat are an object in a triple where the predicate has a sh:defaultValueType.\n\t\tThis can be used as a pre-processor for shape graphs before they are validated.\n\t\t"^^<http://www.w3.org/1999/02/22-rdf-syntax-ns#HTML> .
_:B7463b1c77e1b791dc8f96918e9ed48ab <http://www.w3.org/ns/shacl#property> _:Bcb38cdae1cd4f5c0b1a9201bb0062cdf .
<http://datashapes.org/dash#isNodeKindBlankNode> <http://datashapes.org/dash#cachable> "true"^^<http://www.w3.org/2001/XMLSchema#boolean> .
<http://www.w3.org/ns/shacl#DatatypeConstraintComponent> <http://www.w3.org/ns/shacl#targetClass> <http://www.w3.org/ns/shacl#Shape> .
<http://datashapes.org/dash#ListNodeShape> <http://www.w3.org/2000/01/rdf-schema#label> "List node shape" .
<http://datashapes.org/dash#RDFQueryJSLibrary> <http://www.w3.org/2000/01/rdf-schema#label> "rdfQuery JavaScript Library" .
_:B7f1ad1df154d5b4790aefb896d1c9fb8 <http://www.w3.org/ns/shacl#datatype> <http://www.w3.org/2001/XMLSchema#boolean> .
_:B517776987b29b83bb92acd7f611fa440 <http://www.w3.org/ns/shacl#jsLibrary> <http://datashapes.org/dash#DASHJSLibrary> .
_:Bf0ecfeb376963097d84d425af13c3875 <http://www.w3.org/ns/shacl#prefix> "dcterms" .
<http://datashapes.org/dash#isIn> <http://www.w3.org/ns/shacl#ask> "\n\t\tASK {\n\t\t\tGRAPH $shapesGraph {\n\t\t\t\t$in (rdf:rest*)/rdf:first $value .\n\t\t\t}\n\t\t}\n\t\t" .
_:B23e1001b72de7da857c5cf60a846810f <http://www.w3.org/ns/shacl#jsLibrary> <http://datashapes.org/dash#DASHJSLibrary> .
<http://www.w3.org/ns/shacl#SPARQLExecutable> <http://datashapes.org/dash#abstract> "true"^^<http://www.w3.org/2001/XMLSchema#boolean> .
_:B64037a34fda104980e7dda281bd2bc45 <http://www.w3.org/ns/shacl#path> <http://datashapes.org/dash#expectedResult> .
<http://datashapes.org/dash#URIViewer> <http://www.w3.org/2000/01/rdf-schema#label> "URI Viewer" .
<http://www.w3.org/ns/shacl#ClosedConstraintComponent> <http://www.w3.org/ns/shacl#validator> _:Bed3045d9aeb8442f56a5b5a092925fd8 .
_:Beb225391b5ff8fb10e272118f430ade4 <http://www.w3.org/ns/shacl#jsLibrary> <http://datashapes.org/dash#DASHJSLibrary> .
<http://datashapes.org/dash#hasMinLength> <http://www.w3.org/1999/02/22-rdf-syntax-ns#type> <http://www.w3.org/ns/shacl#SPARQLAskValidator> .
_:B3b32abda9658f358f57cc4b5edac88b8 <http://www.w3.org/ns/shacl#path> <http://datashapes.org/dash#expectedResult> .
<http://datashapes.org/dash#AllObjectsTarget> <http://www.w3.org/2000/01/rdf-schema#comment> "A target containing all objects in the data graph as focus nodes." .
<http://www.w3.org/ns/shacl#ClassConstraintComponent> <http://www.w3.org/ns/shacl#labelTemplate> "Value needs to have class {$class}" .
<http://datashapes.org/dash#PrimaryKeyConstraintComponent-uriStart> <http://www.w3.org/ns/shacl#path> <http://datashapes.org/dash#uriStart> .
_:B9fe7602a489f48a08b22e99931d59d35 <http://www.w3.org/ns/shacl#name> "expected result" .
<http://datashapes.org/dash#AllSubjectsTarget> <http://www.w3.org/2000/01/rdf-schema#comment> "A target containing all subjects in the data graph as focus nodes." .
<http://datashapes.org/dash#suggestion> <http://www.w3.org/2000/01/rdf-schema#domain> <http://www.w3.org/ns/shacl#AbstractResult> .
<http://datashapes.org/dash#valueCount> <http://www.w3.org/ns/shacl#parameter> _:B5672337cd6b085d4efa2003d67fc0562 .
<http://datashapes.org/dash#TestCase> <http://www.w3.org/ns/shacl#property> _:Ba94bb54840f7b2f2def8b93e306cd9bf .
<http://datashapes.org/dash#QueryTestCase> <http://www.w3.org/1999/02/22-rdf-syntax-ns#type> <http://www.w3.org/2000/01/rdf-schema#Class> .
<http://datashapes.org/dash#CoExistsWithConstraintComponent-coExistsWith> <http://www.w3.org/1999/02/22-rdf-syntax-ns#type> <http://www.w3.org/ns/shacl#Parameter> .
<http://datashapes.org/dash#hasStem> <http://www.w3.org/ns/shacl#prefixes> <http://datashapes.org/dash> .
<http://www.w3.org/ns/shacl#AndConstraintComponent> <http://www.w3.org/ns/shacl#validator> _:B6bbc6c369a762614c55c30d7d8b0f737 .
<http://datashapes.org/dash#ReifiableByConstraintComponent> <http://www.w3.org/1999/02/22-rdf-syntax-ns#type> <http://www.w3.org/ns/shacl#ConstraintComponent> .
<http://www.w3.org/ns/shacl#MinCountConstraintComponent> <http://www.w3.org/ns/shacl#targetClass> <http://www.w3.org/ns/shacl#PropertyShape> .
<http://www.w3.org/ns/shacl#LessThanOrEqualsConstraintComponent> <http://www.w3.org/ns/shacl#propertyValidator> _:B83c9da54cec674e1fa200619bc30f9bb .
<http://datashapes.org/dash#DASHJSLibrary> <http://www.w3.org/ns/shacl#jsLibraryURL> "http://datashapes.org/js/dash.js"^^<http://www.w3.org/2001/XMLSchema#anyURI> .
<http://datashapes.org/dash#composite> <http://www.w3.org/2000/01/rdf-schema#range> <http://www.w3.org/2001/XMLSchema#boolean> .
<http://www.w3.org/ns/shacl#EqualsConstraintComponent> <http://www.w3.org/ns/shacl#propertyValidator> _:B555c69d616b27a2b4c8744e4327dadf9 .
<http://datashapes.org/dash#addedTriple> <http://www.w3.org/2000/01/rdf-schema#range> <http://www.w3.org/1999/02/22-rdf-syntax-ns#Statement> .
<http://www.w3.org/ns/shacl#HasValueConstraintComponent> <http://www.w3.org/ns/shacl#nodeValidator> _:B35bf980a43fa9fd53edf3a01919e908b .
<http://datashapes.org/dash#hasMaxInclusive> <http://www.w3.org/1999/02/22-rdf-syntax-ns#type> <http://www.w3.org/ns/shacl#SPARQLAskValidator> .
_:B140f0995d12aa7e2492672c94ebf1c8f <http://www.w3.org/ns/shacl#prefix> "rdf" .
_:B324a4eda45fae1908023e86a8b10dbdb <http://www.w3.org/ns/shacl#jsFunctionName> "validateClosedByTypesNode" .
_:Bf82714b519b59627a7719a96ae3deb05 <http://www.w3.org/ns/shacl#datatype> <http://www.w3.org/2001/XMLSchema#date> .
_:Ba2d95b06X2D9e54X2D48f4X2Db71bX2D49bde683055d <http://www.w3.org/1999/02/22-rdf-syntax-ns#rest> <http://www.w3.org/1999/02/22-rdf-syntax-ns#nil> .
_:B35bf980a43fa9fd53edf3a01919e908b <http://www.w3.org/1999/02/22-rdf-syntax-ns#type> <http://www.w3.org/ns/shacl#SPARQLAskValidator> .
<http://www.w3.org/ns/shacl#PatternConstraintComponent> <http://www.w3.org/ns/shacl#validator> <http://datashapes.org/dash#hasPattern> .
<http://datashapes.org/dash#isNodeKindLiteral> <http://www.w3.org/ns/shacl#returnType> <http://www.w3.org/2001/XMLSchema#boolean> .
<http://datashapes.org/dash#editor> <http://www.w3.org/2000/01/rdf-schema#label> "editor" .
_:Ba2d95b06X2D9e54X2D48f4X2Db71bX2D49bde683055d <http://www.w3.org/1999/02/22-rdf-syntax-ns#first> _:B978525ea2f32d0660c9ffc71e8b5d4cd .
_:B6bbc6c369a762614c55c30d7d8b0f737 <http://www.w3.org/ns/shacl#jsFunctionName> "validateAnd" .
<http://datashapes.org/dash#SPARQLUpdateSuggestionGenerator> <http://www.w3.org/2000/01/rdf-schema#subClassOf> <http://www.w3.org/ns/shacl#SPARQLUpdateExecutable> .
_:B517776987b29b83bb92acd7f611fa440 <http://www.w3.org/ns/shacl#jsFunctionName> "validatePrimaryKeyProperty" .
<http://datashapes.org/dash#TestCaseResult> <http://www.w3.org/2000/01/rdf-schema#label> "Test case result" .
<http://datashapes.org/dash#hasMaxExclusive> <http://www.w3.org/2000/01/rdf-schema#label> "has max exclusive" .
<http://datashapes.org/dash> <http://www.w3.org/1999/02/22-rdf-syntax-ns#type> <http://www.w3.org/2002/07/owl#Ontology> .
<http://datashapes.org/dash> <http://www.w3.org/2000/01/rdf-schema#comment> "DASH defines SPARQL-based validators for many SHACL Core constraint components. These are (among others) utilized by TopBraid and its API. Note that constraint components that require validation of nested shapes (such as sh:node) are not implementable without a function such as tosh:hasShape.\n\nDASH is also a SHACL library for frequently needed features and design patterns. All features in this library are 100% standards compliant and will work on any engine that fully supports SHACL." .
<http://datashapes.org/dash#expectedResultIsTTL> <http://www.w3.org/2000/01/rdf-schema#label> "expected result is Turtle" .
<http://datashapes.org/dash#CoExistsWithConstraintComponent-coExistsWith> <http://www.w3.org/ns/shacl#nodeKind> <http://www.w3.org/ns/shacl#IRI> .
<http://datashapes.org/dash#SymmetricConstraintComponent> <http://www.w3.org/2000/01/rdf-schema#label> "Symmetric constraint component" .
<http://datashapes.org/dash#suggestion> <http://www.w3.org/2000/01/rdf-schema#comment> "Can be used to link a result with one or more suggestions on how to address or improve the underlying issue." .
_:Bfe0a112f2951265152c632d9a5c70c7a <http://www.w3.org/ns/shacl#select> "\n\t\tSELECT DISTINCT $this ?value\n\t\tWHERE {\n\t\t\t$this $PATH ?value .\n\t\t\t$this $lessThanOrEquals ?otherValue .\n\t\t\tBIND (?value <= ?otherValue AS ?result) .\n\t\t\tFILTER (!bound(?result) || !(?result)) .\n\t\t}\n" .
<http://www.w3.org/ns/shacl#HasValueConstraintComponent> <http://www.w3.org/ns/shacl#nodeValidator> _:B77912faa4452655d39dee0cf876cb183 .
<http://datashapes.org/dash> <http://www.w3.org/ns/shacl#declare> _:Bf2df11d10c098c62248867b2af223317 .
<http://datashapes.org/dash#fixed> <http://www.w3.org/2000/01/rdf-schema#domain> <http://www.w3.org/ns/shacl#ValidationResult> .
<http://datashapes.org/dash#isIn> <http://www.w3.org/1999/02/22-rdf-syntax-ns#type> <http://www.w3.org/ns/shacl#SPARQLAskValidator> .
<http://datashapes.org/dash#FailureResult> <http://www.w3.org/2000/01/rdf-schema#subClassOf> <http://www.w3.org/ns/shacl#AbstractResult> .
_:B8911ff43e060d96ba77f70561fffd26e <http://www.w3.org/ns/shacl#jsLibrary> <http://datashapes.org/dash#DASHJSLibrary> .
<http://datashapes.org/dash#requiredExecutionPlatform> <http://www.w3.org/2000/01/rdf-schema#comment> "Links a SPARQL executable with the platforms that it can be executed on. This can be used by a SHACL implementation to determine whether a constraint validator or rule shall be ignored based on the current platform. For example, if a SPARQL query uses a function or magic property that is only available in TopBraid then a non-TopBraid platform can ignore the constraint (or simply always return no validation results). If this property has no value then the assumption is that the execution will succeed. As soon as one value exists, the assumption is that the engine supports at least one of the given platforms." .
<http://datashapes.org/dash#Widget> <http://www.w3.org/2000/01/rdf-schema#label> "Widget" .
_:B6d4cbc3d992ff864f2dac864d1480fb8 <http://www.w3.org/ns/shacl#path> <http://datashapes.org/dash#expectedResult> .
_:B9e11ce9adf350d1895c6096c2ef7444d <http://www.w3.org/ns/shacl#jsLibrary> <http://datashapes.org/dash#DASHJSLibrary> .
_:B0501804cef6c59c65c932d30353a449b <http://www.w3.org/ns/shacl#prefixes> <http://datashapes.org/dash> .
<http://datashapes.org/dash#stem> <http://www.w3.org/1999/02/22-rdf-syntax-ns#type> <http://www.w3.org/1999/02/22-rdf-syntax-ns#Property> .
<http://www.w3.org/ns/shacl#HasValueConstraintComponent> <http://datashapes.org/dash#localConstraint> "true"^^<http://www.w3.org/2001/XMLSchema#boolean> .
<http://datashapes.org/dash#HasValueWithClassConstraintComponent> <http://www.w3.org/ns/shacl#propertyValidator> _:Be4b7da0362b43f04fa717e3e11887a9e .
_:B646fdae9066263aad8548980a9a6346d <http://www.w3.org/ns/shacl#jsFunctionName> "validateRootClass" .
<http://datashapes.org/dash#LangStringViewer> <http://www.w3.org/2000/01/rdf-schema#label> "LangString Viewer" .
_:B2cb630d3ce6cc80fcb0af823135f42af <http://www.w3.org/ns/shacl#description> "A valid SPARQL expression calling the function to test." .
_:B474b201cX2D1114X2D493aX2Da90bX2D68fa0363bb24 <http://www.w3.org/1999/02/22-rdf-syntax-ns#rest> <http://www.w3.org/1999/02/22-rdf-syntax-ns#nil> .
<http://datashapes.org/dash#hasRootClass> <http://www.w3.org/2000/01/rdf-schema#label> "has root class" .
_:B40fc13c18bcea97b695cedc8f377811f <http://www.w3.org/ns/shacl#nodeKind> <http://www.w3.org/ns/shacl#IRI> .
_:B3dc0d1acdae51f4d90e61301d771976f <http://www.w3.org/ns/shacl#jsFunctionName> "validateIn" .
<http://datashapes.org/dash#hasMaxLength> <http://www.w3.org/2000/01/rdf-schema#label> "has max length" .
_:B8137cd87d692f6f1ad4d374873d42a49 <http://www.w3.org/ns/shacl#jsFunctionName> "validateEqualsNode" .
_:B555c69d616b27a2b4c8744e4327dadf9 <http://www.w3.org/ns/shacl#select> "\n\t\tSELECT DISTINCT $this ?value\n\t\tWHERE {\n\t\t\t{\n\t\t\t\t$this $PATH ?value .\n\t\t\t\tMINUS {\n\t\t\t\t\t$this $equals ?value .\n\t\t\t\t}\n\t\t\t}\n\t\t\tUNION\n\t\t\t{\n\t\t\t\t$this $equals ?value .\n\t\t\t\tMINUS {\n\t\t\t\t\t$this $PATH ?value .\n\t\t\t\t}\n\t\t\t}\n\t\t}\n\t\t" .
_:B0bddec390aebe99ada0a7924bd483b4f <http://www.w3.org/ns/shacl#jsFunctionName> "validateMaxLength" .
<http://datashapes.org/dash#SPARQLSelectTemplate> <http://www.w3.org/2000/01/rdf-schema#subClassOf> <http://www.w3.org/ns/shacl#Parameterizable> .
_:B6bbc6c369a762614c55c30d7d8b0f737 <http://www.w3.org/1999/02/22-rdf-syntax-ns#type> <http://www.w3.org/ns/shacl#JSValidator> .
<http://datashapes.org/dash#suggestionConfidence> <http://www.w3.org/2000/01/rdf-schema#domain> <http://datashapes.org/dash#Suggestion> .
<http://datashapes.org/dash#GraphValidationTestCase> <http://www.w3.org/2000/01/rdf-schema#label> "Graph validation test case" .
<http://datashapes.org/dash#editor> <http://www.w3.org/2000/01/rdf-schema#domain> <http://www.w3.org/ns/shacl#PropertyShape> .
<http://www.w3.org/ns/shacl#UniqueLangConstraintComponent> <http://www.w3.org/ns/shacl#targetClass> <http://www.w3.org/ns/shacl#PropertyShape> .
<http://datashapes.org/dash#SubSetOfConstraintComponent> <http://www.w3.org/ns/shacl#message> "Must be one of the values of {$subSetOf}" .
<http://datashapes.org/dash#Viewer> <http://www.w3.org/2000/01/rdf-schema#subClassOf> <http://datashapes.org/dash#Widget> .
<http://datashapes.org/dash#testEnvironment> <http://www.w3.org/1999/02/22-rdf-syntax-ns#type> <http://www.w3.org/1999/02/22-rdf-syntax-ns#Property> .
_:B8326699daa61eff99c25341497b7c80b <http://www.w3.org/1999/02/22-rdf-syntax-ns#type> <http://www.w3.org/ns/shacl#JSValidator> .
<http://datashapes.org/dash#DASHJSLibrary> <http://www.w3.org/1999/02/22-rdf-syntax-ns#type> <http://www.w3.org/ns/shacl#JSLibrary> .
_:B7f1ad1df154d5b4790aefb896d1c9fb8 <http://www.w3.org/ns/shacl#name> "cachable" .
<http://datashapes.org/dash#width> <http://www.w3.org/2000/01/rdf-schema#label> "width" .
_:Bc91acb30da815118fca913844f6cfa7b <http://www.w3.org/ns/shacl#jsLibrary> <http://datashapes.org/dash#DASHJSLibrary> .
<http://datashapes.org/dash#GraphUpdate> <http://www.w3.org/2000/01/rdf-schema#subClassOf> <http://datashapes.org/dash#Suggestion> .
<http://datashapes.org/dash#InstancesSelectEditor> <http://www.w3.org/2000/01/rdf-schema#comment> "A drop-down editor for all instances of the target class (based on sh:class of the property)." .
<http://datashapes.org/dash#SubSetOfConstraintComponent-subSetOf> <http://www.w3.org/ns/shacl#description> "A property (of the focus node) that must (at least) have all values from the set of value nodes." .
_:B8a6d95446c24ef2a1314f1cfdc6ea805 <http://www.w3.org/1999/02/22-rdf-syntax-ns#type> <http://www.w3.org/ns/shacl#SPARQLSelectValidator> .
<http://www.w3.org/ns/shacl#LessThanConstraintComponent> <http://www.w3.org/ns/shacl#message> "Value is not < value of {$lessThan}" .
_:Bb880e354f894466d96da68ac6732829f <http://www.w3.org/ns/shacl#jsLibrary> <http://datashapes.org/dash#DASHJSLibrary> .
_:Bcb38cdae1cd4f5c0b1a9201bb0062cdf <http://www.w3.org/ns/shacl#path> <http://www.w3.org/1999/02/22-rdf-syntax-ns#first> .
_:B1131591453602389668eae575a1a4693 <http://www.w3.org/ns/shacl#datatype> <http://www.w3.org/2001/XMLSchema#string> .
<http://datashapes.org/dash#SymmetricConstraintComponent-symmetric> <http://www.w3.org/1999/02/22-rdf-syntax-ns#type> <http://www.w3.org/ns/shacl#Parameter> .
_:B42c37f93cbd4d4c68e68cfec1631af95 <http://www.w3.org/ns/shacl#jsFunctionName> "validateDisjoint" .
<http://www.w3.org/ns/shacl#node> <http://datashapes.org/dash#defaultValueType> <http://www.w3.org/ns/shacl#NodeShape> .
_:B66978dfbb7ff7fc62ba1381b3242ae8e <http://www.w3.org/ns/shacl#jsFunctionName> "validateOr" .
<http://datashapes.org/dash#NonRecursiveConstraintComponent-nonRecursive> <http://www.w3.org/ns/shacl#path> <http://datashapes.org/dash#nonRecursive> .
<http://datashapes.org/dash#LangStringViewer> <http://www.w3.org/2000/01/rdf-schema#comment> "A Viewer for literals with a language tag, rendering as the text plus a language indicator." .
<http://datashapes.org/dash#toString> <http://datashapes.org/dash#cachable> "true"^^<http://www.w3.org/2001/XMLSchema#boolean> .
_:B42c37f93cbd4d4c68e68cfec1631af95 <http://www.w3.org/1999/02/22-rdf-syntax-ns#type> <http://www.w3.org/ns/shacl#JSValidator> .
<http://datashapes.org/dash#isLanguageIn> <http://www.w3.org/ns/shacl#ask> "\n\t\tASK {\n\t\t\tBIND (lang($value) AS ?valueLang) .\n\t\t\tFILTER EXISTS {\n\t\t\t\tGRAPH $shapesGraph {\n\t\t\t\t\t$languageIn (rdf:rest*)/rdf:first ?lang .\n\t\t\t\t    FILTER (langMatches(?valueLang, ?lang))\n\t\t\t\t} }\n\t\t}\n\t\t" .
<http://datashapes.org/dash#cachable> <http://www.w3.org/2000/01/rdf-schema#comment> "If set to true then the results of the SHACL function can be cached in between invocations with the same arguments. In other words, they are stateless and do not depend on triples in any graph, or the current time stamp etc." .
<http://datashapes.org/dash#LiteralViewer> <http://www.w3.org/2000/01/rdf-schema#comment> "A simple viewer for literals, rendering the lexical form of the value." .
<http://www.w3.org/ns/shacl#MaxLengthConstraintComponent> <http://www.w3.org/ns/shacl#targetClass> <http://www.w3.org/ns/shacl#Shape> .
<http://datashapes.org/dash#ClosedByTypesConstraintComponent> <http://www.w3.org/1999/02/22-rdf-syntax-ns#type> <http://www.w3.org/ns/shacl#ConstraintComponent> .
<http://datashapes.org/dash#HyperlinkViewer> <http://www.w3.org/2000/01/rdf-schema#comment> "A Viewer for literals, rendering as a hyperlink to a URL.\n\nFor literals it assumes the lexical form is the URL.\n\nThis is often used as default viewer for xsd:anyURI literals. Unsupported for blank nodes." .
<http://www.w3.org/ns/shacl#MaxLengthConstraintComponent> <http://www.w3.org/ns/shacl#validator> _:B0bddec390aebe99ada0a7924bd483b4f .
<http://datashapes.org/dash#SymmetricConstraintComponent> <http://www.w3.org/ns/shacl#message> "Symmetric value expected" .
<http://datashapes.org/dash#staticConstraint> <http://www.w3.org/2000/01/rdf-schema#domain> <http://www.w3.org/ns/shacl#ConstraintComponent> .
_:B6d4cbc3d992ff864f2dac864d1480fb8 <http://www.w3.org/ns/shacl#minCount> "1"^^<http://www.w3.org/2001/XMLSchema#integer> .
<http://datashapes.org/dash#InstancesSelectEditor> <http://www.w3.org/1999/02/22-rdf-syntax-ns#type> <http://datashapes.org/dash#Editor> .
<http://datashapes.org/dash#ClosedByTypesConstraintComponent> <http://www.w3.org/2000/01/rdf-schema#comment> "A constraint component that can be used to declare that focus nodes are \"closed\" based on their rdf:types, meaning that focus nodes may only have values for the properties that are explicitly enumerated via sh:property/sh:path in property constraints at their rdf:types and the superclasses of those. This assumes that the type classes are also shapes." .
<http://datashapes.org/dash#suggestionGroup> <http://www.w3.org/2000/01/rdf-schema#domain> <http://datashapes.org/dash#Suggestion> .
<http://datashapes.org/dash#SymmetricConstraintComponent> <http://www.w3.org/ns/shacl#propertyValidator> _:B61f5442de5a071e03f0bc4b21b3752cc .
<http://datashapes.org/dash#ClosedByTypesConstraintComponent> <http://www.w3.org/ns/shacl#nodeValidator> _:B4f9dd044b748456b76262d5363cb5a94 .
<http://datashapes.org/dash#StemConstraintComponent> <http://www.w3.org/ns/shacl#validator> _:Bf87fbb2c21e07adfb80e0445145d23a6 .
<http://datashapes.org/dash#PrimaryKeyConstraintComponent-uriStart> <http://www.w3.org/ns/shacl#name> "URI start" .
<http://datashapes.org/dash#toString> <http://www.w3.org/ns/shacl#returnType> <http://www.w3.org/2001/XMLSchema#string> .
<http://datashapes.org/dash#UniqueValueForClassConstraintComponent> <http://datashapes.org/dash#propertySuggestionGenerator> <http://topbraid.org/tosh#DeleteTripleSuggestionGenerator> .
_:Bcb38cdae1cd4f5c0b1a9201bb0062cdf <http://www.w3.org/ns/shacl#minCount> "1"^^<http://www.w3.org/2001/XMLSchema#integer> .
_:B9fe7602a489f48a08b22e99931d59d35 <http://www.w3.org/ns/shacl#maxCount> "1"^^<http://www.w3.org/2001/XMLSchema#integer> .
<http://datashapes.org/dash#SingleLineConstraintComponent> <http://www.w3.org/2000/01/rdf-schema#comment> "A constraint component that can be used to declare that all values that are literals must have a lexical form that contains no line breaks ('\\n' or '\\r').\n\nUser interfaces may use the dash:singleLine flag to prefer a text field over a (multi-line) text area." .
<http://www.w3.org/ns/shacl#MinLengthConstraintComponent> <http://www.w3.org/ns/shacl#labelTemplate> "Value must have less than {$minLength} characters" .
<http://www.w3.org/ns/shacl#parameter> <http://datashapes.org/dash#defaultValueType> <http://www.w3.org/ns/shacl#Parameter> .
<http://datashapes.org/dash#StringOrLangString> <http://www.w3.org/2000/01/rdf-schema#comment> "An rdf:List that can be used in property constraints as value for sh:or to indicate that all values of a property must be either xsd:string or rdf:langString." .
<http://www.w3.org/ns/shacl#NodeConstraintComponent> <http://www.w3.org/ns/shacl#validator> _:Bdad9596a4e29da75e0aa7a561275dd9f .
<http://datashapes.org/dash#RootClassConstraintComponent> <http://www.w3.org/2000/01/rdf-schema#label> "Root class constraint component" .
<http://datashapes.org/dash#defaultValueType> <http://www.w3.org/2000/01/rdf-schema#comment> "\n\t\tLinks a property with a default value type.\n\t\tThe default value type is assumed to be the <code>rdf:type</code> of values of the property\n\t\tthat declare no type on their own.\n\t\tAn example use of <code>sh:defaultValueType</code> is <code>sh:property</code>,\n\t\tthe values of which are assumed to be instances of <code>sh:PropertyShape</code>\n\t\teven if they are untyped (blank) nodes.\n\t\t"^^<http://www.w3.org/1999/02/22-rdf-syntax-ns#HTML> .
<http://datashapes.org/dash#deletedTriple> <http://www.w3.org/2000/01/rdf-schema#range> <http://www.w3.org/1999/02/22-rdf-syntax-ns#Statement> .
<http://datashapes.org/dash> <http://www.w3.org/2000/01/rdf-schema#label> "DASH Data Shapes Library" .
_:Be4b7da0362b43f04fa717e3e11887a9e <http://www.w3.org/1999/02/22-rdf-syntax-ns#type> <http://www.w3.org/ns/shacl#SPARQLSelectValidator> .
<http://datashapes.org/dash#isNodeKindIRI> <http://datashapes.org/dash#cachable> "true"^^<http://www.w3.org/2001/XMLSchema#boolean> .
<http://datashapes.org/dash#CoExistsWithConstraintComponent> <http://www.w3.org/2000/01/rdf-schema#comment> "A constraint component that can be used to express a constraint on property shapes so that if the property path has any value then the given property must also have a value, and vice versa." .
_:B5672337cd6b085d4efa2003d67fc0562 <http://www.w3.org/ns/shacl#class> <http://www.w3.org/2000/01/rdf-schema#Resource> .
<http://datashapes.org/dash#suggestionConfidence> <http://www.w3.org/2000/01/rdf-schema#range> <http://www.w3.org/2001/XMLSchema#decimal> .
_:Bd048027623bcc6288ff18f5d0dfbb126 <http://www.w3.org/1999/02/22-rdf-syntax-ns#type> <http://www.w3.org/ns/shacl#SPARQLSelectValidator> .
<http://www.w3.org/ns/shacl#MinInclusiveConstraintComponent> <http://www.w3.org/ns/shacl#labelTemplate> "Value must be >= {$minInclusive}" .
<http://datashapes.org/dash#FailureResult> <http://www.w3.org/2000/01/rdf-schema#comment> "A result representing a validation failure such as an unsupported recursion." .
<http://www.w3.org/ns/shacl#XoneConstraintComponent> <http://www.w3.org/ns/shacl#validator> _:B835aab3b1aa9569620d379dbdd889674 .
<http://datashapes.org/dash#hasClass> <http://www.w3.org/1999/02/22-rdf-syntax-ns#type> <http://www.w3.org/ns/shacl#SPARQLAskValidator> .
<http://datashapes.org/dash#coExistsWith> <http://www.w3.org/2000/01/rdf-schema#label> "co-exists with" .
<http://datashapes.org/dash#HasValueWithClassConstraintComponent> <http://www.w3.org/ns/shacl#message> "At least one of the values must be an instance of class {$hasValueWithClass}" .
<http://www.w3.org/ns/shacl#MaxInclusiveConstraintComponent> <http://www.w3.org/ns/shacl#targetClass> <http://www.w3.org/ns/shacl#Shape> .
<http://datashapes.org/dash#StemConstraintComponent> <http://www.w3.org/ns/shacl#validator> <http://datashapes.org/dash#hasStem> .
<http://datashapes.org/dash#SingleLineConstraintComponent> <http://www.w3.org/ns/shacl#parameter> _:B0c0f328c69e13d06674f58bb5b4a9284 .
_:B6df3b0d09d638883ddc7eaf55d1a9646 <http://www.w3.org/ns/shacl#class> <http://www.w3.org/2000/01/rdf-schema#Resource> .
<http://datashapes.org/dash#hasStem> <http://www.w3.org/2000/01/rdf-schema#comment> "Checks whether a given node is an IRI starting with a given stem." .
<http://datashapes.org/dash#valueCount> <http://www.w3.org/ns/shacl#returnType> <http://www.w3.org/2001/XMLSchema#integer> .
_:B8a6d95446c24ef2a1314f1cfdc6ea805 <http://www.w3.org/ns/shacl#select> "\n\t\tSELECT $this (?predicate AS ?path) ?value\n\t\tWHERE {\n\t\t\t{\n\t\t\t\tFILTER ($closed) .\n\t\t\t}\n\t\t\t$this ?predicate ?value .\n\t\t\tFILTER (NOT EXISTS {\n\t\t\t\tGRAPH $shapesGraph {\n\t\t\t\t\t$currentShape sh:property/sh:path ?predicate .\n\t\t\t\t}\n\t\t\t} && (!bound($ignoredProperties) || NOT EXISTS {\n\t\t\t\tGRAPH $shapesGraph {\n\t\t\t\t\t$ignoredProperties rdf:rest*/rdf:first ?predicate .\n\t\t\t\t}\n\t\t\t}))\n\t\t}\n" .
_:B6d4cbc3d992ff864f2dac864d1480fb8 <http://www.w3.org/ns/shacl#datatype> <http://www.w3.org/2001/XMLSchema#string> .
<http://datashapes.org/dash#cachable> <http://www.w3.org/1999/02/22-rdf-syntax-ns#type> <http://www.w3.org/1999/02/22-rdf-syntax-ns#Property> .
<http://datashapes.org/dash#HTMLOrStringOrLangString> <http://www.w3.org/1999/02/22-rdf-syntax-ns#type> <http://www.w3.org/1999/02/22-rdf-syntax-ns#List> .
_:B555c69d616b27a2b4c8744e4327dadf9 <http://www.w3.org/ns/shacl#prefixes> <http://datashapes.org/dash> .
<http://datashapes.org/dash#TestEnvironment> <http://www.w3.org/1999/02/22-rdf-syntax-ns#type> <http://www.w3.org/2000/01/rdf-schema#Class> .
<http://datashapes.org/dash#suggestionGroup> <http://www.w3.org/2000/01/rdf-schema#label> "suggestion" .
<http://datashapes.org/dash#SubSetOfConstraintComponent> <http://www.w3.org/ns/shacl#propertyValidator> _:B80b7e2f9fc1f404e1d9d214172e0e1b3 .
<http://www.w3.org/ns/shacl#MaxCountConstraintComponent> <http://www.w3.org/ns/shacl#labelTemplate> "Must not have more than {$maxCount} values" .
<http://datashapes.org/dash#abstract> <http://www.w3.org/2000/01/rdf-schema#label> "abstract" .
<http://datashapes.org/dash#PrimaryKeyConstraintComponent> <http://www.w3.org/1999/02/22-rdf-syntax-ns#type> <http://www.w3.org/ns/shacl#ConstraintComponent> .
<http://datashapes.org/dash#QueryTestCase> <http://www.w3.org/1999/02/22-rdf-syntax-ns#type> <http://www.w3.org/ns/shacl#NodeShape> .
<http://datashapes.org/dash#testModifiesEnvironment> <http://www.w3.org/1999/02/22-rdf-syntax-ns#type> <http://www.w3.org/1999/02/22-rdf-syntax-ns#Property> .
<http://datashapes.org/dash#suggestionGenerator> <http://www.w3.org/2000/01/rdf-schema#label> "suggestion generator" .
<http://www.w3.org/ns/shacl#MaxLengthConstraintComponent> <http://www.w3.org/ns/shacl#message> "Value has more than {$maxLength} characters" .
_:B835aab3b1aa9569620d379dbdd889674 <http://www.w3.org/ns/shacl#jsFunctionName> "validateXone" .
<http://datashapes.org/dash> <http://www.w3.org/2002/07/owl#imports> <http://topbraid.org/tosh> .
<http://datashapes.org/dash#deletedTriple> <http://www.w3.org/2000/01/rdf-schema#domain> <http://datashapes.org/dash#GraphUpdate> .
<http://datashapes.org/dash#ReifiableByConstraintComponent> <http://www.w3.org/ns/shacl#parameter> <http://datashapes.org/dash#ReifiableByConstraintComponent-reifiableBy> .
_:Be48162e9c0f86045a8d1a3b5697cfc8b <http://www.w3.org/ns/shacl#node> <http://datashapes.org/dash#ListNodeShape> .
<http://datashapes.org/dash#viewer> <http://www.w3.org/2000/01/rdf-schema#domain> <http://www.w3.org/ns/shacl#PropertyShape> .
<http://datashapes.org/dash#reifiableBy> <http://www.w3.org/2000/01/rdf-schema#range> <http://www.w3.org/ns/shacl#NodeShape> .
<http://www.w3.org/ns/shacl#MaxCountConstraintComponent> <http://www.w3.org/ns/shacl#message> "More than {$maxCount} values" .
<http://datashapes.org/dash#UniqueValueForClassConstraintComponent> <http://www.w3.org/ns/shacl#parameter> <http://datashapes.org/dash#UniqueValueForClassConstraintComponent-uniqueValueForClass> .
<http://datashapes.org/dash#ValueTableViewer> <http://www.w3.org/1999/02/22-rdf-syntax-ns#type> <http://datashapes.org/dash#Viewer> .
<http://datashapes.org/dash#expectedResult> <http://www.w3.org/2000/01/rdf-schema#domain> <http://datashapes.org/dash#TestCase> .
_:B0c0f328c69e13d06674f58bb5b4a9284 <http://www.w3.org/ns/shacl#description> "True to state that the lexical form of literal value nodes must not contain any line breaks. False to state that line breaks are explicitly permitted." .
<http://www.w3.org/ns/shacl#MaxInclusiveConstraintComponent> <http://www.w3.org/ns/shacl#labelTemplate> "Value must be <= {$maxInclusive}" .
<http://datashapes.org/dash#all> <http://www.w3.org/1999/02/22-rdf-syntax-ns#type> <http://www.w3.org/2000/01/rdf-schema#Resource> .
<http://www.w3.org/ns/shacl#MaxInclusiveConstraintComponent> <http://www.w3.org/ns/shacl#message> "Value is not <= {$maxInclusive}" .
<http://datashapes.org/dash#SymmetricConstraintComponent-symmetric> <http://www.w3.org/ns/shacl#path> <http://datashapes.org/dash#symmetric> .
<http://www.w3.org/ns/shacl#Shape> <http://datashapes.org/dash#abstract> "true"^^<http://www.w3.org/2001/XMLSchema#boolean> .
<http://www.w3.org/ns/shacl#LessThanConstraintComponent> <http://www.w3.org/ns/shacl#propertyValidator> _:B9e11ce9adf350d1895c6096c2ef7444d .
<http://datashapes.org/dash#editor> <http://www.w3.org/2000/01/rdf-schema#range> <http://datashapes.org/dash#Editor> .
<http://datashapes.org/dash#toString> <http://www.w3.org/1999/02/22-rdf-syntax-ns#type> <http://www.w3.org/ns/shacl#JSFunction> .
<http://datashapes.org/dash#SuggestionGenerator> <http://www.w3.org/1999/02/22-rdf-syntax-ns#type> <http://www.w3.org/2000/01/rdf-schema#Class> .
_:B881d49f14342613394c38418a3e2b26e <http://www.w3.org/1999/02/22-rdf-syntax-ns#type> <http://www.w3.org/ns/shacl#SPARQLSelectValidator> .
<http://datashapes.org/dash#deletedTriple> <http://www.w3.org/1999/02/22-rdf-syntax-ns#type> <http://www.w3.org/1999/02/22-rdf-syntax-ns#Property> .
<http://datashapes.org/dash#hasMaxExclusive> <http://www.w3.org/1999/02/22-rdf-syntax-ns#type> <http://www.w3.org/ns/shacl#SPARQLAskValidator> .
_:B8326699daa61eff99c25341497b7c80b <http://www.w3.org/ns/shacl#jsLibrary> <http://datashapes.org/dash#DASHJSLibrary> .
_:B6bbc6c369a762614c55c30d7d8b0f737 <http://www.w3.org/ns/shacl#jsLibrary> <http://datashapes.org/dash#DASHJSLibrary> .
<http://www.w3.org/ns/shacl#MinLengthConstraintComponent> <http://www.w3.org/ns/shacl#targetClass> <http://www.w3.org/ns/shacl#Shape> .
_:B96cb50ba954aab266bfb44f5557bd78e <http://www.w3.org/ns/shacl#path> <http://datashapes.org/dash#constraintOrShape> .
<http://datashapes.org/dash#suggestionGenerator> <http://www.w3.org/1999/02/22-rdf-syntax-ns#type> <http://www.w3.org/1999/02/22-rdf-syntax-ns#Property> .
<http://datashapes.org/dash#readOnly> <http://www.w3.org/2000/01/rdf-schema#domain> <http://www.w3.org/ns/shacl#PropertyShape> .
<http://www.w3.org/ns/shacl#HasValueConstraintComponent> <http://www.w3.org/ns/shacl#targetClass> <http://www.w3.org/ns/shacl#Shape> .
<http://datashapes.org/dash#JSTestCase> <http://www.w3.org/2000/01/rdf-schema#comment> "A test case that calls a given JavaScript function like a sh:JSFunction and compares its result with the dash:expectedResult." .
<http://datashapes.org/dash#TextFieldWithLangEditor> <http://www.w3.org/2000/01/rdf-schema#comment> "A single-line input field to enter the value of a literal and a drop down to select language, which is mandatory unless xsd:string is among the permissible datatypes." .
<http://www.w3.org/ns/shacl#ClosedConstraintComponent> <http://datashapes.org/dash#localConstraint> "true"^^<http://www.w3.org/2001/XMLSchema#boolean> .
<http://datashapes.org/dash#FunctionTestCase> <http://www.w3.org/2000/01/rdf-schema#comment> "A test case that verifies that a given SPARQL expression produces a given, expected result." .
<http://datashapes.org/dash#ParameterConstraintComponent> <http://www.w3.org/ns/shacl#parameter> <http://datashapes.org/dash#ParameterConstraintComponent-parameter> .
<http://www.w3.org/ns/shacl#MinCountConstraintComponent> <http://www.w3.org/ns/shacl#propertyValidator> _:B3b39cb9aee43fa574acdbcdac62b381f .
_:B42c37f93cbd4d4c68e68cfec1631af95 <http://www.w3.org/ns/shacl#jsLibrary> <http://datashapes.org/dash#DASHJSLibrary> .
<http://www.w3.org/ns/shacl#MinExclusiveConstraintComponent> <http://www.w3.org/ns/shacl#validator> <http://datashapes.org/dash#hasMinExclusive> .
_:B78dae72f06fd9f3e8a68413ba2347650 <http://www.w3.org/ns/shacl#prefixes> <http://datashapes.org/dash> .
_:B140f0995d12aa7e2492672c94ebf1c8f <http://www.w3.org/ns/shacl#namespace> "http://www.w3.org/1999/02/22-rdf-syntax-ns#"^^<http://www.w3.org/2001/XMLSchema#anyURI> .
<http://www.w3.org/ns/shacl#ClosedConstraintComponent> <http://www.w3.org/ns/shacl#labelTemplate> "Closed shape: only the enumerated properties can be used" .
_:Bc91acb30da815118fca913844f6cfa7b <http://www.w3.org/1999/02/22-rdf-syntax-ns#type> <http://www.w3.org/ns/shacl#JSValidator> .
<http://www.w3.org/ns/shacl#QualifiedMaxCountConstraintComponent> <http://www.w3.org/ns/shacl#message> "More than {$qualifiedMaxCount} values have shape {$qualifiedValueShape}" .
<http://datashapes.org/dash#SuccessTestCaseResult> <http://www.w3.org/2000/01/rdf-schema#subClassOf> <http://datashapes.org/dash#TestCaseResult> .
_:B1131591453602389668eae575a1a4693 <http://www.w3.org/ns/shacl#minCount> "1"^^<http://www.w3.org/2001/XMLSchema#integer> .
<http://datashapes.org/dash#expectedResultIsTTL> <http://www.w3.org/2000/01/rdf-schema#comment> "A flag to indicate that the expected result represents an RDF graph encoded as a Turtle file. If set to true, then tests would compare graphs instead of actual syntax." .
<http://datashapes.org/dash#AllSubjectsTarget> <http://www.w3.org/1999/02/22-rdf-syntax-ns#type> <http://www.w3.org/ns/shacl#SPARQLTargetType> .
_:Bb880e354f894466d96da68ac6732829f <http://www.w3.org/1999/02/22-rdf-syntax-ns#type> <http://www.w3.org/ns/shacl#JSValidator> .
_:B40fc13c18bcea97b695cedc8f377811f <http://www.w3.org/ns/shacl#class> <http://www.w3.org/ns/shacl#NodeKind> .
<http://datashapes.org/dash#ListNodeShape> <http://www.w3.org/ns/shacl#or> _:B160084f8X2D001cX2D4ef7X2Db5e9X2D120abccde94e .
<http://datashapes.org/dash#ParameterConstraintComponent-parameter> <http://www.w3.org/1999/02/22-rdf-syntax-ns#type> <http://www.w3.org/ns/shacl#Parameter> .
<http://www.w3.org/ns/shacl#NodeKindConstraintComponent> <http://www.w3.org/ns/shacl#targetClass> <http://www.w3.org/ns/shacl#Shape> .
_:B61f5442de5a071e03f0bc4b21b3752cc <http://www.w3.org/ns/shacl#prefixes> <http://datashapes.org/dash> .
<http://datashapes.org/dash#TestEnvironment> <http://www.w3.org/2000/01/rdf-schema#subClassOf> <http://www.w3.org/2000/01/rdf-schema#Resource> .
_:B31473064d8bd1e288bd70b63b0f116a3 <http://www.w3.org/ns/shacl#path> <http://datashapes.org/dash#nodeKind> .
<http://datashapes.org/dash#applicableToClass> <http://www.w3.org/2000/01/rdf-schema#comment> "Can be used to state that a shape is applicable to instances of a given class. This is a softer statement than \"target class\": a target means that all instances of the class must conform to the shape. Being applicable to simply means that the shape may apply to (some) instances of the class. This information can be used by algorithms or humans." .
<http://datashapes.org/dash#hasClass> <http://www.w3.org/2000/01/rdf-schema#label> "has class" .
_:B9c8553d682def0269e89fe21a9181cad <http://www.w3.org/1999/02/22-rdf-syntax-ns#type> <http://www.w3.org/ns/shacl#JSValidator> .
<http://datashapes.org/dash#suggestion> <http://www.w3.org/1999/02/22-rdf-syntax-ns#type> <http://www.w3.org/1999/02/22-rdf-syntax-ns#Property> .
<http://datashapes.org/dash#toString> <http://www.w3.org/ns/shacl#labelTemplate> "Convert {$arg} to xsd:string" .
<http://datashapes.org/dash#ValidationTestCase> <http://www.w3.org/2000/01/rdf-schema#subClassOf> <http://datashapes.org/dash#TestCase> .
<http://datashapes.org/dash#Viewer> <http://www.w3.org/1999/02/22-rdf-syntax-ns#type> <http://www.w3.org/2000/01/rdf-schema#Class> .
<http://www.w3.org/ns/shacl#Rules> <http://www.w3.org/1999/02/22-rdf-syntax-ns#type> <http://www.w3.org/2000/01/rdf-schema#Resource> .
<http://datashapes.org/dash#StemConstraintComponent-stem> <http://www.w3.org/ns/shacl#path> <http://datashapes.org/dash#stem> .
<http://datashapes.org/dash#hasRootClass> <http://www.w3.org/ns/shacl#ask> "ASK {\n    $value rdfs:subClassOf* $rootClass .\n}" .
<http://datashapes.org/dash#GraphUpdate> <http://www.w3.org/2000/01/rdf-schema#label> "Graph update" .
<http://datashapes.org/dash#SubSetOfConstraintComponent> <http://www.w3.org/ns/shacl#parameter> <http://datashapes.org/dash#SubSetOfConstraintComponent-subSetOf> .
<http://datashapes.org/dash#AllObjectsTarget> <http://www.w3.org/ns/shacl#prefixes> <http://datashapes.org/dash> .
<http://datashapes.org/dash#ImageViewer> <http://www.w3.org/2000/01/rdf-schema#label> "Image Viewer" .
_:B9c8553d682def0269e89fe21a9181cad <http://www.w3.org/ns/shacl#jsFunctionName> "validateCoExistsWith" .
<http://datashapes.org/dash#NonRecursiveConstraintComponent> <http://www.w3.org/ns/shacl#propertyValidator> _:B78dae72f06fd9f3e8a68413ba2347650 .
<http://datashapes.org/dash#UniqueValueForClassConstraintComponent> <http://www.w3.org/ns/shacl#targetClass> <http://www.w3.org/ns/shacl#PropertyShape> .
<http://datashapes.org/dash#TestCaseResult> <http://www.w3.org/2000/01/rdf-schema#subClassOf> <http://www.w3.org/ns/shacl#AbstractResult> .
<http://datashapes.org/dash#hasMaxExclusive> <http://www.w3.org/ns/shacl#prefixes> <http://datashapes.org/dash> .
_:B83c9da54cec674e1fa200619bc30f9bb <http://www.w3.org/ns/shacl#jsLibrary> <http://datashapes.org/dash#DASHJSLibrary> .
_:B31473064d8bd1e288bd70b63b0f116a3 <http://www.w3.org/ns/shacl#name> "node kind" .
_:B160084f8X2D001cX2D4ef7X2Db5e9X2D120abccde94e <http://www.w3.org/1999/02/22-rdf-syntax-ns#first> _:B5ea6cb49b4f6b98c242342a8a98d3388 .
<http://datashapes.org/dash#StemConstraintComponent> <http://www.w3.org/ns/shacl#targetClass> <http://www.w3.org/ns/shacl#Shape> .
_:B485dc9d077951c4a981419e27a12efce <http://www.w3.org/ns/shacl#name> "subject" .
_:B66978dfbb7ff7fc62ba1381b3242ae8e <http://www.w3.org/1999/02/22-rdf-syntax-ns#type> <http://www.w3.org/ns/shacl#JSValidator> .
<http://www.w3.org/ns/shacl#NodeKindConstraintComponent> <http://www.w3.org/ns/shacl#labelTemplate> "Value must have node kind {$nodeKind}" .
<http://datashapes.org/dash#isNodeKindBlankNode> <http://www.w3.org/ns/shacl#returnType> <http://www.w3.org/2001/XMLSchema#boolean> .
<http://datashapes.org/dash#RootClassConstraintComponent> <http://www.w3.org/ns/shacl#message> "Value must be subclass of {$rootClass}" .
_:B8326699daa61eff99c25341497b7c80b <http://www.w3.org/ns/shacl#jsFunctionName> "validateSubSetOf" .
<http://datashapes.org/dash#hasNodeKind> <http://www.w3.org/2000/01/rdf-schema#label> "has node kind" .
_:B485dc9d077951c4a981419e27a12efce <http://www.w3.org/ns/shacl#description> "The subject to get the number of objects of." .
_:B12898dca29ca363f5ae4b1b4c90c363b <http://www.w3.org/ns/shacl#minCount> "1"^^<http://www.w3.org/2001/XMLSchema#integer> .
_:B80b7e2f9fc1f404e1d9d214172e0e1b3 <http://www.w3.org/ns/shacl#ask> "ASK {\n    $this $subSetOf $value .\n}" .
_:B0bddec390aebe99ada0a7924bd483b4f <http://www.w3.org/ns/shacl#jsLibrary> <http://datashapes.org/dash#DASHJSLibrary> .
<http://datashapes.org/dash#DefaultValueTypeRule> <http://www.w3.org/1999/02/22-rdf-syntax-ns#type> <http://www.w3.org/ns/shacl#SPARQLConstructExecutable> .
_:B7f1ad1df154d5b4790aefb896d1c9fb8 <http://www.w3.org/ns/shacl#description> "True to indicate that this function will always return the same values for the same combination of arguments, regardless of the query graphs. Engines can use this information to cache and reuse previous function calls." .
<http://datashapes.org/dash#UniqueValueForClassConstraintComponent> <http://www.w3.org/ns/shacl#labelTemplate> "Values must be unique among all instances of {?uniqueValueForClass}" .
<http://datashapes.org/dash#valueCount> <http://www.w3.org/2000/01/rdf-schema#label> "value count" .
_:B707d4e7635546fda18ee3fda129e9373 <http://www.w3.org/1999/02/22-rdf-syntax-ns#type> <http://www.w3.org/ns/shacl#JSValidator> .
<http://www.w3.org/ns/shacl#UniqueLangConstraintComponent> <http://www.w3.org/ns/shacl#propertyValidator> _:Bb254f7a557dd3b29bbe20622d1b148be .
<http://datashapes.org/dash#SuggestionGenerator> <http://www.w3.org/2000/01/rdf-schema#label> "Suggestion generator" .
<http://www.w3.org/2002/07/owl#Class> <http://www.w3.org/1999/02/22-rdf-syntax-ns#type> <http://www.w3.org/2000/01/rdf-schema#Class> .
<http://datashapes.org/dash#localConstraint> <http://www.w3.org/2000/01/rdf-schema#label> "local constraint" .
_:Baf7234052e57bdd00025c4c0de812c1d <http://www.w3.org/ns/shacl#message> "Missing expected value {$hasValue}" .
<http://datashapes.org/dash#RootClassConstraintComponent> <http://www.w3.org/1999/02/22-rdf-syntax-ns#type> <http://www.w3.org/ns/shacl#ConstraintComponent> .
_:Baca6b78cb251a419ee913fa362fa0fad <http://www.w3.org/1999/02/22-rdf-syntax-ns#type> <http://www.w3.org/ns/shacl#JSValidator> .
<http://www.w3.org/ns/shacl#MaxLengthConstraintComponent> <http://www.w3.org/ns/shacl#validator> <http://datashapes.org/dash#hasMaxLength> .
<http://datashapes.org/dash#SymmetricConstraintComponent> <http://www.w3.org/2000/01/rdf-schema#comment> "A contraint component for property shapes to validate that a property is symmetric. For symmetric properties, if A relates to B then B must relate to A." .
<http://datashapes.org/dash#AllObjectsTarget> <http://www.w3.org/2000/01/rdf-schema#subClassOf> <http://www.w3.org/ns/shacl#Target> .
<http://datashapes.org/dash#None> <http://www.w3.org/2000/01/rdf-schema#comment> "A Shape that is no node can conform to." .
_:Ba94bb54840f7b2f2def8b93e306cd9bf <http://www.w3.org/ns/shacl#description> "If set to true, this test case will be skipped." .
<http://www.w3.org/ns/shacl#HasValueConstraintComponent> <http://www.w3.org/ns/shacl#propertyValidator> _:B3198ee9db9f046c7a63785bb62bb0766 .
<http://datashapes.org/dash#SuggestionGenerator> <http://www.w3.org/2000/01/rdf-schema#subClassOf> <http://www.w3.org/2000/01/rdf-schema#Resource> .
<http://datashapes.org/dash#composite> <http://www.w3.org/2000/01/rdf-schema#domain> <http://www.w3.org/ns/shacl#PropertyShape> .
_:B1db6386c181b226090f5a502966d369b <http://www.w3.org/ns/shacl#jsFunctionName> "validateLanguageIn" .
<http://datashapes.org/dash#hasClass> <http://www.w3.org/ns/shacl#prefixes> <http://datashapes.org/dash> .
<http://www.w3.org/ns/shacl#MinCountConstraintComponent> <http://datashapes.org/dash#localConstraint> "true"^^<http://www.w3.org/2001/XMLSchema#boolean> .
_:B8ba63feb6e245955b305042229b7785c <http://www.w3.org/1999/02/22-rdf-syntax-ns#type> <http://www.w3.org/ns/shacl#JSValidator> .
<http://www.w3.org/ns/shacl#MinInclusiveConstraintComponent> <http://www.w3.org/ns/shacl#targetClass> <http://www.w3.org/ns/shacl#Shape> .
<http://www.w3.org/ns/shacl#MinExclusiveConstraintComponent> <http://www.w3.org/ns/shacl#targetClass> <http://www.w3.org/ns/shacl#Shape> .
<http://datashapes.org/dash#InferencingTestCase> <http://www.w3.org/1999/02/22-rdf-syntax-ns#type> <http://www.w3.org/ns/shacl#NodeShape> .
_:Bd5a64ddffc0079f527ee5678e81011df <http://www.w3.org/ns/shacl#path> <http://datashapes.org/dash#expectedResult> .
<http://datashapes.org/dash#TextAreaEditor> <http://www.w3.org/1999/02/22-rdf-syntax-ns#type> <http://datashapes.org/dash#Editor> .
<http://datashapes.org/dash#QueryTestCase> <http://www.w3.org/ns/shacl#property> _:B1131591453602389668eae575a1a4693 .
<http://www.w3.org/ns/shacl#order> <http://www.w3.org/2000/01/rdf-schema#range> <http://www.w3.org/2001/XMLSchema#decimal> .
<http://datashapes.org/dash#PrimaryKeyConstraintComponent> <http://www.w3.org/ns/shacl#message> "Violation of primary key constraint" .
<http://datashapes.org/dash#NonRecursiveConstraintComponent> <http://www.w3.org/ns/shacl#targetClass> <http://www.w3.org/ns/shacl#PropertyShape> .
<http://datashapes.org/dash#hasStem> <http://www.w3.org/2000/01/rdf-schema#label> "has stem" .
<http://datashapes.org/dash#PrimaryKeyConstraintComponent> <http://www.w3.org/2000/01/rdf-schema#comment> "Enforces a constraint that the given property (sh:path) serves as primary key for all resources in the target of the shape. If a property has been declared to be the primary key then each resource must have exactly one value for that property. Furthermore, the URIs of those resources must start with a given string (dash:uriStart), followed by the URL-encoded primary key value. For example if dash:uriStart is \"http://example.org/country-\" and the primary key for an instance is \"de\" then the URI must be \"http://example.org/country-de\". Finally, as a result of the URI policy, there can not be any other resource with the same value under the same primary key policy." .
<http://www.w3.org/ns/shacl#MaxLengthConstraintComponent> <http://www.w3.org/ns/shacl#labelTemplate> "Value must not have more than {$maxLength} characters" .
_:B2b4ab9b1e883630e0b4029800ec9db7e <http://www.w3.org/ns/shacl#maxCount> "0"^^<http://www.w3.org/2001/XMLSchema#integer> .
<http://datashapes.org/dash#SPARQLConstructTemplate> <http://www.w3.org/2000/01/rdf-schema#label> "SPARQL CONSTRUCT template" .
_:Bfb96260a3d1be1805270339a2809aef8 <http://www.w3.org/ns/shacl#datatype> <http://www.w3.org/2001/XMLSchema#dateTime> .
<http://datashapes.org/dash#x> <http://www.w3.org/2000/01/rdf-schema#label> "x" .
<http://datashapes.org/dash#testEnvironment> <http://www.w3.org/2000/01/rdf-schema#domain> <http://datashapes.org/dash#TestCase> .
<http://datashapes.org/dash#y> <http://www.w3.org/2000/01/rdf-schema#label> "y" .
<http://datashapes.org/dash#RDFQueryJSLibrary> <http://www.w3.org/ns/shacl#jsLibraryURL> "http://datashapes.org/js/rdfquery.js"^^<http://www.w3.org/2001/XMLSchema#anyURI> .
<http://datashapes.org/dash#defaultViewForRole> <http://www.w3.org/2000/01/rdf-schema#comment> "Links a node shape with the roles for which it shall be used as default view. User interfaces can use these values to select how to present a given RDF resource. The values of this property are URIs representing a group of users or agents. There is a dedicated URI dash:all representing all users." .
<http://datashapes.org/dash#GraphValidationTestCase> <http://www.w3.org/2000/01/rdf-schema#comment> "A test case that performs SHACL constraint validation on the whole graph and compares the results with the expected validation results stored with the test case. By default this excludes meta-validation (i.e. the validation of the shape definitions themselves). If that's desired, set dash:validateShapes to true." .
<http://datashapes.org/dash#composite> <http://www.w3.org/2000/01/rdf-schema#comment> "Can be used to indicate that a property/path represented by a property constraint represents a composite relationship. In a composite relationship, the life cycle of a \"child\" object (value of the property/path) depends on the \"parent\" object (focus node). If the parent gets deleted, then the child objects should be deleted, too. Tools may use dash:composite (if set to true) to implement cascading delete operations." .
<http://datashapes.org/dash#GraphStoreTestCase> <http://www.w3.org/ns/shacl#property> _:Bbc6a3e0006c01fd1021e9a87d62d127a .
<http://datashapes.org/dash#UniqueValueForClassConstraintComponent> <http://www.w3.org/2000/01/rdf-schema#label> "Unique value for class constraint component" .
_:B96cb50ba954aab266bfb44f5557bd78e <http://www.w3.org/ns/shacl#description> "The sh:Constraint or sh:Shape to test." .
<http://datashapes.org/dash#isDeactivated> <http://www.w3.org/ns/shacl#prefixes> <http://datashapes.org/dash> .
_:B6df3b0d09d638883ddc7eaf55d1a9646 <http://www.w3.org/ns/shacl#path> <http://datashapes.org/dash#testGraph> .
<http://datashapes.org/dash> <http://www.w3.org/ns/shacl#declare> _:Ba6e7b59cb1609800d73a83169cfb1050 .
<http://datashapes.org/dash#Suggestion> <http://datashapes.org/dash#abstract> "true"^^<http://www.w3.org/2001/XMLSchema#boolean> .
<http://datashapes.org/dash#hidden> <http://www.w3.org/2000/01/rdf-schema#range> <http://www.w3.org/2001/XMLSchema#boolean> .
<http://www.w3.org/ns/shacl#MinInclusiveConstraintComponent> <http://www.w3.org/ns/shacl#validator> _:B21421ade4ccc7092969f52bbcc0d7484 .
<http://www.w3.org/ns/shacl#MaxCountConstraintComponent> <http://www.w3.org/ns/shacl#targetClass> <http://www.w3.org/ns/shacl#PropertyShape> .
_:B104823182afa6c235b8daed98b3b5ac7 <http://www.w3.org/ns/shacl#path> _:Bcfe9344fc73c29171f67ab7f8d807e68 .
_:Baca6b78cb251a419ee913fa362fa0fad <http://www.w3.org/ns/shacl#jsLibrary> <http://datashapes.org/dash#DASHJSLibrary> .
_:Ba94bb54840f7b2f2def8b93e306cd9bf <http://www.w3.org/ns/shacl#maxCount> "1"^^<http://www.w3.org/2001/XMLSchema#integer> .
_:B7463b1c77e1b791dc8f96918e9ed48ab <http://www.w3.org/ns/shacl#not> _:B06b9e21bc94574feceeed0f3417951b5 .
<http://datashapes.org/dash#SuccessResult> <http://www.w3.org/2000/01/rdf-schema#label> "Success result" .
<http://datashapes.org/dash#Widget> <http://www.w3.org/2000/01/rdf-schema#comment> "Base class of user interface components that can be used to display or edit value nodes." .
_:Ba6e7b59cb1609800d73a83169cfb1050 <http://www.w3.org/ns/shacl#namespace> "http://datashapes.org/dash#"^^<http://www.w3.org/2001/XMLSchema#anyURI> .
<http://datashapes.org/dash#isNodeKindLiteral> <http://datashapes.org/dash#cachable> "true"^^<http://www.w3.org/2001/XMLSchema#boolean> .
<http://datashapes.org/dash#LabelViewer> <http://www.w3.org/2000/01/rdf-schema#comment> "A Viewer for URI resources, rendering as a hyperlink to that URI based on the display label of the resource. Also includes other ways of interacting with the URI such as opening a nested summary display." .
<http://datashapes.org/dash#TestEnvironment> <http://www.w3.org/2000/01/rdf-schema#label> "Test environment" .
<http://datashapes.org/dash#InferencingTestCase> <http://www.w3.org/ns/shacl#property> _:B3b32abda9658f358f57cc4b5edac88b8 .
<http://datashapes.org/dash#SingleLineConstraintComponent> <http://www.w3.org/ns/shacl#targetClass> <http://www.w3.org/ns/shacl#PropertyShape> .
<http://datashapes.org/dash#AllSubjects> <http://www.w3.org/1999/02/22-rdf-syntax-ns#type> <http://datashapes.org/dash#AllSubjectsTarget> .
_:Be48162e9c0f86045a8d1a3b5697cfc8b <http://www.w3.org/ns/shacl#path> _:Bf9e0a90e2bec32cab15ae9486a22ce81 .
<http://datashapes.org/dash#CoExistsWithConstraintComponent> <http://www.w3.org/ns/shacl#targetClass> <http://www.w3.org/ns/shacl#PropertyShape> .
_:B0cd35e055bd003648f8b9739d1d3297a <http://www.w3.org/ns/shacl#prefixes> <http://datashapes.org/dash> .
_:B6431ca200460b7f86c096adcb4867b07 <http://www.w3.org/ns/shacl#path> <http://datashapes.org/dash#expectedResult> .
<http://datashapes.org/dash#defaultValueType> <http://www.w3.org/2002/07/owl#versionInfo> "Note this property may get removed in future versions. It is a left-over from a previous design in SHACL." .
<http://datashapes.org/dash#FailureTestCaseResult> <http://www.w3.org/2000/01/rdf-schema#subClassOf> <http://datashapes.org/dash#TestCaseResult> .
_:B8ba63feb6e245955b305042229b7785c <http://www.w3.org/ns/shacl#jsLibrary> <http://datashapes.org/dash#DASHJSLibrary> .
<http://www.w3.org/ns/shacl#Rules> <http://www.w3.org/2000/01/rdf-schema#label> "SHACL Rules" .
_:Bbc6a3e0006c01fd1021e9a87d62d127a <http://www.w3.org/ns/shacl#minCount> "1"^^<http://www.w3.org/2001/XMLSchema#integer> .
<http://datashapes.org/dash#SubSetOfConstraintComponent> <http://www.w3.org/ns/shacl#validator> _:B8326699daa61eff99c25341497b7c80b .
_:B0c0f328c69e13d06674f58bb5b4a9284 <http://www.w3.org/ns/shacl#name> "single line" .
_:Baf7234052e57bdd00025c4c0de812c1d <http://www.w3.org/1999/02/22-rdf-syntax-ns#type> <http://www.w3.org/ns/shacl#SPARQLSelectValidator> .
<http://datashapes.org/dash#rootClass> <http://www.w3.org/1999/02/22-rdf-syntax-ns#type> <http://www.w3.org/1999/02/22-rdf-syntax-ns#Property> .
_:B3b39cb9aee43fa574acdbcdac62b381f <http://www.w3.org/ns/shacl#jsFunctionName> "validateMinCountProperty" .
_:B850a3561a7b96169d0a48349ceccf59d <http://www.w3.org/ns/shacl#jsFunctionName> "validateUniqueLangProperty" .
_:B83c9da54cec674e1fa200619bc30f9bb <http://www.w3.org/1999/02/22-rdf-syntax-ns#type> <http://www.w3.org/ns/shacl#JSValidator> .
_:B8a6d95446c24ef2a1314f1cfdc6ea805 <http://www.w3.org/ns/shacl#message> "Predicate {?path} is not allowed (closed shape)" .
_:B66978dfbb7ff7fc62ba1381b3242ae8e <http://www.w3.org/ns/shacl#jsLibrary> <http://datashapes.org/dash#DASHJSLibrary> .
<http://datashapes.org/dash#DateOrDateTime> <http://www.w3.org/2000/01/rdf-schema#label> "Date or date time" .
<http://datashapes.org/dash#DefaultValueTypeRule> <http://www.w3.org/ns/shacl#construct> "\n\t\tCONSTRUCT {\n\t\t\t?node a ?defaultValueType .\n\t\t}\n\t\tWHERE {\n\t\t\t?predicate sh:defaultValueType ?defaultValueType .\n\t\t\t?anySubject ?predicate ?node .\n\t\t\tFILTER (NOT EXISTS { ?node a ?anyType }) .\n\t\t}\n\t\t" .
<http://datashapes.org/dash#toString> <http://www.w3.org/ns/shacl#parameter> _:Ba6acc14fd45c4c8b7041edd8b3005f16 .
<http://www.w3.org/ns/shacl#HasValueConstraintComponent> <http://www.w3.org/ns/shacl#propertyValidator> _:Baf7234052e57bdd00025c4c0de812c1d .
<http://datashapes.org/dash#UniqueValueForClassConstraintComponent> <http://www.w3.org/2000/01/rdf-schema#comment> "A constraint component that can be used to state that the values of a property must be unique for all instances of a given class (and its subclasses)." .
_:B9c8553d682def0269e89fe21a9181cad <http://www.w3.org/ns/shacl#jsLibrary> <http://datashapes.org/dash#DASHJSLibrary> .
<http://datashapes.org/dash#expectedResult> <http://www.w3.org/1999/02/22-rdf-syntax-ns#type> <http://www.w3.org/1999/02/22-rdf-syntax-ns#Property> .
<http://datashapes.org/dash#isNodeKindBlankNode> <http://www.w3.org/ns/shacl#parameter> _:B40fc13c18bcea97b695cedc8f377811f .
<http://datashapes.org/dash#localConstraint> <http://www.w3.org/1999/02/22-rdf-syntax-ns#type> <http://www.w3.org/1999/02/22-rdf-syntax-ns#Property> .
<http://datashapes.org/dash#fixed> <http://www.w3.org/2000/01/rdf-schema#range> <http://www.w3.org/2001/XMLSchema#boolean> .
_:B4f9dd044b748456b76262d5363cb5a94 <http://www.w3.org/ns/shacl#prefixes> <http://datashapes.org/dash> .
<http://datashapes.org/dash#PrimaryKeyConstraintComponent-uriStart> <http://www.w3.org/ns/shacl#datatype> <http://www.w3.org/2001/XMLSchema#string> .
<http://datashapes.org/dash#SubSetOfConstraintComponent-subSetOf> <http://www.w3.org/ns/shacl#path> <http://datashapes.org/dash#subSetOf> .
<http://datashapes.org/dash#StringOrLangString> <http://www.w3.org/1999/02/22-rdf-syntax-ns#rest> _:B474b201cX2D1114X2D493aX2Da90bX2D68fa0363bb24 .
_:B707d4e7635546fda18ee3fda129e9373 <http://www.w3.org/ns/shacl#jsLibrary> <http://datashapes.org/dash#DASHJSLibrary> .
<http://datashapes.org/dash#validateShapes> <http://www.w3.org/2000/01/rdf-schema#range> <http://www.w3.org/2001/XMLSchema#boolean> .
<http://www.w3.org/ns/shacl#EqualsConstraintComponent> <http://www.w3.org/ns/shacl#targetClass> <http://www.w3.org/ns/shacl#Shape> .
_:B4f9dd044b748456b76262d5363cb5a94 <http://www.w3.org/ns/shacl#message> "Property {?path} is not among those permitted for any of the types" .
<http://datashapes.org/dash#testModifiesEnvironment> <http://www.w3.org/2000/01/rdf-schema#domain> <http://datashapes.org/dash#TestCase> .
<http://datashapes.org/dash#AllSubjectsTarget> <http://www.w3.org/ns/shacl#select> "SELECT DISTINCT ?this\nWHERE {\n    ?this ?anyP ?anyO .\n}" .
<http://datashapes.org/dash#isNodeKindLiteral> <http://www.w3.org/2000/01/rdf-schema#label> "is NodeKind Literal" .
<http://datashapes.org/dash#propertySuggestionGenerator> <http://www.w3.org/2000/01/rdf-schema#domain> <http://www.w3.org/ns/shacl#ConstraintComponent> .
<http://datashapes.org/dash#subSetOf> <http://www.w3.org/1999/02/22-rdf-syntax-ns#type> <http://www.w3.org/1999/02/22-rdf-syntax-ns#Property> .
_:B44ba6ca913112e299d99b54732ce1509 <http://www.w3.org/1999/02/22-rdf-syntax-ns#type> <http://www.w3.org/ns/shacl#SPARQLSelectValidator> .
<http://www.w3.org/ns/shacl#QualifiedMinCountConstraintComponent> <http://www.w3.org/ns/shacl#targetClass> <http://www.w3.org/ns/shacl#PropertyShape> .
_:Be4f653eeb42a8e37fe88ebda84c784fa <http://www.w3.org/ns/shacl#datatype> <http://www.w3.org/2001/XMLSchema#string> .
<http://datashapes.org/dash#SuccessTestCaseResult> <http://www.w3.org/2000/01/rdf-schema#label> "Success test case result" .
_:B0bddec390aebe99ada0a7924bd483b4f <http://www.w3.org/1999/02/22-rdf-syntax-ns#type> <http://www.w3.org/ns/shacl#JSValidator> .
_:B5ea6cb49b4f6b98c242342a8a98d3388 <http://www.w3.org/ns/shacl#property> _:B2b4ab9b1e883630e0b4029800ec9db7e .
_:B51e81f8eX2Dded0X2D4b0bX2D97bbX2Dea24608138ee <http://www.w3.org/1999/02/22-rdf-syntax-ns#rest> <http://www.w3.org/1999/02/22-rdf-syntax-ns#nil> .
<http://www.w3.org/ns/shacl#NodeKindConstraintComponent> <http://www.w3.org/ns/shacl#validator> _:Beb225391b5ff8fb10e272118f430ade4 .
_:Ba94bb54840f7b2f2def8b93e306cd9bf <http://www.w3.org/ns/shacl#path> <http://www.w3.org/ns/shacl#deactivated> .
<http://datashapes.org/dash#isNodeKindLiteral> <http://www.w3.org/ns/shacl#ask> "ASK {\n\tFILTER ($nodeKind IN ( sh:Literal, sh:BlankNodeOrLiteral, sh:IRIOrLiteral ))\n}" .
_:Bf9e0a90e2bec32cab15ae9486a22ce81 <http://www.w3.org/ns/shacl#zeroOrMorePath> <http://www.w3.org/1999/02/22-rdf-syntax-ns#rest> .
_:B2cb630d3ce6cc80fcb0af823135f42af <http://www.w3.org/ns/shacl#path> <http://datashapes.org/dash#expression> .
<http://datashapes.org/dash#testModifiesEnvironment> <http://www.w3.org/2000/01/rdf-schema#comment> "Indicates whether this test modifies the specified dash:testEnvironment. If set to true then a test runner can make sure to wipe out the previous environment, while leaving it false (or undefined) means that the test runner can reuse the environment from the previous test case. As setting up and tearing down tests is sometimes slow, this flag can significantly accelerate test execution." .
_:B150417b36eb7ea87cdf5e9ac4c94221b <http://www.w3.org/1999/02/22-rdf-syntax-ns#type> <http://www.w3.org/ns/shacl#SPARQLSelectValidator> .
_:B06b9e21bc94574feceeed0f3417951b5 <http://www.w3.org/ns/shacl#hasValue> <http://www.w3.org/1999/02/22-rdf-syntax-ns#nil> .
<http://www.w3.org/ns/shacl#HasValueConstraintComponent> <http://www.w3.org/ns/shacl#labelTemplate> "Must have value {$hasValue}" .
<http://datashapes.org/dash#HTMLOrStringOrLangString> <http://www.w3.org/1999/02/22-rdf-syntax-ns#first> _:Bbbfe7c69c794385222859a92b4606741 .
_:B12898dca29ca363f5ae4b1b4c90c363b <http://www.w3.org/ns/shacl#name> "test case" .
_:B35bf980a43fa9fd53edf3a01919e908b <http://www.w3.org/ns/shacl#prefixes> <http://datashapes.org/dash> .
<http://datashapes.org/dash#applicableToClass> <http://www.w3.org/2000/01/rdf-schema#domain> <http://www.w3.org/ns/shacl#Shape> .
<http://datashapes.org/dash#toString> <http://www.w3.org/ns/shacl#select> "SELECT (xsd:string($arg) AS ?result)\nWHERE {\n}" .
<http://www.w3.org/ns/shacl#QualifiedMaxCountConstraintComponent> <http://www.w3.org/ns/shacl#propertyValidator> _:B1f243cca064dc36a3759b064b48d1d3d .
<http://datashapes.org/dash#TextAreaEditor> <http://www.w3.org/2000/01/rdf-schema#label> "Text area editor" .
_:B9f5ec4ceX2D5991X2D4a1dX2Da81aX2D237da79bf345 <http://www.w3.org/1999/02/22-rdf-syntax-ns#first> _:Be4f653eeb42a8e37fe88ebda84c784fa .
_:B78dae72f06fd9f3e8a68413ba2347650 <http://www.w3.org/ns/shacl#select> "SELECT DISTINCT $this ($this AS ?value)\nWHERE {\n\t{\n\t\tFILTER (?nonRecursive)\n\t}\n    $this $PATH $this .\n}" .
<http://datashapes.org/dash#hasMinLength> <http://www.w3.org/ns/shacl#ask> "\n\t\tASK {\n\t\t\tFILTER (STRLEN(str($value)) >= $minLength) .\n\t\t}\n\t\t" .
<http://datashapes.org/dash#isNodeKindIRI> <http://www.w3.org/ns/shacl#returnType> <http://www.w3.org/2001/XMLSchema#boolean> .
<http://datashapes.org/dash#AllSubjectsTarget> <http://www.w3.org/ns/shacl#jsLibrary> <http://datashapes.org/dash#DASHJSLibrary> .
<http://datashapes.org/dash#SPARQLUpdateSuggestionGenerator> <http://www.w3.org/2000/01/rdf-schema#subClassOf> <http://datashapes.org/dash#SuggestionGenerator> .
<http://datashapes.org/dash#HasValueWithClassConstraintComponent> <http://www.w3.org/ns/shacl#propertyValidator> _:B707d4e7635546fda18ee3fda129e9373 .
<http://datashapes.org/dash#SuggestionResult> <http://www.w3.org/2000/01/rdf-schema#comment> "Class of results that have been produced as suggestions, not through SHACL validation. How the actual results are produced is up to implementers. Each instance of this class should have values for sh:focusNode, sh:resultMessage, sh:resultSeverity (suggested default: sh:Info), and dash:suggestion to point at one or more suggestions." .
<http://datashapes.org/dash#x> <http://www.w3.org/2000/01/rdf-schema#range> <http://www.w3.org/2001/XMLSchema#integer> .
_:B13da662fb0d609b0fa8798a656baca2d <http://www.w3.org/ns/shacl#jsFunctionName> "validatePattern" .
_:Bf2df11d10c098c62248867b2af223317 <http://www.w3.org/ns/shacl#prefix> "xsd" .
<http://datashapes.org/dash#SymmetricConstraintComponent> <http://www.w3.org/1999/02/22-rdf-syntax-ns#type> <http://www.w3.org/ns/shacl#ConstraintComponent> .
<http://datashapes.org/dash#includedExecutionPlatform> <http://www.w3.org/1999/02/22-rdf-syntax-ns#type> <http://www.w3.org/1999/02/22-rdf-syntax-ns#Property> .
<http://datashapes.org/dash#detailsGraph> <http://www.w3.org/2000/01/rdf-schema#comment> "Can be used to link a SHACL property shape with a SHACL node expression that produces the URIs of one or more graphs that contain further RDF triples for the value nodes delivered by the property. This can be used to inform a processor that it should switch to another data graph when the user wants to retrieve more information about a value.\n\nThe node expressions are evaluated with the focus node as input. (It is unclear whether there are also cases where the result may be different for each specific value, in which case the node expression would need a second input argument).\n\nThis property should be regarded as an \"annotation\", i.e. it does not have any impact on validation or other built-in SHACL features. However, selected tools may want to use this information." .
<http://datashapes.org/dash#y> <http://www.w3.org/2000/01/rdf-schema#range> <http://www.w3.org/2001/XMLSchema#integer> .
<http://datashapes.org/dash#TestEnvironment> <http://datashapes.org/dash#abstract> "true"^^<http://www.w3.org/2001/XMLSchema#boolean> .
<http://datashapes.org/dash#SPARQLConstructTemplate> <http://www.w3.org/1999/02/22-rdf-syntax-ns#type> <http://www.w3.org/2000/01/rdf-schema#Class> .
_:B8ba63feb6e245955b305042229b7785c <http://www.w3.org/ns/shacl#jsFunctionName> "validateMaxCountProperty" .
<http://www.w3.org/ns/shacl#MinExclusiveConstraintComponent> <http://www.w3.org/ns/shacl#message> "Value is not > {$minExclusive}" .
<http://datashapes.org/dash#ClosedByTypesConstraintComponent-closedByTypes> <http://www.w3.org/1999/02/22-rdf-syntax-ns#type> <http://www.w3.org/ns/shacl#Parameter> .
<http://datashapes.org/dash#Viewer> <http://www.w3.org/1999/02/22-rdf-syntax-ns#type> <http://www.w3.org/ns/shacl#NodeShape> .
<http://www.w3.org/ns/shacl#EqualsConstraintComponent> <http://www.w3.org/ns/shacl#nodeValidator> _:B8137cd87d692f6f1ad4d374873d42a49 .
_:Bb254f7a557dd3b29bbe20622d1b148be <http://www.w3.org/ns/shacl#prefixes> <http://datashapes.org/dash> .
<http://datashapes.org/dash#isIn> <http://www.w3.org/ns/shacl#prefixes> <http://datashapes.org/dash> .
_:Bf0deb4dbfedca171cbc3d5e34c7d597d <http://www.w3.org/ns/shacl#maxCount> "0"^^<http://www.w3.org/2001/XMLSchema#integer> .
<http://datashapes.org/dash#JSTestCase> <http://www.w3.org/2000/01/rdf-schema#subClassOf> <http://www.w3.org/ns/shacl#JSFunction> .
_:B485dc9d077951c4a981419e27a12efce <http://www.w3.org/ns/shacl#order> "0"^^<http://www.w3.org/2001/XMLSchema#integer> .
_:B28e99018c21492355cbeb7ce9c303876 <http://www.w3.org/ns/shacl#jsLibrary> <http://datashapes.org/dash#DASHJSLibrary> .
_:B2cb630d3ce6cc80fcb0af823135f42af <http://www.w3.org/ns/shacl#minCount> "1"^^<http://www.w3.org/2001/XMLSchema#integer> .
<http://datashapes.org/dash#SubSetOfConstraintComponent> <http://www.w3.org/1999/02/22-rdf-syntax-ns#type> <http://www.w3.org/ns/shacl#ConstraintComponent> .
<http://www.w3.org/ns/shacl#InConstraintComponent> <http://www.w3.org/ns/shacl#validator> <http://datashapes.org/dash#isIn> .
<http://datashapes.org/dash#HasValueWithClassConstraintComponent> <http://www.w3.org/1999/02/22-rdf-syntax-ns#type> <http://www.w3.org/ns/shacl#ConstraintComponent> .
<http://datashapes.org/dash#hasMinLength> <http://www.w3.org/ns/shacl#prefixes> <http://datashapes.org/dash> .
_:B35bf980a43fa9fd53edf3a01919e908b <http://www.w3.org/ns/shacl#message> "Value must be {$hasValue}" .
_:Bd79d8623d532452c0b9fb0617219aa16 <http://www.w3.org/ns/shacl#jsLibrary> <http://datashapes.org/dash#DASHJSLibrary> .
_:B6a3dda78c1d1372a3ae27e96a10584b5 <http://www.w3.org/ns/shacl#namespace> "http://www.w3.org/2002/07/owl#"^^<http://www.w3.org/2001/XMLSchema#anyURI> .
_:B576b207887a27c8640d054dd19740272 <http://www.w3.org/ns/shacl#prefixes> <http://datashapes.org/dash> .
_:Bb254f7a557dd3b29bbe20622d1b148be <http://www.w3.org/ns/shacl#select> "\n\t\tSELECT DISTINCT $this ?lang\n\t\tWHERE {\n\t\t\t{\n\t\t\t\tFILTER sameTerm($uniqueLang, true) .\n\t\t\t}\n\t\t\t$this $PATH ?value .\n\t\t\tBIND (lang(?value) AS ?lang) .\n\t\t\tFILTER (bound(?lang) && ?lang != \"\") .\n\t\t\tFILTER EXISTS {\n\t\t\t\t$this $PATH ?otherValue .\n\t\t\t\tFILTER (?otherValue != ?value && ?lang = lang(?otherValue)) .\n\t\t\t}\n\t\t}\n\t\t" .
_:B6df3b0d09d638883ddc7eaf55d1a9646 <http://www.w3.org/ns/shacl#description> "The graph containing the test case." .
<http://datashapes.org/dash#ClosedByTypesConstraintComponent> <http://www.w3.org/2000/01/rdf-schema#label> "Closed by types constraint component" .
<http://datashapes.org/dash#InferencingTestCase> <http://www.w3.org/1999/02/22-rdf-syntax-ns#type> <http://www.w3.org/2000/01/rdf-schema#Class> .
<http://datashapes.org/dash#shape> <http://www.w3.org/2000/01/rdf-schema#label> "shape" .
<http://datashapes.org/dash#Suggestion> <http://www.w3.org/2000/01/rdf-schema#comment> "Base class of suggestions that modify a graph to \"fix\" the source of a validation result." .
<http://datashapes.org/dash#HasValueWithClassConstraintComponent> <http://www.w3.org/2000/01/rdf-schema#comment> "A constraint component that can be used to express a constraint on property shapes so that one of the values of the property path must be an instance of a given class." .
<http://www.w3.org/ns/shacl#DisjointConstraintComponent> <http://www.w3.org/ns/shacl#validator> _:B42c37f93cbd4d4c68e68cfec1631af95 .
_:B77912faa4452655d39dee0cf876cb183 <http://www.w3.org/ns/shacl#jsLibrary> <http://datashapes.org/dash#DASHJSLibrary> .
_:Bbbfe7c69c794385222859a92b4606741 <http://www.w3.org/ns/shacl#datatype> <http://www.w3.org/1999/02/22-rdf-syntax-ns#HTML> .
<http://datashapes.org/dash#detailsEndpoint> <http://www.w3.org/2000/01/rdf-schema#label> "details endpoint" .
_:B3198ee9db9f046c7a63785bb62bb0766 <http://www.w3.org/ns/shacl#jsFunctionName> "validateHasValueProperty" .
<http://datashapes.org/dash#SuggestionResult> <http://www.w3.org/1999/02/22-rdf-syntax-ns#type> <http://www.w3.org/2000/01/rdf-schema#Class> .
_:B44ba6ca913112e299d99b54732ce1509 <http://www.w3.org/ns/shacl#select> "SELECT DISTINCT $this\nWHERE {\n        FILTER (\n\t\t\t# Must have a value for the primary key\n\t\t\tNOT EXISTS { ?this $PATH ?any }\n\t\t\t||\n\t\t\t# Must have no more than one value for the primary key\n\t\t\tEXISTS {\n\t\t\t\t?this $PATH ?value1 .\n\t\t\t\t?this $PATH ?value2 .\n\t\t\t\tFILTER (?value1 != ?value2) .\n\t\t\t}\n\t\t\t||\n\t\t\t# The value of the primary key must align with the derived URI\n\t\t\tEXISTS {\n\t\t\t\t{\n        \t\t\t?this $PATH ?value .\n\t\t\t\t\tFILTER NOT EXISTS { ?this $PATH ?value2 . FILTER (?value != ?value2) }\n\t\t\t\t}\n        \t\tBIND (CONCAT($uriStart, ENCODE_FOR_URI(str(?value))) AS ?uri) .\n        \t\tFILTER (str(?this) != ?uri) .\n    \t\t}\n\t\t)\n}" .
<http://datashapes.org/dash#AllSubjects> <http://www.w3.org/2000/01/rdf-schema#label> "All subjects" .
<http://datashapes.org/dash#QueryTestCase> <http://www.w3.org/2000/01/rdf-schema#subClassOf> <http://www.w3.org/ns/shacl#SPARQLSelectExecutable> .
<http://datashapes.org/dash#SuggestionGenerator> <http://datashapes.org/dash#abstract> "true"^^<http://www.w3.org/2001/XMLSchema#boolean> .
<http://datashapes.org/dash#QueryTestCase> <http://www.w3.org/ns/shacl#property> _:B9fe7602a489f48a08b22e99931d59d35 .
<http://datashapes.org/dash#hasMaxInclusive> <http://www.w3.org/ns/shacl#prefixes> <http://datashapes.org/dash> .
<http://datashapes.org/dash#isDeactivated> <http://www.w3.org/2000/01/rdf-schema#comment> "Checks whether a given shape or constraint has been marked as \"deactivated\" using sh:deactivated." .
<http://datashapes.org/dash#hasStem> <http://www.w3.org/1999/02/22-rdf-syntax-ns#type> <http://www.w3.org/ns/shacl#SPARQLAskValidator> .
<http://datashapes.org/dash#HTMLOrStringOrLangString> <http://www.w3.org/1999/02/22-rdf-syntax-ns#rest> _:B9f5ec4ceX2D5991X2D4a1dX2Da81aX2D237da79bf345 .
_:Bd2820cd0X2D1befX2D4fb9X2D934fX2Dd31b1666ea53 <http://www.w3.org/1999/02/22-rdf-syntax-ns#first> _:Bbd150169a34ef6489542c2938b3e8f67 .
<http://datashapes.org/dash#AllSubjectsTarget> <http://www.w3.org/1999/02/22-rdf-syntax-ns#type> <http://www.w3.org/ns/shacl#JSTargetType> .
<http://datashapes.org/dash#TestCaseResult> <http://www.w3.org/ns/shacl#property> _:B12898dca29ca363f5ae4b1b4c90c363b .
<http://datashapes.org/dash#PrimaryKeyConstraintComponent> <http://www.w3.org/2000/01/rdf-schema#label> "Primary key constraint component" .
<http://datashapes.org/dash#rootClass> <http://www.w3.org/2000/01/rdf-schema#label> "root class" .
_:Bed3045d9aeb8442f56a5b5a092925fd8 <http://www.w3.org/ns/shacl#jsFunctionName> "validateClosed" .
<http://datashapes.org/dash#SPARQLSelectTemplate> <http://www.w3.org/2000/01/rdf-schema#label> "SPARQL SELECT template" .
<http://datashapes.org/dash#NonRecursiveConstraintComponent-nonRecursive> <http://www.w3.org/ns/shacl#name> "non-recursive" .
<http://datashapes.org/dash#hasPattern> <http://www.w3.org/ns/shacl#ask> "ASK { FILTER (!isBlank($value) && IF(bound($flags), regex(str($value), $pattern, $flags), regex(str($value), $pattern))) }" .
<http://datashapes.org/dash#DateOrDateTime> <http://www.w3.org/1999/02/22-rdf-syntax-ns#rest> _:B51e81f8eX2Dded0X2D4b0bX2D97bbX2Dea24608138ee .
<http://datashapes.org/dash#SuccessResult> <http://www.w3.org/1999/02/22-rdf-syntax-ns#type> <http://www.w3.org/2000/01/rdf-schema#Class> .
<http://datashapes.org/dash#AllObjects> <http://www.w3.org/2000/01/rdf-schema#comment> "A reusable instance of dash:AllObjectsTarget." .
_:Bd79d8623d532452c0b9fb0617219aa16 <http://www.w3.org/1999/02/22-rdf-syntax-ns#type> <http://www.w3.org/ns/shacl#JSValidator> .
<http://datashapes.org/dash#validateShapes> <http://www.w3.org/2000/01/rdf-schema#domain> <http://datashapes.org/dash#GraphValidationTestCase> .
<http://datashapes.org/dash#toString> <http://www.w3.org/ns/shacl#jsLibrary> <http://datashapes.org/dash#DASHJSLibrary> .
<http://datashapes.org/dash#ClosedByTypesConstraintComponent> <http://www.w3.org/ns/shacl#nodeValidator> _:B324a4eda45fae1908023e86a8b10dbdb .
<http://datashapes.org/dash#expectedResultIsJSON> <http://www.w3.org/2000/01/rdf-schema#range> <http://www.w3.org/2001/XMLSchema#boolean> .
<http://datashapes.org/dash#SuggestionResult> <http://www.w3.org/2000/01/rdf-schema#label> "Suggestion result" .
<http://datashapes.org/dash#DetailsViewer> <http://www.w3.org/2000/01/rdf-schema#label> "Details Viewer" .
_:B2a3499b11e685d3ad17286d18e230c41 <http://www.w3.org/ns/shacl#jsFunctionName> "validateClass" .
<http://datashapes.org/dash#RootClassConstraintComponent-rootClass> <http://www.w3.org/1999/02/22-rdf-syntax-ns#type> <http://www.w3.org/ns/shacl#Parameter> .
<http://datashapes.org/dash#isNodeKindBlankNode> <http://www.w3.org/2000/01/rdf-schema#comment> "Checks if a given sh:NodeKind is one that includes BlankNodes." .
<http://www.w3.org/ns/shacl#NodeConstraintComponent> <http://www.w3.org/ns/shacl#targetClass> <http://www.w3.org/ns/shacl#Shape> .
_:B28e99018c21492355cbeb7ce9c303876 <http://www.w3.org/1999/02/22-rdf-syntax-ns#type> <http://www.w3.org/ns/shacl#JSValidator> .
_:Bbc6a3e0006c01fd1021e9a87d62d127a <http://www.w3.org/ns/shacl#datatype> <http://www.w3.org/2001/XMLSchema#anyURI> .
<http://datashapes.org/dash#URIViewer> <http://www.w3.org/1999/02/22-rdf-syntax-ns#type> <http://datashapes.org/dash#Viewer> .
<http://datashapes.org/dash#ClosedByTypesConstraintComponent> <http://www.w3.org/ns/shacl#targetClass> <http://www.w3.org/ns/shacl#NodeShape> .
<http://datashapes.org/dash#StemConstraintComponent-stem> <http://www.w3.org/ns/shacl#datatype> <http://www.w3.org/2001/XMLSchema#string> .
<http://datashapes.org/dash#Viewer> <http://www.w3.org/2000/01/rdf-schema#comment> "The class of widgets for viewing value nodes." .
<http://datashapes.org/dash#BlankNodeViewer> <http://www.w3.org/2000/01/rdf-schema#comment> "A Viewer for blank nodes, rendering as the label of the blank node." .
_:Bfe0a112f2951265152c632d9a5c70c7a <http://www.w3.org/1999/02/22-rdf-syntax-ns#type> <http://www.w3.org/ns/shacl#SPARQLSelectValidator> .
<http://datashapes.org/dash#hasPattern> <http://www.w3.org/2000/01/rdf-schema#comment> "Checks whether the string representation of a given node (?value) matches a given regular expression (?pattern). Returns false if the value is a blank node." .
_:Bef4b4e661cf3b607381181797fae49a3 <http://www.w3.org/ns/shacl#name> "node kind" .
<http://datashapes.org/dash#RootClassConstraintComponent> <http://www.w3.org/ns/shacl#validator> <http://datashapes.org/dash#hasRootClass> .
_:B9fe7602a489f48a08b22e99931d59d35 <http://www.w3.org/1999/02/22-rdf-syntax-ns#type> <http://www.w3.org/ns/shacl#PropertyShape> .
<http://datashapes.org/dash#LabelViewer> <http://www.w3.org/2000/01/rdf-schema#label> "Label Viewer" .
_:Baca6b78cb251a419ee913fa362fa0fad <http://www.w3.org/ns/shacl#message> "Value {?value} must be unique but is also used by {?other}" .
<http://datashapes.org/dash#Suggestion> <http://www.w3.org/2000/01/rdf-schema#subClassOf> <http://www.w3.org/2000/01/rdf-schema#Resource> .
_:B77912faa4452655d39dee0cf876cb183 <http://www.w3.org/1999/02/22-rdf-syntax-ns#type> <http://www.w3.org/ns/shacl#JSValidator> .
<http://datashapes.org/dash#SuccessResult> <http://www.w3.org/2000/01/rdf-schema#comment> "A result representing a successfully validated constraint." .
<http://datashapes.org/dash#AllObjectsTarget> <http://www.w3.org/ns/shacl#labelTemplate> "All objects" .
<http://datashapes.org/dash#RootClassConstraintComponent-rootClass> <http://www.w3.org/ns/shacl#class> <http://www.w3.org/2000/01/rdf-schema#Class> .
<http://datashapes.org/dash#ValidationTestCase> <http://www.w3.org/2000/01/rdf-schema#comment> "Abstract superclass for test cases concerning SHACL constraint validation. Future versions may add new kinds of validatin test cases, e.g. to validate a single resource only." .
<http://datashapes.org/dash#LiteralViewer> <http://www.w3.org/1999/02/22-rdf-syntax-ns#type> <http://datashapes.org/dash#Viewer> .
<http://datashapes.org/dash#Viewer> <http://www.w3.org/2000/01/rdf-schema#label> "Viewer" .
_:Bef4b4e661cf3b607381181797fae49a3 <http://www.w3.org/ns/shacl#path> <http://datashapes.org/dash#nodeKind> .
<http://datashapes.org/dash#isLanguageIn> <http://www.w3.org/2000/01/rdf-schema#label> "is language in" .
<http://datashapes.org/dash#isNodeKindIRI> <http://www.w3.org/ns/shacl#parameter> _:B31473064d8bd1e288bd70b63b0f116a3 .
_:B6df3b0d09d638883ddc7eaf55d1a9646 <http://www.w3.org/ns/shacl#minCount> "1"^^<http://www.w3.org/2001/XMLSchema#integer> .
<http://datashapes.org/dash#detailsGraph> <http://www.w3.org/1999/02/22-rdf-syntax-ns#type> <http://www.w3.org/1999/02/22-rdf-syntax-ns#Property> .
<http://datashapes.org/dash#ListNodeShape> <http://www.w3.org/2000/01/rdf-schema#comment> "Defines constraints on what it means for a node to be a node within a well-formed RDF list. Note that this does not check whether the rdf:rest items are also well-formed lists as this would lead to unsupported recursion." .
<http://datashapes.org/dash#reifiableBy> <http://www.w3.org/1999/02/22-rdf-syntax-ns#type> <http://www.w3.org/1999/02/22-rdf-syntax-ns#Property> .
<http://www.w3.org/ns/shacl#EqualsConstraintComponent> <http://www.w3.org/ns/shacl#propertyValidator> _:Bb880e354f894466d96da68ac6732829f .
<http://www.w3.org/ns/shacl#MinCountConstraintComponent> <http://www.w3.org/ns/shacl#message> "Fewer than {$minCount} values" .
<http://datashapes.org/dash#expectedResult> <http://www.w3.org/2000/01/rdf-schema#label> "expected result" .
_:Baca6b78cb251a419ee913fa362fa0fad <http://www.w3.org/ns/shacl#jsFunctionName> "validateUniqueValueForClass" .
<http://datashapes.org/dash#ExecutionPlatform> <http://www.w3.org/2000/01/rdf-schema#comment> "An platform (such as TopBraid) that may have features needed to execute, for example, SPARQL queries." .
<http://datashapes.org/dash#SingleLineConstraintComponent> <http://www.w3.org/ns/shacl#message> "Must not contain line breaks." .
<http://datashapes.org/dash#SuccessTestCaseResult> <http://www.w3.org/2000/01/rdf-schema#comment> "Represents a successful run of a test case." .
<http://datashapes.org/dash#localConstraint> <http://www.w3.org/2000/01/rdf-schema#domain> <http://www.w3.org/ns/shacl#ConstraintComponent> .
_:B8791b3a24b8675de3fe6cea3980f416f <http://www.w3.org/1999/02/22-rdf-syntax-ns#type> <http://www.w3.org/ns/shacl#SPARQLAskValidator> .
_:B51e81f8eX2Dded0X2D4b0bX2D97bbX2Dea24608138ee <http://www.w3.org/1999/02/22-rdf-syntax-ns#first> _:Bfb96260a3d1be1805270339a2809aef8 .
<http://datashapes.org/dash#RootClassConstraintComponent-rootClass> <http://www.w3.org/ns/shacl#name> "root class" .
<http://datashapes.org/dash#shape> <http://www.w3.org/1999/02/22-rdf-syntax-ns#type> <http://www.w3.org/1999/02/22-rdf-syntax-ns#Property> .
<http://datashapes.org/dash#RichTextEditor> <http://www.w3.org/2000/01/rdf-schema#comment> "A rich text editor to enter the lexical value of a literal and a drop down to select language. The selected language is stored in the HTML lang attribute of the root node in the HTML DOM tree." .
<http://datashapes.org/dash#hasValueWithClass> <http://www.w3.org/2000/01/rdf-schema#comment> "Specifies a constraint that at least one of the value nodes must be an instance of a given class." .
<http://www.w3.org/ns/shacl#EqualsConstraintComponent> <http://datashapes.org/dash#localConstraint> "true"^^<http://www.w3.org/2001/XMLSchema#boolean> .
<http://datashapes.org/dash#NonRecursiveConstraintComponent> <http://www.w3.org/ns/shacl#message> "Points back at itself (recursively)" .
<http://datashapes.org/dash#TextAreaEditor> <http://www.w3.org/2000/01/rdf-schema#comment> "A multi-line text area to enter the value of a literal." .
_:B40fc13c18bcea97b695cedc8f377811f <http://www.w3.org/ns/shacl#description> "The sh:NodeKind to check." .
<http://datashapes.org/dash#ParameterConstraintComponent-parameter> <http://www.w3.org/ns/shacl#path> <http://www.w3.org/ns/shacl#parameter> .
<http://datashapes.org/dash#uniqueValueForClass> <http://www.w3.org/1999/02/22-rdf-syntax-ns#type> <http://www.w3.org/1999/02/22-rdf-syntax-ns#Property> .
<http://datashapes.org/dash#RootClassConstraintComponent-rootClass> <http://www.w3.org/ns/shacl#nodeKind> <http://www.w3.org/ns/shacl#IRI> .
_:Bc91acb30da815118fca913844f6cfa7b <http://www.w3.org/ns/shacl#jsFunctionName> "validateSingleLine" .
_:B4d5234299127eb5252bb141a36ca256e <http://www.w3.org/ns/shacl#datatype> <http://www.w3.org/1999/02/22-rdf-syntax-ns#langString> .
<http://datashapes.org/dash#TextFieldEditor> <http://www.w3.org/2000/01/rdf-schema#comment> "A simple input field to enter the value of a literal, without the ability to change language or datatype.\n\nThis is the fallback editor for any literal if no other editors are more suitable." .
<http://datashapes.org/dash#height> <http://www.w3.org/2000/01/rdf-schema#label> "height" .
<http://www.w3.org/ns/shacl#MaxExclusiveConstraintComponent> <http://datashapes.org/dash#staticConstraint> "true"^^<http://www.w3.org/2001/XMLSchema#boolean> .
<http://www.w3.org/ns/shacl#LessThanOrEqualsConstraintComponent> <http://www.w3.org/ns/shacl#propertyValidator> _:Bfe0a112f2951265152c632d9a5c70c7a .
<http://datashapes.org/dash#ParameterConstraintComponent> <http://www.w3.org/2000/01/rdf-schema#comment> "A constraint component that can be used to verify that all value nodes conform to the given Parameter."@en .
<http://datashapes.org/dash#SPARQLUpdateSuggestionGenerator> <http://www.w3.org/1999/02/22-rdf-syntax-ns#type> <http://www.w3.org/2000/01/rdf-schema#Class> .
_:B0c0f328c69e13d06674f58bb5b4a9284 <http://www.w3.org/1999/02/22-rdf-syntax-ns#type> <http://www.w3.org/ns/shacl#Parameter> .
<http://datashapes.org/dash#suggestion> <http://www.w3.org/2000/01/rdf-schema#label> "suggestion" .
<http://datashapes.org/dash#CoExistsWithConstraintComponent-coExistsWith> <http://www.w3.org/ns/shacl#class> <http://www.w3.org/1999/02/22-rdf-syntax-ns#Property> .
<http://datashapes.org/dash#None> <http://www.w3.org/2000/01/rdf-schema#label> "None" .
<http://datashapes.org/dash#QueryTestCase> <http://www.w3.org/2000/01/rdf-schema#comment> "A test case running a given SPARQL SELECT query and comparing its results with those stored as JSON Result Set in the expected result property." .
<http://datashapes.org/dash#hasMinLength> <http://www.w3.org/2000/01/rdf-schema#comment> "Checks whether a given string (?value) has a length within a given minimum string length." .
<http://datashapes.org/dash#propertySuggestionGenerator> <http://www.w3.org/1999/02/22-rdf-syntax-ns#type> <http://www.w3.org/1999/02/22-rdf-syntax-ns#Property> .
<http://www.w3.org/ns/shacl#LanguageInConstraintComponent> <http://www.w3.org/ns/shacl#labelTemplate> "Language must match any of {$languageIn}" .
<http://www.w3.org/ns/shacl#PatternConstraintComponent> <http://datashapes.org/dash#staticConstraint> "true"^^<http://www.w3.org/2001/XMLSchema#boolean> .
_:B485dc9d077951c4a981419e27a12efce <http://www.w3.org/ns/shacl#path> <http://datashapes.org/dash#subject> .
<http://datashapes.org/dash#width> <http://www.w3.org/2000/01/rdf-schema#comment> "The width." .
<http://datashapes.org/dash#AllSubjectsTarget> <http://www.w3.org/ns/shacl#labelTemplate> "All subjects" .
<http://www.w3.org/ns/shacl#UniqueLangConstraintComponent> <http://datashapes.org/dash#localConstraint> "true"^^<http://www.w3.org/2001/XMLSchema#boolean> .
<http://datashapes.org/dash#RootClassConstraintComponent> <http://www.w3.org/ns/shacl#labelTemplate> "Root class {$rootClass}" .
<http://datashapes.org/dash#NonRecursiveConstraintComponent-nonRecursive> <http://www.w3.org/ns/shacl#datatype> <http://www.w3.org/2001/XMLSchema#boolean> .
<http://datashapes.org/dash#TestEnvironment> <http://www.w3.org/2000/01/rdf-schema#comment> "Abstract base class for test environments, holding information on how to set up a test case." .
<http://datashapes.org/dash#ListShape> <http://www.w3.org/ns/shacl#property> _:Be48162e9c0f86045a8d1a3b5697cfc8b .
<http://datashapes.org/dash#SubSetOfConstraintComponent> <http://datashapes.org/dash#localConstraint> "true"^^<http://www.w3.org/2001/XMLSchema#boolean> .
<http://datashapes.org/dash#Editor> <http://www.w3.org/2000/01/rdf-schema#subClassOf> <http://datashapes.org/dash#Widget> .
<http://datashapes.org/dash#PrimaryKeyConstraintComponent> <http://www.w3.org/ns/shacl#propertyValidator> _:B44ba6ca913112e299d99b54732ce1509 .
_:B6d4cbc3d992ff864f2dac864d1480fb8 <http://www.w3.org/ns/shacl#description> "The expected RDF graph, as a Turtle string." .
<http://datashapes.org/dash#ReifiableByConstraintComponent-reifiableBy> <http://www.w3.org/ns/shacl#path> <http://datashapes.org/dash#reifiableBy> .
<http://datashapes.org/dash#SubSetOfConstraintComponent-subSetOf> <http://www.w3.org/1999/02/22-rdf-syntax-ns#type> <http://www.w3.org/ns/shacl#Parameter> .
_:B6431ca200460b7f86c096adcb4867b07 <http://www.w3.org/ns/shacl#class> <http://www.w3.org/ns/shacl#ValidationReport> .
<http://datashapes.org/dash#SymmetricConstraintComponent-symmetric> <http://www.w3.org/ns/shacl#datatype> <http://www.w3.org/2001/XMLSchema#boolean> .
_:B40fc13c18bcea97b695cedc8f377811f <http://www.w3.org/ns/shacl#path> <http://datashapes.org/dash#nodeKind> .
<http://datashapes.org/dash#EnumSelectEditor> <http://www.w3.org/1999/02/22-rdf-syntax-ns#type> <http://datashapes.org/dash#Editor> .
<http://www.w3.org/ns/shacl#QualifiedMinCountConstraintComponent> <http://www.w3.org/ns/shacl#propertyValidator> _:B9f8708a030e28285db3efcfa7150f80b .
_:B8d319a0761f1abba217993df30ee7b93 <http://www.w3.org/ns/shacl#namespace> "http://www.w3.org/2004/02/skos/core#"^^<http://www.w3.org/2001/XMLSchema#anyURI> .
<http://datashapes.org/dash#Widget> <http://www.w3.org/1999/02/22-rdf-syntax-ns#type> <http://www.w3.org/ns/shacl#NodeShape> .
<http://www.w3.org/ns/shacl#NodeConstraintComponent> <http://www.w3.org/ns/shacl#message> "Value does not have shape {$node}" .
<http://datashapes.org/dash#PrimaryKeyConstraintComponent-uriStart> <http://www.w3.org/ns/shacl#description> "The start of the URIs of well-formed resources. If specified then the associated property/path serves as \"primary key\" for all target nodes (instances). All such target nodes need to have a URI that starts with the given string, followed by the URI-encoded value of the primary key property." .
_:B40fc13c18bcea97b695cedc8f377811f <http://www.w3.org/ns/shacl#name> "node kind" .
<http://datashapes.org/dash#ListNodeShape> <http://www.w3.org/1999/02/22-rdf-syntax-ns#type> <http://www.w3.org/ns/shacl#NodeShape> .
<http://datashapes.org/dash#expectedResultIsJSON> <http://www.w3.org/2000/01/rdf-schema#comment> "A flag to indicate that the expected result represents a JSON string. If set to true, then tests would compare JSON structures (regardless of whitespaces) instead of actual syntax." .
_:B21421ade4ccc7092969f52bbcc0d7484 <http://www.w3.org/ns/shacl#jsLibrary> <http://datashapes.org/dash#DASHJSLibrary> .
_:B13da662fb0d609b0fa8798a656baca2d <http://www.w3.org/1999/02/22-rdf-syntax-ns#type> <http://www.w3.org/ns/shacl#JSValidator> .
<http://datashapes.org/dash#HasValueWithClassConstraintComponent> <http://www.w3.org/ns/shacl#parameter> <http://datashapes.org/dash#HasValueWithClassConstraintComponent-hasValueWithClass> .
<http://www.w3.org/2002/07/owl#Class> <http://www.w3.org/2000/01/rdf-schema#subClassOf> <http://www.w3.org/2000/01/rdf-schema#Class> .
<http://www.w3.org/ns/shacl#MaxInclusiveConstraintComponent> <http://www.w3.org/ns/shacl#validator> _:B28e99018c21492355cbeb7ce9c303876 .
<http://datashapes.org/dash#testEnvironment> <http://www.w3.org/2000/01/rdf-schema#label> "test environment" .
<http://www.w3.org/ns/shacl#QualifiedMaxCountConstraintComponent> <http://www.w3.org/ns/shacl#targetClass> <http://www.w3.org/ns/shacl#PropertyShape> .
<http://datashapes.org/dash#PrimaryKeyConstraintComponent> <http://www.w3.org/ns/shacl#targetClass> <http://www.w3.org/ns/shacl#PropertyShape> .
_:B6431ca200460b7f86c096adcb4867b07 <http://www.w3.org/ns/shacl#name> "expected result" .
_:B8a6d95446c24ef2a1314f1cfdc6ea805 <http://www.w3.org/ns/shacl#prefixes> <http://datashapes.org/dash> .
<http://datashapes.org/dash> <http://www.w3.org/ns/shacl#declare> _:B54c36a3353a36f7de1eb49377ffde112 .
_:B2a3499b11e685d3ad17286d18e230c41 <http://www.w3.org/ns/shacl#jsLibrary> <http://datashapes.org/dash#DASHJSLibrary> .
<http://www.w3.org/ns/shacl#LessThanConstraintComponent> <http://www.w3.org/ns/shacl#targetClass> <http://www.w3.org/ns/shacl#PropertyShape> .
<http://datashapes.org/dash> <http://www.w3.org/ns/shacl#declare> _:B8d319a0761f1abba217993df30ee7b93 .
_:B80b7e2f9fc1f404e1d9d214172e0e1b3 <http://www.w3.org/ns/shacl#prefixes> <http://datashapes.org/dash> .
_:B8911ff43e060d96ba77f70561fffd26e <http://www.w3.org/ns/shacl#jsFunctionName> "validateNonRecursiveProperty" .
_:Bf87fbb2c21e07adfb80e0445145d23a6 <http://www.w3.org/1999/02/22-rdf-syntax-ns#type> <http://www.w3.org/ns/shacl#JSValidator> .
<http://datashapes.org/dash#valueCount> <http://www.w3.org/ns/shacl#select> "\n\t\tSELECT (COUNT(?object) AS ?result)\n\t\tWHERE {\n    \t\t$subject $predicate ?object .\n\t\t}\n" .
<http://datashapes.org/dash#AllSubjects> <http://www.w3.org/2000/01/rdf-schema#comment> "A reusable instance of dash:AllSubjectsTarget." .
<http://www.w3.org/ns/shacl#DatatypeConstraintComponent> <http://www.w3.org/ns/shacl#message> "Value does not have datatype {$datatype}" .
<http://www.w3.org/ns/shacl#Rules> <http://www.w3.org/2000/01/rdf-schema#comment> "The SHACL rules entailment regime." .
<http://www.w3.org/ns/shacl#UniqueLangConstraintComponent> <http://www.w3.org/ns/shacl#labelTemplate> "No language can be used more than once" .
_:Bed3045d9aeb8442f56a5b5a092925fd8 <http://www.w3.org/ns/shacl#jsLibrary> <http://datashapes.org/dash#DASHJSLibrary> .
<http://datashapes.org/dash#hasValueWithClass> <http://www.w3.org/2000/01/rdf-schema#label> "has value with class" .
<http://www.w3.org/ns/shacl#Validator> <http://datashapes.org/dash#abstract> "true"^^<http://www.w3.org/2001/XMLSchema#boolean> .
<http://datashapes.org/dash#FailureResult> <http://www.w3.org/1999/02/22-rdf-syntax-ns#type> <http://www.w3.org/2000/01/rdf-schema#Class> .
_:Ba7e7c348f2c50eb0f8f5b0beb9fb6862 <http://www.w3.org/1999/02/22-rdf-syntax-ns#type> <http://www.w3.org/ns/shacl#JSValidator> .
<http://datashapes.org/dash#isNodeKindBlankNode> <http://www.w3.org/1999/02/22-rdf-syntax-ns#type> <http://www.w3.org/ns/shacl#SPARQLFunction> .
<http://datashapes.org/dash#AllSubjectsTarget> <http://www.w3.org/ns/shacl#jsFunctionName> "dash_allSubjects" .
_:B5672337cd6b085d4efa2003d67fc0562 <http://www.w3.org/ns/shacl#description> "The predicate to get the number of objects of." .
<http://datashapes.org/dash#isNodeKindIRI> <http://www.w3.org/2000/01/rdf-schema#comment> "Checks if a given sh:NodeKind is one that includes IRIs." .
<http://www.w3.org/ns/shacl#DisjointConstraintComponent> <http://www.w3.org/ns/shacl#targetClass> <http://www.w3.org/ns/shacl#Shape> .
<http://datashapes.org/dash#DefaultValueTypeRule> <http://www.w3.org/2000/01/rdf-schema#label> "default value type inference rule" .
_:Be48162e9c0f86045a8d1a3b5697cfc8b <http://www.w3.org/2000/01/rdf-schema#comment> "Each list member (including this node) must be have the shape dash:ListNodeShape." .
<http://datashapes.org/dash#None> <http://www.w3.org/ns/shacl#in> <http://www.w3.org/1999/02/22-rdf-syntax-ns#nil> .
<http://datashapes.org/dash#hasMaxInclusive> <http://www.w3.org/2000/01/rdf-schema#label> "has max inclusive" .
<http://datashapes.org/dash#hasMaxLength> <http://www.w3.org/2000/01/rdf-schema#comment> "Checks whether a given string (?value) has a length within a given maximum string length." .
<http://www.w3.org/ns/shacl#MinCountConstraintComponent> <http://www.w3.org/ns/shacl#propertyValidator> _:B881d49f14342613394c38418a3e2b26e .
<http://datashapes.org/dash#isNodeKindLiteral> <http://www.w3.org/ns/shacl#prefixes> <http://datashapes.org/dash> .
<http://datashapes.org/dash#ExecutionPlatform> <http://www.w3.org/2000/01/rdf-schema#subClassOf> <http://www.w3.org/2000/01/rdf-schema#Resource> .
<http://datashapes.org/dash#suggestionConfidence> <http://www.w3.org/2000/01/rdf-schema#label> "suggestion confidence" .
_:B54c36a3353a36f7de1eb49377ffde112 <http://www.w3.org/ns/shacl#namespace> "http://www.w3.org/2000/01/rdf-schema#"^^<http://www.w3.org/2001/XMLSchema#anyURI> .
<http://datashapes.org/dash#BooleanSelectEditor> <http://www.w3.org/2000/01/rdf-schema#comment> "An editor for boolean literals, rendering as a select box with values true and false.\n\nAlso displays the current value (such as \"1\"^^xsd:boolean), but only allows to switch to true or false." .
<http://datashapes.org/dash#NonRecursiveConstraintComponent> <http://www.w3.org/2000/01/rdf-schema#label> "Non-recursive constraint component" .
<http://www.w3.org/ns/shacl#LessThanOrEqualsConstraintComponent> <http://datashapes.org/dash#localConstraint> "true"^^<http://www.w3.org/2001/XMLSchema#boolean> .
<http://datashapes.org/dash#hasValueWithClass> <http://www.w3.org/2000/01/rdf-schema#range> <http://www.w3.org/2000/01/rdf-schema#Class> .
_:Bef4b4e661cf3b607381181797fae49a3 <http://www.w3.org/ns/shacl#description> "The sh:NodeKind to check." .
_:B850a3561a7b96169d0a48349ceccf59d <http://www.w3.org/ns/shacl#jsLibrary> <http://datashapes.org/dash#DASHJSLibrary> .
<http://www.w3.org/ns/shacl#PatternConstraintComponent> <http://www.w3.org/ns/shacl#validator> _:B13da662fb0d609b0fa8798a656baca2d .
_:B1f243cca064dc36a3759b064b48d1d3d <http://www.w3.org/ns/shacl#jsLibrary> <http://datashapes.org/dash#DASHJSLibrary> .
_:Bff9ecbe5a61b70becac46f6b4ddfdb03 <http://www.w3.org/ns/shacl#path> <http://www.w3.org/1999/02/22-rdf-syntax-ns#rest> .
<http://datashapes.org/dash#SPARQLConstructTemplate> <http://www.w3.org/2000/01/rdf-schema#comment> "Encapsulates one or more SPARQL CONSTRUCT queries that can be parameterized. Parameters will become pre-bound variables in the queries." .
<http://datashapes.org/dash#SymmetricConstraintComponent> <http://www.w3.org/ns/shacl#propertyValidator> _:B192ffa056ee292f9513e19adb943a589 .
<http://datashapes.org/dash#StemConstraintComponent> <http://www.w3.org/1999/02/22-rdf-syntax-ns#type> <http://www.w3.org/ns/shacl#ConstraintComponent> .
<http://datashapes.org/dash#composite> <http://www.w3.org/1999/02/22-rdf-syntax-ns#type> <http://www.w3.org/1999/02/22-rdf-syntax-ns#Property> .
_:Bbc6a3e0006c01fd1021e9a87d62d127a <http://www.w3.org/ns/shacl#maxCount> "1"^^<http://www.w3.org/2001/XMLSchema#integer> .
<http://datashapes.org/dash#hasMinExclusive> <http://www.w3.org/2000/01/rdf-schema#comment> "Checks whether a given node (?value) has value greater than (>) the provided ?minExclusive. Returns false if this cannot be determined, e.g. because values do not have comparable types." .
<http://datashapes.org/dash#hasMaxLength> <http://www.w3.org/ns/shacl#ask> "\n\t\tASK {\n\t\t\tFILTER (STRLEN(str($value)) <= $maxLength) .\n\t\t}\n\t\t" .
<http://datashapes.org/dash#None> <http://www.w3.org/1999/02/22-rdf-syntax-ns#type> <http://www.w3.org/ns/shacl#NodeShape> .
<http://datashapes.org/dash#TestCaseResult> <http://datashapes.org/dash#abstract> "true"^^<http://www.w3.org/2001/XMLSchema#boolean> .
<http://datashapes.org/dash#hasMaxInclusive> <http://www.w3.org/2000/01/rdf-schema#comment> "Checks whether a given node (?value) has a value less than or equal to (<=) the provided ?maxInclusive. Returns false if this cannot be determined, e.g. because values do not have comparable types." .
<http://datashapes.org/dash#singleLine> <http://www.w3.org/2000/01/rdf-schema#label> "single line" .
<http://datashapes.org/dash#ValueTableViewer> <http://www.w3.org/2000/01/rdf-schema#label> "Value table viewer" .
<http://datashapes.org/dash#HTMLViewer> <http://www.w3.org/2000/01/rdf-schema#label> "HTML Viewer" .
<http://www.w3.org/ns/shacl#DatatypeConstraintComponent> <http://datashapes.org/dash#staticConstraint> "true"^^<http://www.w3.org/2001/XMLSchema#boolean> .
_:Be4b7da0362b43f04fa717e3e11887a9e <http://www.w3.org/ns/shacl#prefixes> <http://datashapes.org/dash> .
_:B6df3b0d09d638883ddc7eaf55d1a9646 <http://www.w3.org/ns/shacl#nodeKind> <http://www.w3.org/ns/shacl#IRI> .
<http://datashapes.org/dash#hasRootClass> <http://www.w3.org/1999/02/22-rdf-syntax-ns#type> <http://www.w3.org/ns/shacl#SPARQLAskValidator> .
<http://datashapes.org/dash#suggestionGenerator> <http://www.w3.org/2000/01/rdf-schema#range> <http://datashapes.org/dash#SuggestionGenerator> .
<http://datashapes.org/dash#GraphStoreTestCase> <http://www.w3.org/1999/02/22-rdf-syntax-ns#type> <http://www.w3.org/ns/shacl#NodeShape> .
<http://datashapes.org/dash#DatePickerEditor> <http://www.w3.org/1999/02/22-rdf-syntax-ns#type> <http://datashapes.org/dash#Editor> .
<http://datashapes.org/dash#DateOrDateTime> <http://www.w3.org/2000/01/rdf-schema#comment> "An rdf:List that can be used in property constraints as value for sh:or to indicate that all values of a property must be either xsd:date or xsd:dateTime." .
<http://www.w3.org/ns/shacl#ClosedConstraintComponent> <http://www.w3.org/ns/shacl#targetClass> <http://www.w3.org/ns/shacl#NodeShape> .
_:Bd048027623bcc6288ff18f5d0dfbb126 <http://www.w3.org/ns/shacl#prefixes> <http://datashapes.org/dash> .
<http://datashapes.org/dash#ListShape> <http://www.w3.org/2000/01/rdf-schema#label> "List shape" .
<http://datashapes.org/dash#hidden> <http://www.w3.org/2000/01/rdf-schema#label> "hidden" .
<http://datashapes.org/dash#Editor> <http://www.w3.org/2000/01/rdf-schema#comment> "The class of widgets for editing value nodes." .
_:B9f8708a030e28285db3efcfa7150f80b <http://www.w3.org/ns/shacl#jsFunctionName> "validateQualifiedMinCountProperty" .
<http://datashapes.org/dash#HyperlinkViewer> <http://www.w3.org/2000/01/rdf-schema#label> "Hyperlink Viewer" .
<http://datashapes.org/dash#BlankNodeViewer> <http://www.w3.org/1999/02/22-rdf-syntax-ns#type> <http://datashapes.org/dash#Viewer> .
<http://datashapes.org/dash> <http://www.w3.org/2002/07/owl#imports> <http://www.w3.org/ns/shacl#> .
<http://datashapes.org/dash#StemConstraintComponent> <http://www.w3.org/ns/shacl#labelTemplate> "Value needs to have stem {$stem}" .
<http://datashapes.org/dash#abstract> <http://www.w3.org/1999/02/22-rdf-syntax-ns#type> <http://www.w3.org/1999/02/22-rdf-syntax-ns#Property> .
<http://datashapes.org/dash#Suggestion> <http://www.w3.org/2000/01/rdf-schema#label> "Suggestion" .
_:B850a3561a7b96169d0a48349ceccf59d <http://www.w3.org/1999/02/22-rdf-syntax-ns#type> <http://www.w3.org/ns/shacl#JSValidator> .
<http://datashapes.org/dash#AllObjects> <http://www.w3.org/2000/01/rdf-schema#label> "All objects" .
<http://datashapes.org/dash#hasMinInclusive> <http://www.w3.org/2000/01/rdf-schema#label> "has min inclusive" .
<http://datashapes.org/dash#CoExistsWithConstraintComponent-coExistsWith> <http://www.w3.org/ns/shacl#path> <http://datashapes.org/dash#coExistsWith> .
<http://datashapes.org/dash#hasMaxExclusive> <http://www.w3.org/ns/shacl#ask> "ASK { FILTER ($value < $maxExclusive) }" .
<http://datashapes.org/dash#TextFieldWithLangEditor> <http://www.w3.org/1999/02/22-rdf-syntax-ns#type> <http://datashapes.org/dash#Editor> .
_:B1f243cca064dc36a3759b064b48d1d3d <http://www.w3.org/1999/02/22-rdf-syntax-ns#type> <http://www.w3.org/ns/shacl#JSValidator> .
<http://datashapes.org/dash#staticConstraint> <http://www.w3.org/2000/01/rdf-schema#range> <http://www.w3.org/2001/XMLSchema#boolean> .
<http://datashapes.org/dash#EnumSelectEditor> <http://www.w3.org/2000/01/rdf-schema#label> "Enum select editor" .
<http://datashapes.org/dash#deletedTriple> <http://www.w3.org/2000/01/rdf-schema#comment> "May link a dash:GraphUpdate result with one or more triples (represented as instances of rdf:Statement) that should be deleted to fix the source of the result." .
<http://datashapes.org/dash#height> <http://www.w3.org/2000/01/rdf-schema#range> <http://www.w3.org/2001/XMLSchema#integer> .
_:B555c69d616b27a2b4c8744e4327dadf9 <http://www.w3.org/1999/02/22-rdf-syntax-ns#type> <http://www.w3.org/ns/shacl#SPARQLSelectValidator> .
<http://www.w3.org/ns/shacl#NotConstraintComponent> <http://www.w3.org/ns/shacl#labelTemplate> "Value must not have shape {$not}" .
<http://datashapes.org/dash#AllObjectsTarget> <http://www.w3.org/1999/02/22-rdf-syntax-ns#type> <http://www.w3.org/ns/shacl#SPARQLTargetType> .
<http://datashapes.org/dash#expectedResultIsTTL> <http://www.w3.org/1999/02/22-rdf-syntax-ns#type> <http://www.w3.org/1999/02/22-rdf-syntax-ns#Property> .
_:Ba94bb54840f7b2f2def8b93e306cd9bf <http://www.w3.org/ns/shacl#name> "deactivated" .
<http://datashapes.org/dash#isNodeKindIRI> <http://www.w3.org/ns/shacl#ask> "ASK {\n\tFILTER ($nodeKind IN ( sh:IRI, sh:BlankNodeOrIRI, sh:IRIOrLiteral ))\n}" .
<http://datashapes.org/dash#HasValueWithClassConstraintComponent-hasValueWithClass> <http://www.w3.org/ns/shacl#path> <http://datashapes.org/dash#hasValueWithClass> .
<http://datashapes.org/dash#SubSetOfConstraintComponent> <http://www.w3.org/2000/01/rdf-schema#label> "Sub set of constraint component" .
<http://datashapes.org/dash#width> <http://www.w3.org/1999/02/22-rdf-syntax-ns#type> <http://www.w3.org/1999/02/22-rdf-syntax-ns#Property> .
<http://datashapes.org/dash#InferencingTestCase> <http://www.w3.org/2000/01/rdf-schema#label> "Inferencing test case" .
_:B978525ea2f32d0660c9ffc71e8b5d4cd <http://www.w3.org/ns/shacl#property> _:B104823182afa6c235b8daed98b3b5ac7 .
_:B150417b36eb7ea87cdf5e9ac4c94221b <http://www.w3.org/ns/shacl#select> "SELECT $this\nWHERE {\n\t{\n    \tFILTER (EXISTS { $this $PATH ?any } && NOT EXISTS { $this $coExistsWith ?any })\n\t}\n\tUNION\n\t{\n    \tFILTER (NOT EXISTS { $this $PATH ?any } && EXISTS { $this $coExistsWith ?any })\n\t}\n}" .
<http://datashapes.org/dash#TestCase> <http://www.w3.org/1999/02/22-rdf-syntax-ns#type> <http://www.w3.org/2000/01/rdf-schema#Class> .
<http://datashapes.org/dash#hasClass> <http://www.w3.org/ns/shacl#ask> "\n\t\tASK {\n\t\t\t$value rdf:type/rdfs:subClassOf* $class .\n\t\t}\n\t\t" .
_:Bdad9596a4e29da75e0aa7a561275dd9f <http://www.w3.org/ns/shacl#jsFunctionName> "validateNode" .
_:B7f1ad1df154d5b4790aefb896d1c9fb8 <http://www.w3.org/ns/shacl#maxCount> "1"^^<http://www.w3.org/2001/XMLSchema#integer> .
<http://datashapes.org/dash#requiredExecutionPlatform> <http://www.w3.org/2000/01/rdf-schema#domain> <http://www.w3.org/ns/shacl#SPARQLExecutable> .
<http://datashapes.org/dash#StemConstraintComponent-stem> <http://www.w3.org/1999/02/22-rdf-syntax-ns#type> <http://www.w3.org/ns/shacl#Parameter> .
<http://datashapes.org/dash#hasMinInclusive> <http://www.w3.org/1999/02/22-rdf-syntax-ns#type> <http://www.w3.org/ns/shacl#SPARQLAskValidator> .
_:B13da662fb0d609b0fa8798a656baca2d <http://www.w3.org/ns/shacl#jsLibrary> <http://datashapes.org/dash#DASHJSLibrary> .
_:B21421ade4ccc7092969f52bbcc0d7484 <http://www.w3.org/1999/02/22-rdf-syntax-ns#type> <http://www.w3.org/ns/shacl#JSValidator> .
<http://www.w3.org/ns/shacl#TargetType> <http://datashapes.org/dash#abstract> "true"^^<http://www.w3.org/2001/XMLSchema#boolean> .
_:B881d49f14342613394c38418a3e2b26e <http://www.w3.org/ns/shacl#prefixes> <http://datashapes.org/dash> .
<http://datashapes.org/dash#DASHJSLibrary> <http://www.w3.org/2000/01/rdf-schema#label> "DASH JavaScript library" .
<http://datashapes.org/dash#reifiableBy> <http://www.w3.org/2000/01/rdf-schema#comment> "Can be used to specify the node shape that may be applied to reified statements produced by a property shape. The property shape must have a URI resource as its sh:path. The values of this property must be node shapes. User interfaces can use this information to determine which properties to present to users when reified statements are explored or edited. Use dash:None to indicate that no reification should be permitted." .
_:Bd79d8623d532452c0b9fb0617219aa16 <http://www.w3.org/ns/shacl#jsFunctionName> "validateMinExclusive" .
<http://datashapes.org/dash#SPARQLSelectTemplate> <http://www.w3.org/2000/01/rdf-schema#subClassOf> <http://www.w3.org/ns/shacl#SPARQLSelectExecutable> .
<http://www.w3.org/ns/shacl#NotConstraintComponent> <http://www.w3.org/ns/shacl#validator> _:B23e1001b72de7da857c5cf60a846810f .
_:B8d319a0761f1abba217993df30ee7b93 <http://www.w3.org/ns/shacl#prefix> "skos" .
_:B5672337cd6b085d4efa2003d67fc0562 <http://www.w3.org/ns/shacl#path> <http://datashapes.org/dash#predicate> .
<http://www.w3.org/ns/shacl#Parameterizable> <http://datashapes.org/dash#abstract> "true"^^<http://www.w3.org/2001/XMLSchema#boolean> .
<http://datashapes.org/dash#FailureTestCaseResult> <http://www.w3.org/2000/01/rdf-schema#label> "Failure test case result" .
<http://datashapes.org/dash#singleLine> <http://www.w3.org/1999/02/22-rdf-syntax-ns#type> <http://www.w3.org/1999/02/22-rdf-syntax-ns#Property> .
<http://datashapes.org/dash#cachable> <http://www.w3.org/2000/01/rdf-schema#label> "cachable" .
_:B160084f8X2D001cX2D4ef7X2Db5e9X2D120abccde94e <http://www.w3.org/1999/02/22-rdf-syntax-ns#rest> _:B58e95880X2Dc724X2D448aX2Da84dX2D04be1dee6648 .
<http://datashapes.org/dash#abstract> <http://www.w3.org/2000/01/rdf-schema#domain> <http://www.w3.org/2000/01/rdf-schema#Class> .
<http://datashapes.org/dash#TestCaseResult> <http://www.w3.org/ns/shacl#property> _:B6df3b0d09d638883ddc7eaf55d1a9646 .
<http://datashapes.org/dash#ClosedByTypesConstraintComponent> <http://www.w3.org/ns/shacl#parameter> <http://datashapes.org/dash#ClosedByTypesConstraintComponent-closedByTypes> .
_:Bed3045d9aeb8442f56a5b5a092925fd8 <http://www.w3.org/1999/02/22-rdf-syntax-ns#type> <http://www.w3.org/ns/shacl#JSValidator> .
_:Bd5a64ddffc0079f527ee5678e81011df <http://www.w3.org/ns/shacl#name> "expected result" .
<http://datashapes.org/dash#CoExistsWithConstraintComponent> <http://www.w3.org/ns/shacl#parameter> <http://datashapes.org/dash#CoExistsWithConstraintComponent-coExistsWith> .
_:B58e95880X2Dc724X2D448aX2Da84dX2D04be1dee6648 <http://www.w3.org/1999/02/22-rdf-syntax-ns#first> _:B7463b1c77e1b791dc8f96918e9ed48ab .
<http://datashapes.org/dash#HTMLOrStringOrLangString> <http://www.w3.org/2000/01/rdf-schema#comment> "An rdf:List that can be used in property constraints as value for sh:or to indicate that all values of a property must be either rdf:HTML, xsd:string or rdf:langString." .
<http://datashapes.org/dash#URIEditor> <http://www.w3.org/1999/02/22-rdf-syntax-ns#type> <http://datashapes.org/dash#Editor> .
<http://www.w3.org/ns/shacl#MaxExclusiveConstraintComponent> <http://www.w3.org/ns/shacl#validator> _:Ba7e7c348f2c50eb0f8f5b0beb9fb6862 .
_:B2b4ab9b1e883630e0b4029800ec9db7e <http://www.w3.org/ns/shacl#path> <http://www.w3.org/1999/02/22-rdf-syntax-ns#first> .
_:B78dae72f06fd9f3e8a68413ba2347650 <http://www.w3.org/1999/02/22-rdf-syntax-ns#type> <http://www.w3.org/ns/shacl#SPARQLSelectValidator> .
_:Ba7e7c348f2c50eb0f8f5b0beb9fb6862 <http://www.w3.org/ns/shacl#jsLibrary> <http://datashapes.org/dash#DASHJSLibrary> .
<http://datashapes.org/dash#InferencingTestCase> <http://www.w3.org/2000/01/rdf-schema#comment> "A test case to verify whether an inferencing engine is producing identical results to those stored as expected results." .
<http://datashapes.org/dash#FunctionTestCase> <http://www.w3.org/ns/shacl#property> _:B64037a34fda104980e7dda281bd2bc45 .
<http://datashapes.org/dash#editor> <http://www.w3.org/2000/01/rdf-schema#comment> "Can be used to link a property shape with an editor, to state a preferred editing widget in user interfaces." .
_:B2a3499b11e685d3ad17286d18e230c41 <http://www.w3.org/1999/02/22-rdf-syntax-ns#type> <http://www.w3.org/ns/shacl#JSValidator> .
<http://datashapes.org/dash#ReifiableByConstraintComponent> <http://www.w3.org/ns/shacl#labelTemplate> "Reifiable by {$reifiableBy}" .
_:B5672337cd6b085d4efa2003d67fc0562 <http://www.w3.org/ns/shacl#order> "1"^^<http://www.w3.org/2001/XMLSchema#integer> .
<http://datashapes.org/dash#stem> <http://www.w3.org/2000/01/rdf-schema#comment> "Specifies a string value that the IRI of the value nodes must start with."@en .
_:B12898dca29ca363f5ae4b1b4c90c363b <http://www.w3.org/ns/shacl#maxCount> "1"^^<http://www.w3.org/2001/XMLSchema#integer> .
<http://datashapes.org/dash#all> <http://www.w3.org/2000/01/rdf-schema#label> "all" .
_:Bf87fbb2c21e07adfb80e0445145d23a6 <http://www.w3.org/ns/shacl#jsLibrary> <http://datashapes.org/dash#DASHJSLibrary> .
<http://datashapes.org/dash#addedTriple> <http://www.w3.org/2000/01/rdf-schema#label> "added triple" .
<http://datashapes.org/dash#readOnly> <http://www.w3.org/2000/01/rdf-schema#label> "read only" .
<http://datashapes.org/dash#FunctionTestCase> <http://www.w3.org/ns/shacl#property> _:B2cb630d3ce6cc80fcb0af823135f42af .
<http://datashapes.org/dash#ExecutionPlatform> <http://www.w3.org/2000/01/rdf-schema#label> "Execution platform" .
_:B1f243cca064dc36a3759b064b48d1d3d <http://www.w3.org/ns/shacl#jsFunctionName> "validateQualifiedMaxCountProperty" .
<http://www.w3.org/ns/shacl#MaxInclusiveConstraintComponent> <http://www.w3.org/ns/shacl#validator> <http://datashapes.org/dash#hasMaxInclusive> .
<http://www.w3.org/ns/shacl#PatternConstraintComponent> <http://www.w3.org/ns/shacl#labelTemplate> "Value must match pattern \"{$pattern}\"" .
_:B35bf980a43fa9fd53edf3a01919e908b <http://www.w3.org/ns/shacl#ask> "ASK {\n    FILTER ($value = $hasValue)\n}" .
<http://datashapes.org/dash#GraphValidationTestCase> <http://www.w3.org/1999/02/22-rdf-syntax-ns#type> <http://www.w3.org/2000/01/rdf-schema#Class> .
<http://datashapes.org/dash#FunctionTestCase> <http://www.w3.org/2000/01/rdf-schema#label> "Function test case" .
_:B6df3b0d09d638883ddc7eaf55d1a9646 <http://www.w3.org/ns/shacl#maxCount> "1"^^<http://www.w3.org/2001/XMLSchema#integer> .
<http://datashapes.org/dash#validateShapes> <http://www.w3.org/2000/01/rdf-schema#comment> "True to also validate the shapes itself (i.e. parameter declarations)." .
<http://datashapes.org/dash#viewer> <http://www.w3.org/2000/01/rdf-schema#comment> "Can be used to link a property shape with a viewer, to state a preferred viewing widget in user interfaces." .
<http://datashapes.org/dash#DatePickerEditor> <http://www.w3.org/2000/01/rdf-schema#comment> "An editor for xsd:date literals, offering a calendar-like date picker." .
_:Bd5a64ddffc0079f527ee5678e81011df <http://www.w3.org/ns/shacl#maxCount> "1"^^<http://www.w3.org/2001/XMLSchema#integer> .
<http://datashapes.org/dash#DatePickerEditor> <http://www.w3.org/2000/01/rdf-schema#label> "Date picker editor" .
<http://datashapes.org/dash#JSTestCase> <http://www.w3.org/1999/02/22-rdf-syntax-ns#type> <http://www.w3.org/2000/01/rdf-schema#Class> .
_:Bbc6a3e0006c01fd1021e9a87d62d127a <http://www.w3.org/ns/shacl#path> <http://datashapes.org/dash#uri> .
_:B96cb50ba954aab266bfb44f5557bd78e <http://www.w3.org/ns/shacl#name> "constraint or shape" .
<http://datashapes.org/dash#BlankNodeViewer> <http://www.w3.org/2000/01/rdf-schema#label> "Blank Node Viewer" .
_:B192ffa056ee292f9513e19adb943a589 <http://www.w3.org/ns/shacl#jsLibrary> <http://datashapes.org/dash#DASHJSLibrary> .
<http://datashapes.org/dash#CoExistsWithConstraintComponent> <http://www.w3.org/ns/shacl#propertyValidator> _:B150417b36eb7ea87cdf5e9ac4c94221b .
_:B64037a34fda104980e7dda281bd2bc45 <http://www.w3.org/1999/02/22-rdf-syntax-ns#type> <http://www.w3.org/ns/shacl#PropertyShape> .
<http://datashapes.org/dash#hasMinLength> <http://www.w3.org/2000/01/rdf-schema#label> "has min length" .
<http://datashapes.org/dash#SPARQLConstructTemplate> <http://www.w3.org/2000/01/rdf-schema#subClassOf> <http://www.w3.org/ns/shacl#Parameterizable> .
<http://datashapes.org/dash#shape> <http://www.w3.org/2000/01/rdf-schema#range> <http://www.w3.org/ns/shacl#Shape> .
<http://www.w3.org/ns/shacl#PatternConstraintComponent> <http://www.w3.org/ns/shacl#message> "Value does not match pattern \"{$pattern}\"" .
<http://datashapes.org/dash#FunctionTestCase> <http://www.w3.org/1999/02/22-rdf-syntax-ns#type> <http://www.w3.org/2000/01/rdf-schema#Class> .
<http://datashapes.org/dash#isIn> <http://www.w3.org/2000/01/rdf-schema#label> "is in" .
_:B3b32abda9658f358f57cc4b5edac88b8 <http://www.w3.org/1999/02/22-rdf-syntax-ns#type> <http://www.w3.org/ns/shacl#PropertyShape> .
<http://datashapes.org/dash#viewer> <http://www.w3.org/2000/01/rdf-schema#range> <http://datashapes.org/dash#Viewer> .
<http://datashapes.org/dash#AllObjects> <http://www.w3.org/1999/02/22-rdf-syntax-ns#type> <http://datashapes.org/dash#AllObjectsTarget> .
<http://datashapes.org/dash#SuccessTestCaseResult> <http://www.w3.org/1999/02/22-rdf-syntax-ns#type> <http://www.w3.org/2000/01/rdf-schema#Class> .
_:Ba6acc14fd45c4c8b7041edd8b3005f16 <http://www.w3.org/ns/shacl#name> "arg" .
<http://datashapes.org/dash#isNodeKindIRI> <http://www.w3.org/1999/02/22-rdf-syntax-ns#type> <http://www.w3.org/ns/shacl#SPARQLFunction> .
_:B835aab3b1aa9569620d379dbdd889674 <http://www.w3.org/1999/02/22-rdf-syntax-ns#type> <http://www.w3.org/ns/shacl#JSValidator> .
<http://datashapes.org/dash#SubSetOfConstraintComponent> <http://www.w3.org/2000/01/rdf-schema#comment> "A constraint component that can be used to state that the set of value nodes must be a subset of the value of a given property." .
<http://datashapes.org/dash#Widget> <http://www.w3.org/1999/02/22-rdf-syntax-ns#type> <http://www.w3.org/2000/01/rdf-schema#Class> .
_:Ba7e7c348f2c50eb0f8f5b0beb9fb6862 <http://www.w3.org/ns/shacl#jsFunctionName> "validateMaxExclusive" .
_:Bed3045d9aeb8442f56a5b5a092925fd8 <http://www.w3.org/ns/shacl#message> "Predicate is not allowed (closed shape)" .
<http://datashapes.org/dash#cachable> <http://www.w3.org/2000/01/rdf-schema#range> <http://www.w3.org/2001/XMLSchema#boolean> .
<http://www.w3.org/ns/shacl#Rule> <http://datashapes.org/dash#abstract> "true"^^<http://www.w3.org/2001/XMLSchema#boolean> .
<http://datashapes.org/dash#TestCase> <http://www.w3.org/2000/01/rdf-schema#comment> "A test case to verify that a (SHACL-based) feature works as expected." .
<http://datashapes.org/dash#GraphStoreTestCase> <http://www.w3.org/2000/01/rdf-schema#label> "Graph store test case" .
<http://datashapes.org/dash#fixed> <http://www.w3.org/2000/01/rdf-schema#label> "fixed" .
<http://www.w3.org/ns/shacl#DisjointConstraintComponent> <http://www.w3.org/ns/shacl#validator> _:B8791b3a24b8675de3fe6cea3980f416f .
<http://datashapes.org/dash#GraphStoreTestCase> <http://www.w3.org/1999/02/22-rdf-syntax-ns#type> <http://www.w3.org/2000/01/rdf-schema#Class> .
<http://datashapes.org/dash#RootClassConstraintComponent> <http://www.w3.org/ns/shacl#parameter> <http://datashapes.org/dash#RootClassConstraintComponent-rootClass> .
<http://datashapes.org/dash#defaultViewForRole> <http://www.w3.org/2000/01/rdf-schema#label> "default view for role" .
<http://datashapes.org/dash#testModifiesEnvironment> <http://www.w3.org/2000/01/rdf-schema#range> <http://www.w3.org/2001/XMLSchema#boolean> .
<http://www.w3.org/ns/shacl#Rules> <http://www.w3.org/2000/01/rdf-schema#seeAlso> <https://www.w3.org/TR/shacl-af/#Rules> .
_:B3dc0d1acdae51f4d90e61301d771976f <http://www.w3.org/1999/02/22-rdf-syntax-ns#type> <http://www.w3.org/ns/shacl#JSValidator> .
<http://datashapes.org/dash#TextFieldEditor> <http://www.w3.org/2000/01/rdf-schema#label> "Text field editor" .
<http://www.w3.org/ns/shacl#MaxLengthConstraintComponent> <http://datashapes.org/dash#staticConstraint> "true"^^<http://www.w3.org/2001/XMLSchema#boolean> .
_:B6d4cbc3d992ff864f2dac864d1480fb8 <http://www.w3.org/1999/02/22-rdf-syntax-ns#type> <http://www.w3.org/ns/shacl#PropertyShape> .
_:B4f9dd044b748456b76262d5363cb5a94 <http://www.w3.org/ns/shacl#select> "SELECT $this (?predicate AS ?path) ?value\nWHERE {\n\tFILTER ($closedByTypes) .\n    $this ?predicate ?value .\n\tFILTER (?predicate != rdf:type) .\n\tFILTER NOT EXISTS {\n\t\t$this rdf:type ?type .\n\t\t?type rdfs:subClassOf* ?class .\n\t\tGRAPH $shapesGraph {\n\t\t\t?class sh:property/sh:path ?predicate .\n\t\t}\n\t}\n}" .
<http://datashapes.org/dash#hasNodeKind> <http://www.w3.org/ns/shacl#prefixes> <http://datashapes.org/dash> .
<http://datashapes.org/dash#toString> <http://www.w3.org/2000/01/rdf-schema#label> "to string" .
<http://datashapes.org/dash#StemConstraintComponent> <http://www.w3.org/2000/01/rdf-schema#label> "Stem constraint component"@en .
<http://datashapes.org/dash#hasMaxLength> <http://www.w3.org/1999/02/22-rdf-syntax-ns#type> <http://www.w3.org/ns/shacl#SPARQLAskValidator> .
<http://www.w3.org/ns/shacl#OrConstraintComponent> <http://www.w3.org/ns/shacl#validator> _:B66978dfbb7ff7fc62ba1381b3242ae8e .
<http://datashapes.org/dash#ListShape> <http://www.w3.org/ns/shacl#or> _:Bd2820cd0X2D1befX2D4fb9X2D934fX2Dd31b1666ea53 .
<http://datashapes.org/dash#SingleLineConstraintComponent> <http://www.w3.org/ns/shacl#validator> _:Bc91acb30da815118fca913844f6cfa7b .
<http://datashapes.org/dash#ImageViewer> <http://www.w3.org/2000/01/rdf-schema#comment> "A Viewer for URI values that are recognized as images by a browser, rendering as an image." .
<http://datashapes.org/dash#includedExecutionPlatform> <http://www.w3.org/2000/01/rdf-schema#label> "included execution platform" .
<http://datashapes.org/dash#valueCount> <http://www.w3.org/ns/shacl#prefixes> <http://datashapes.org/dash> .
<http://datashapes.org/dash#symmetric> <http://www.w3.org/1999/02/22-rdf-syntax-ns#type> <http://www.w3.org/1999/02/22-rdf-syntax-ns#Property> .
_:B5ea6cb49b4f6b98c242342a8a98d3388 <http://www.w3.org/ns/shacl#hasValue> <http://www.w3.org/1999/02/22-rdf-syntax-ns#nil> .
<http://datashapes.org/dash#addedTriple> <http://www.w3.org/2000/01/rdf-schema#comment> "May link a dash:GraphUpdate with one or more triples (represented as instances of rdf:Statement) that should be added to fix the source of the result." .
_:Ba6acc14fd45c4c8b7041edd8b3005f16 <http://www.w3.org/ns/shacl#path> <http://datashapes.org/dash#arg> .
<http://datashapes.org/dash#InstancesSelectEditor> <http://www.w3.org/2000/01/rdf-schema#label> "Instances select editor" .
_:B9e11ce9adf350d1895c6096c2ef7444d <http://www.w3.org/ns/shacl#jsFunctionName> "validateLessThanProperty" .
_:B9fe7602a489f48a08b22e99931d59d35 <http://www.w3.org/ns/shacl#description> "The expected result set, as a JSON string." .
<http://datashapes.org/dash#toString> <http://www.w3.org/1999/02/22-rdf-syntax-ns#type> <http://www.w3.org/ns/shacl#SPARQLFunction> .
<http://datashapes.org/dash#StringOrLangString> <http://www.w3.org/2000/01/rdf-schema#label> "String or langString" .
<http://datashapes.org/dash#hasMinExclusive> <http://www.w3.org/1999/02/22-rdf-syntax-ns#type> <http://www.w3.org/ns/shacl#SPARQLAskValidator> .
<http://www.w3.org/ns/shacl#DisjointConstraintComponent> <http://datashapes.org/dash#localConstraint> "true"^^<http://www.w3.org/2001/XMLSchema#boolean> .
<http://datashapes.org/dash#HTMLViewer> <http://www.w3.org/2000/01/rdf-schema#comment> "A Viewer for HTML encoded text from rdf:HTML literals, rendering as parsed HTML DOM elements. Also displays the language if the HTML has a lang attribute on its root DOM element." .
<http://datashapes.org/dash#ImageViewer> <http://www.w3.org/1999/02/22-rdf-syntax-ns#type> <http://datashapes.org/dash#Viewer> .
<http://datashapes.org/dash#GraphStoreTestCase> <http://www.w3.org/ns/shacl#property> _:B6d4cbc3d992ff864f2dac864d1480fb8 .
<http://www.w3.org/ns/shacl#ClosedConstraintComponent> <http://www.w3.org/ns/shacl#nodeValidator> _:B8a6d95446c24ef2a1314f1cfdc6ea805 .
<http://datashapes.org/dash#TextAreaWithLangEditor> <http://www.w3.org/1999/02/22-rdf-syntax-ns#type> <http://datashapes.org/dash#Editor> .
<http://datashapes.org/dash#defaultValueType> <http://www.w3.org/1999/02/22-rdf-syntax-ns#type> <http://www.w3.org/1999/02/22-rdf-syntax-ns#Property> .
<http://datashapes.org/dash> <http://www.w3.org/ns/shacl#declare> _:B140f0995d12aa7e2492672c94ebf1c8f .
<http://datashapes.org/dash#HasValueWithClassConstraintComponent-hasValueWithClass> <http://www.w3.org/1999/02/22-rdf-syntax-ns#type> <http://www.w3.org/ns/shacl#Parameter> .
<http://datashapes.org/dash#TextAreaWithLangEditor> <http://www.w3.org/2000/01/rdf-schema#label> "Text area with lang editor" .
<http://datashapes.org/dash#hasPattern> <http://www.w3.org/ns/shacl#prefixes> <http://datashapes.org/dash> .
<http://datashapes.org/dash#StemConstraintComponent> <http://www.w3.org/2000/01/rdf-schema#comment> "A constraint component that can be used to verify that every value node is an IRI and the IRI starts with a given string value."@en .
<http://www.w3.org/ns/shacl#MaxInclusiveConstraintComponent> <http://datashapes.org/dash#staticConstraint> "true"^^<http://www.w3.org/2001/XMLSchema#boolean> .
<http://www.w3.org/ns/shacl#QualifiedMinCountConstraintComponent> <http://www.w3.org/ns/shacl#labelTemplate> "No fewer than {$qualifiedMinCount} values can have shape {$qualifiedValueShape}" .
<http://datashapes.org/dash#detailsGraph> <http://www.w3.org/2000/01/rdf-schema#label> "details graph" .
<http://datashapes.org/dash#requiredExecutionPlatform> <http://www.w3.org/1999/02/22-rdf-syntax-ns#type> <http://www.w3.org/1999/02/22-rdf-syntax-ns#Property> .
<http://datashapes.org/dash#staticConstraint> <http://www.w3.org/2000/01/rdf-schema#comment> "Can be set to true for those constraint components where the validation does not require to visit any other triples than the parameters. Examples of this include sh:datatype or sh:nodeKind, where no further triples need to be queried to determine the result.\n\nConstraint components that are marked as such can be optimized by engines, e.g. they can be evaluated client-side at form submission time, without having to make a round-trip to a server." .
<http://www.w3.org/ns/shacl#NodeKindConstraintComponent> <http://www.w3.org/ns/shacl#validator> <http://datashapes.org/dash#hasNodeKind> .
<http://datashapes.org/dash#RootClassConstraintComponent-rootClass> <http://www.w3.org/ns/shacl#path> <http://datashapes.org/dash#rootClass> .
<http://datashapes.org/dash#localConstraint> <http://www.w3.org/2000/01/rdf-schema#comment> "Can be set to true for those constraint components where the validation does not require to visit any other triples than the shape definitions and the direct property values of the focus node mentioned in the property constraints. Examples of this include sh:minCount and sh:hasValue.\n\nConstraint components that are marked as such can be optimized by engines, e.g. they can be evaluated client-side at form submission time, without having to make a round-trip to a server, assuming the client has downloaded a complete snapshot of the resource.\n\nAny component marked with dash:staticConstraint is also a dash:localConstraint." .
_:B2cb630d3ce6cc80fcb0af823135f42af <http://www.w3.org/ns/shacl#maxCount> "1"^^<http://www.w3.org/2001/XMLSchema#integer> .
_:B0c0f328c69e13d06674f58bb5b4a9284 <http://www.w3.org/ns/shacl#path> <http://datashapes.org/dash#singleLine> .
_:B3dc0d1acdae51f4d90e61301d771976f <http://www.w3.org/ns/shacl#jsLibrary> <http://datashapes.org/dash#DASHJSLibrary> .
_:Bd5a64ddffc0079f527ee5678e81011df <http://www.w3.org/ns/shacl#description> "The expected result of the JavaScript function call, as an RDF node." .
<http://datashapes.org/dash#ClosedByTypesConstraintComponent-closedByTypes> <http://www.w3.org/ns/shacl#description> "True to indicate that the focus nodes are closed by their types. A constraint violation is reported for each property value of the focus node where the property is not among those that are explicitly declared via sh:property/sh:path in any of the rdf:types of the focus node (and their superclasses). The property rdf:type is always permitted." .
<http://www.w3.org/ns/shacl#LessThanOrEqualsConstraintComponent> <http://www.w3.org/ns/shacl#message> "Value is not <= value of {$lessThanOrEquals}" .
<http://datashapes.org/dash#UniqueValueForClassConstraintComponent-uniqueValueForClass> <http://www.w3.org/ns/shacl#nodeKind> <http://www.w3.org/ns/shacl#IRI> .
_:B64037a34fda104980e7dda281bd2bc45 <http://www.w3.org/ns/shacl#description> "The expected result of a function call." .
_:B88430adc5caf16f7f8cd82bc8fb6a6f8 <http://www.w3.org/ns/shacl#prefixes> <http://datashapes.org/dash> .
_:B0501804cef6c59c65c932d30353a449b <http://www.w3.org/ns/shacl#message> "Value {?value} must be unique but is also used by {?other}" .
<http://datashapes.org/dash#HasValueWithClassConstraintComponent-hasValueWithClass> <http://www.w3.org/ns/shacl#class> <http://www.w3.org/2000/01/rdf-schema#Class> .
<http://datashapes.org/dash#hasStem> <http://www.w3.org/ns/shacl#ask> "ASK { FILTER (isIRI($value) && STRSTARTS(str($value), $stem)) }" .
<http://datashapes.org/dash#applicableToClass> <http://www.w3.org/2000/01/rdf-schema#range> <http://www.w3.org/2000/01/rdf-schema#Class> .
<http://www.w3.org/ns/shacl#DatatypeConstraintComponent> <http://www.w3.org/ns/shacl#validator> _:B567e621e200ca5c599b5f14c17b0e7b3 .
<http://datashapes.org/dash#URIViewer> <http://www.w3.org/2000/01/rdf-schema#comment> "A Viewer for URI resources, rendering as a hyperlink to that URI. Also includes other ways of interacting with the URI such as opening a nested summary display." .
<http://datashapes.org/dash#QueryTestCase> <http://www.w3.org/2000/01/rdf-schema#subClassOf> <http://datashapes.org/dash#TestCase> .
<http://datashapes.org/dash#ValidationTestCase> <http://datashapes.org/dash#abstract> "true"^^<http://www.w3.org/2001/XMLSchema#boolean> .
<http://datashapes.org/dash#isLanguageIn> <http://www.w3.org/1999/02/22-rdf-syntax-ns#type> <http://www.w3.org/ns/shacl#SPARQLAskValidator> .
<http://datashapes.org/dash#staticConstraint> <http://www.w3.org/2000/01/rdf-schema#label> "static constraint" .
<http://datashapes.org/dash#PrimaryKeyConstraintComponent-uriStart> <http://www.w3.org/1999/02/22-rdf-syntax-ns#type> <http://www.w3.org/ns/shacl#Parameter> .
_:Ba6acc14fd45c4c8b7041edd8b3005f16 <http://www.w3.org/ns/shacl#description> "The input value." .
<http://datashapes.org/dash#DateOrDateTime> <http://www.w3.org/1999/02/22-rdf-syntax-ns#first> _:Bf82714b519b59627a7719a96ae3deb05 .
<http://datashapes.org/dash#NonRecursiveConstraintComponent> <http://www.w3.org/ns/shacl#parameter> <http://datashapes.org/dash#NonRecursiveConstraintComponent-nonRecursive> .
<http://datashapes.org/dash#LabelViewer> <http://www.w3.org/1999/02/22-rdf-syntax-ns#type> <http://datashapes.org/dash#Viewer> .
<http://datashapes.org/dash> <http://www.w3.org/ns/shacl#declare> _:B6a3dda78c1d1372a3ae27e96a10584b5 .
<http://datashapes.org/dash#UniqueValueForClassConstraintComponent-uniqueValueForClass> <http://www.w3.org/1999/02/22-rdf-syntax-ns#type> <http://www.w3.org/ns/shacl#Parameter> .
_:Beb225391b5ff8fb10e272118f430ade4 <http://www.w3.org/ns/shacl#jsFunctionName> "validateNodeKind" .
<http://datashapes.org/dash#EnumSelectEditor> <http://www.w3.org/2000/01/rdf-schema#comment> "A drop-down editor for enumerated values (typically based on sh:in lists)." .
<http://www.w3.org/ns/shacl#MinLengthConstraintComponent> <http://www.w3.org/ns/shacl#validator> <http://datashapes.org/dash#hasMinLength> .
<http://datashapes.org/dash#RDFQueryJSLibrary> <http://www.w3.org/1999/02/22-rdf-syntax-ns#type> <http://www.w3.org/ns/shacl#JSLibrary> .
<http://datashapes.org/dash#JSTestCase> <http://www.w3.org/2000/01/rdf-schema#label> "JavaScript test case" .
<http://www.w3.org/ns/shacl#MinLengthConstraintComponent> <http://datashapes.org/dash#staticConstraint> "true"^^<http://www.w3.org/2001/XMLSchema#boolean> .
<http://datashapes.org/dash#readOnly> <http://www.w3.org/2000/01/rdf-schema#comment> "Used as a hint for user interfaces that values of the associated property should not be editable. The values of this may be the boolean literals true or false or, more generally, a SHACL node expression that must evaluate to true or false." .
<http://datashapes.org/dash#hasClass> <http://www.w3.org/ns/shacl#message> "Value does not have class {$class}" .
<http://datashapes.org/dash#stem> <http://www.w3.org/2000/01/rdf-schema#label> "stem"@en .
_:B835aab3b1aa9569620d379dbdd889674 <http://www.w3.org/ns/shacl#jsLibrary> <http://datashapes.org/dash#DASHJSLibrary> .
_:B31473064d8bd1e288bd70b63b0f116a3 <http://www.w3.org/ns/shacl#description> "The sh:NodeKind to check." .
_:B104823182afa6c235b8daed98b3b5ac7 <http://datashapes.org/dash#nonRecursive> "true"^^<http://www.w3.org/2001/XMLSchema#boolean> .
_:B58e95880X2Dc724X2D448aX2Da84dX2D04be1dee6648 <http://www.w3.org/1999/02/22-rdf-syntax-ns#rest> <http://www.w3.org/1999/02/22-rdf-syntax-ns#nil> .
_:B0501804cef6c59c65c932d30353a449b <http://www.w3.org/1999/02/22-rdf-syntax-ns#type> <http://www.w3.org/ns/shacl#SPARQLSelectValidator> .
_:B1131591453602389668eae575a1a4693 <http://www.w3.org/1999/02/22-rdf-syntax-ns#type> <http://www.w3.org/ns/shacl#PropertyShape> .
<http://www.w3.org/ns/shacl#NodeKindConstraintComponent> <http://datashapes.org/dash#staticConstraint> "true"^^<http://www.w3.org/2001/XMLSchema#boolean> .
<http://datashapes.org/dash#HasValueWithClassConstraintComponent-hasValueWithClass> <http://www.w3.org/ns/shacl#nodeKind> <http://www.w3.org/ns/shacl#IRI> .
_:B192ffa056ee292f9513e19adb943a589 <http://www.w3.org/1999/02/22-rdf-syntax-ns#type> <http://www.w3.org/ns/shacl#JSValidator> .
<http://datashapes.org/dash#reifiableBy> <http://www.w3.org/2000/01/rdf-schema#domain> <http://www.w3.org/ns/shacl#PropertyShape> .
<http://datashapes.org/dash#ValidationTestCase> <http://www.w3.org/2000/01/rdf-schema#label> "Validation test case" .
_:B567e621e200ca5c599b5f14c17b0e7b3 <http://www.w3.org/ns/shacl#jsFunctionName> "validateDatatype" .
<http://datashapes.org/dash#includedExecutionPlatform> <http://www.w3.org/2000/01/rdf-schema#domain> <http://datashapes.org/dash#ExecutionPlatform> .
_:B978525ea2f32d0660c9ffc71e8b5d4cd <http://www.w3.org/ns/shacl#not> _:B2bc3ad21d29b4bdb3981840c7e38c769 .
<http://www.w3.org/ns/shacl#MaxExclusiveConstraintComponent> <http://www.w3.org/ns/shacl#message> "Value is not < {$maxExclusive}" .
<http://datashapes.org/dash#PrimaryKeyConstraintComponent> <http://www.w3.org/ns/shacl#labelTemplate> "The property {?predicate} is the primary key and URIs start with {?uriStart}" .
<http://datashapes.org/dash#testEnvironment> <http://www.w3.org/2000/01/rdf-schema#range> <http://datashapes.org/dash#TestEnvironment> .
<http://datashapes.org/dash#UniqueValueForClassConstraintComponent-uniqueValueForClass> <http://www.w3.org/ns/shacl#class> <http://www.w3.org/2000/01/rdf-schema#Class> .
_:Bd7d823a9ff3f41bf4f9c8b66d70cce69 <http://www.w3.org/ns/shacl#jsFunctionName> "validateMinLength" .
<http://datashapes.org/dash#RichTextEditor> <http://www.w3.org/2000/01/rdf-schema#label> "Rich text editor" .
_:Baf7234052e57bdd00025c4c0de812c1d <http://www.w3.org/ns/shacl#select> "\n\t\tSELECT $this\n\t\tWHERE {\n\t\t\tFILTER NOT EXISTS { $this $PATH $hasValue }\n\t\t}\n\t\t" .
<http://datashapes.org/dash#closedByTypes> <http://www.w3.org/1999/02/22-rdf-syntax-ns#type> <http://www.w3.org/1999/02/22-rdf-syntax-ns#Property> .
<http://www.w3.org/ns/shacl#MinLengthConstraintComponent> <http://www.w3.org/ns/shacl#validator> _:Bd7d823a9ff3f41bf4f9c8b66d70cce69 .
<http://datashapes.org/dash#isDeactivated> <http://www.w3.org/ns/shacl#returnType> <http://www.w3.org/2001/XMLSchema#boolean> .
<http://datashapes.org/dash#UniqueValueForClassConstraintComponent> <http://www.w3.org/ns/shacl#propertyValidator> _:Baca6b78cb251a419ee913fa362fa0fad .
<http://datashapes.org/dash#localConstraint> <http://www.w3.org/2000/01/rdf-schema#range> <http://www.w3.org/2001/XMLSchema#boolean> .
<http://datashapes.org/dash#SPARQLSelectTemplate> <http://www.w3.org/2000/01/rdf-schema#comment> "Encapsulates a SPARQL SELECT query that can be parameterized. Parameters will become pre-bound variables in the query." .
<http://datashapes.org/dash#stem> <http://www.w3.org/2000/01/rdf-schema#range> <http://www.w3.org/2001/XMLSchema#string> .
_:B324a4eda45fae1908023e86a8b10dbdb <http://www.w3.org/ns/shacl#jsLibrary> <http://datashapes.org/dash#DASHJSLibrary> .
<http://datashapes.org/dash#fixed> <http://www.w3.org/1999/02/22-rdf-syntax-ns#type> <http://www.w3.org/1999/02/22-rdf-syntax-ns#Property> .
<http://datashapes.org/dash#propertySuggestionGenerator> <http://www.w3.org/2000/01/rdf-schema#label> "property suggestion generator" .
<http://www.w3.org/ns/shacl#EqualsConstraintComponent> <http://www.w3.org/ns/shacl#nodeValidator> _:Bd048027623bcc6288ff18f5d0dfbb126 .
_:B150417b36eb7ea87cdf5e9ac4c94221b <http://www.w3.org/ns/shacl#prefixes> <http://datashapes.org/dash> .
<http://www.w3.org/ns/shacl#MaxCountConstraintComponent> <http://www.w3.org/ns/shacl#propertyValidator> _:B8ba63feb6e245955b305042229b7785c .
<http://datashapes.org/dash#hasNodeKind> <http://www.w3.org/ns/shacl#ask> "\n\t\tASK {\n\t\t\tFILTER ((isIRI($value) && $nodeKind IN ( sh:IRI, sh:BlankNodeOrIRI, sh:IRIOrLiteral ) ) ||\n\t\t\t\t(isLiteral($value) && $nodeKind IN ( sh:Literal, sh:BlankNodeOrLiteral, sh:IRIOrLiteral ) ) ||\n\t\t\t\t(isBlank($value)   && $nodeKind IN ( sh:BlankNode, sh:BlankNodeOrIRI, sh:BlankNodeOrLiteral ) )) .\n\t\t}\n\t\t" .
_:B646fdae9066263aad8548980a9a6346d <http://www.w3.org/1999/02/22-rdf-syntax-ns#type> <http://www.w3.org/ns/shacl#JSValidator> .
<http://datashapes.org/dash#StemConstraintComponent> <http://datashapes.org/dash#staticConstraint> "true"^^<http://www.w3.org/2001/XMLSchema#boolean> .
_:B83c9da54cec674e1fa200619bc30f9bb <http://www.w3.org/ns/shacl#jsFunctionName> "validateLessThanOrEqualsProperty" .
<http://datashapes.org/dash#hasMinExclusive> <http://www.w3.org/2000/01/rdf-schema#label> "has min exclusive" .
<http://datashapes.org/dash#ClosedByTypesConstraintComponent-closedByTypes> <http://www.w3.org/ns/shacl#datatype> <http://www.w3.org/2001/XMLSchema#boolean> .
_:B9fe7602a489f48a08b22e99931d59d35 <http://www.w3.org/ns/shacl#path> <http://datashapes.org/dash#expectedResult> .
<http://datashapes.org/dash#ReifiableByConstraintComponent-reifiableBy> <http://www.w3.org/1999/02/22-rdf-syntax-ns#type> <http://www.w3.org/ns/shacl#Parameter> .
_:B8791b3a24b8675de3fe6cea3980f416f <http://www.w3.org/ns/shacl#ask> "\n\t\tASK {\n\t\t\tFILTER NOT EXISTS {\n\t\t\t\t$this $disjoint $value .\n\t\t\t}\n\t\t}\n\t\t" .
_:B64037a34fda104980e7dda281bd2bc45 <http://www.w3.org/ns/shacl#name> "expected result" .
<http://datashapes.org/dash#TestCase> <http://datashapes.org/dash#abstract> "true"^^<http://www.w3.org/2001/XMLSchema#boolean> .
<http://datashapes.org/dash#DetailsViewer> <http://www.w3.org/2000/01/rdf-schema#comment> "A Viewer for resources that shows the details of the value using its default view shape as a nested form-like display." .
_:B3b32abda9658f358f57cc4b5edac88b8 <http://www.w3.org/ns/shacl#name> "expected result" .
<http://datashapes.org/dash#defaultValueType> <http://www.w3.org/2000/01/rdf-schema#range> <http://www.w3.org/2000/01/rdf-schema#Class> .
<http://www.w3.org/ns/shacl#UniqueLangConstraintComponent> <http://www.w3.org/ns/shacl#propertyValidator> _:B850a3561a7b96169d0a48349ceccf59d .
<http://datashapes.org/dash#GraphStoreTestCase> <http://www.w3.org/2000/01/rdf-schema#comment> "A test case that can be used to verify that an RDF file could be loaded (from a file) and that the resulting RDF graph is equivalent to a given TTL file." .
_:B7463b1c77e1b791dc8f96918e9ed48ab <http://www.w3.org/ns/shacl#property> _:Bff9ecbe5a61b70becac46f6b4ddfdb03 .
<http://datashapes.org/dash#AllObjectsTarget> <http://www.w3.org/1999/02/22-rdf-syntax-ns#type> <http://www.w3.org/ns/shacl#JSTargetType> .
<http://datashapes.org/dash#Editor> <http://www.w3.org/1999/02/22-rdf-syntax-ns#type> <http://www.w3.org/ns/shacl#NodeShape> .
_:B324a4eda45fae1908023e86a8b10dbdb <http://www.w3.org/ns/shacl#message> "Property is not among those permitted for any of the types" .
<http://datashapes.org/dash#TestCaseResult> <http://www.w3.org/2000/01/rdf-schema#comment> "Base class for results produced by running test cases." .
<http://datashapes.org/dash#ValidationTestCase> <http://www.w3.org/1999/02/22-rdf-syntax-ns#type> <http://www.w3.org/ns/shacl#NodeShape> .
<http://www.w3.org/ns/shacl#JSExecutable> <http://datashapes.org/dash#abstract> "true"^^<http://www.w3.org/2001/XMLSchema#boolean> .
_:B9f8708a030e28285db3efcfa7150f80b <http://www.w3.org/ns/shacl#jsLibrary> <http://datashapes.org/dash#DASHJSLibrary> .
<http://datashapes.org/dash#defaultViewForRole> <http://www.w3.org/1999/02/22-rdf-syntax-ns#type> <http://www.w3.org/1999/02/22-rdf-syntax-ns#Property> .
_:B12898dca29ca363f5ae4b1b4c90c363b <http://www.w3.org/1999/02/22-rdf-syntax-ns#type> <http://www.w3.org/ns/shacl#PropertyShape> .
<http://datashapes.org/dash#validateShapes> <http://www.w3.org/1999/02/22-rdf-syntax-ns#type> <http://www.w3.org/1999/02/22-rdf-syntax-ns#Property> .
<http://datashapes.org/dash#ValidationTestCase> <http://www.w3.org/ns/shacl#property> _:B6431ca200460b7f86c096adcb4867b07 .
<http://datashapes.org/dash#detailsEndpoint> <http://www.w3.org/2000/01/rdf-schema#comment> "Can be used to link a SHACL property shape with the URL of a SPARQL endpoint that may contain further RDF triples for the value nodes delivered by the property. This can be used to inform a processor that it should switch to values from an external graph when the user wants to retrieve more information about a value.\n\nThis property should be regarded as an \"annotation\", i.e. it does not have any impact on validation or other built-in SHACL features. However, selected tools may want to use this information. One implementation strategy would be to periodically fetch the values specified by the sh:node or sh:class shape associated with the property, using the property shapes in that shape, and add the resulting triples into the main query graph.\n\nAn example value is \"https://query.wikidata.org/sparql\"." .
_:B576b207887a27c8640d054dd19740272 <http://www.w3.org/ns/shacl#select> "\n\t\tSELECT $this ?value\n\t\tWHERE {\n\t\t\t$this $PATH ?value .\n\t\t\t$this $lessThan ?otherValue .\n\t\t\tBIND (?value < ?otherValue AS ?result) .\n\t\t\tFILTER (!bound(?result) || !(?result)) .\n\t\t}\n\t\t" .
<http://datashapes.org/dash#AutoCompleteEditor> <http://www.w3.org/2000/01/rdf-schema#comment> "An auto-complete field to enter the label of instances of a class. This is the fallback editor for any URI resource if no other editors are more suitable." .
<http://datashapes.org/dash#ClosedByTypesConstraintComponent-closedByTypes> <http://www.w3.org/ns/shacl#path> <http://datashapes.org/dash#closedByTypes> .
<http://datashapes.org/dash#suggestionGenerator> <http://www.w3.org/2000/01/rdf-schema#comment> "Links a sh:SPARQLConstraint or sh:JSConstraint with instances of dash:SuggestionGenerator that may be used to produce suggestions for a given validation result that was produced by the constraint." .
_:B61f5442de5a071e03f0bc4b21b3752cc <http://www.w3.org/ns/shacl#select> "SELECT $this ?value {\n\tFILTER ($symmetric) .\n\t$this $PATH ?value .\n\tFILTER NOT EXISTS {\n    \t?value $PATH $this .\n\t}\n}" .
_:Bb254f7a557dd3b29bbe20622d1b148be <http://www.w3.org/1999/02/22-rdf-syntax-ns#type> <http://www.w3.org/ns/shacl#SPARQLSelectValidator> .
_:Bef4b4e661cf3b607381181797fae49a3 <http://www.w3.org/ns/shacl#class> <http://www.w3.org/ns/shacl#NodeKind> .
_:Bdad9596a4e29da75e0aa7a561275dd9f <http://www.w3.org/1999/02/22-rdf-syntax-ns#type> <http://www.w3.org/ns/shacl#JSValidator> .
<http://datashapes.org/dash#ReifiableByConstraintComponent> <http://www.w3.org/2000/01/rdf-schema#label> "Reifiable-by constraint component" .
<http://datashapes.org/dash#suggestionConfidence> <http://www.w3.org/2000/01/rdf-schema#comment> "An optional confidence between 0% and 100%. Suggestions with 100% confidence are strongly recommended. Can be used to sort recommended updates." .
_:B1db6386c181b226090f5a502966d369b <http://www.w3.org/ns/shacl#jsLibrary> <http://datashapes.org/dash#DASHJSLibrary> .
_:B6431ca200460b7f86c096adcb4867b07 <http://www.w3.org/ns/shacl#description> "The expected validation report." .
<http://datashapes.org/dash#hasMinInclusive> <http://www.w3.org/ns/shacl#ask> "ASK { FILTER ($value >= $minInclusive) }" .
_:Ba6acc14fd45c4c8b7041edd8b3005f16 <http://www.w3.org/ns/shacl#nodeKind> <http://www.w3.org/ns/shacl#IRIOrLiteral> .
<http://datashapes.org/dash#DateOrDateTime> <http://www.w3.org/1999/02/22-rdf-syntax-ns#type> <http://www.w3.org/1999/02/22-rdf-syntax-ns#List> .
<http://datashapes.org/dash#InferencingTestCase> <http://www.w3.org/2000/01/rdf-schema#subClassOf> <http://datashapes.org/dash#TestCase> .
<http://datashapes.org/dash#propertySuggestionGenerator> <http://www.w3.org/2000/01/rdf-schema#range> <http://datashapes.org/dash#SuggestionGenerator> .
_:B1131591453602389668eae575a1a4693 <http://www.w3.org/ns/shacl#path> <http://www.w3.org/ns/shacl#select> .
<http://www.w3.org/ns/shacl#LanguageInConstraintComponent> <http://www.w3.org/ns/shacl#validator> <http://datashapes.org/dash#isLanguageIn> .
<http://datashapes.org/dash#viewer> <http://www.w3.org/2000/01/rdf-schema#label> "viewer" .
<http://datashapes.org/dash#BooleanSelectEditor> <http://www.w3.org/2000/01/rdf-schema#label> "Boolean select editor" .
<http://www.w3.org/ns/shacl#NotConstraintComponent> <http://www.w3.org/ns/shacl#targetClass> <http://www.w3.org/ns/shacl#Shape> .
_:B576b207887a27c8640d054dd19740272 <http://www.w3.org/1999/02/22-rdf-syntax-ns#type> <http://www.w3.org/ns/shacl#SPARQLSelectValidator> .
<http://datashapes.org/dash#hasPattern> <http://www.w3.org/1999/02/22-rdf-syntax-ns#type> <http://www.w3.org/ns/shacl#SPARQLAskValidator> .
<http://www.w3.org/ns/shacl#XoneConstraintComponent> <http://www.w3.org/ns/shacl#targetClass> <http://www.w3.org/ns/shacl#Shape> .
<http://datashapes.org/dash#hidden> <http://www.w3.org/1999/02/22-rdf-syntax-ns#type> <http://www.w3.org/1999/02/22-rdf-syntax-ns#Property> .
<http://datashapes.org/dash#TextFieldWithLangEditor> <http://www.w3.org/2000/01/rdf-schema#label> "Text field with lang editor" .
<http://datashapes.org/dash#UniqueValueForClassConstraintComponent> <http://www.w3.org/ns/shacl#propertyValidator> _:B0501804cef6c59c65c932d30353a449b .
<http://datashapes.org/dash#isLanguageIn> <http://www.w3.org/ns/shacl#prefixes> <http://datashapes.org/dash> .
<http://datashapes.org/dash#toString> <http://www.w3.org/ns/shacl#jsFunctionName> "dash_toString" .
_:B3198ee9db9f046c7a63785bb62bb0766 <http://www.w3.org/ns/shacl#message> "Missing expected value {$hasValue}" .
<http://datashapes.org/dash#ReifiableByConstraintComponent-reifiableBy> <http://www.w3.org/ns/shacl#nodeKind> <http://www.w3.org/ns/shacl#IRI> .
<http://www.w3.org/ns/shacl#AbstractResult> <http://datashapes.org/dash#abstract> "true"^^<http://www.w3.org/2001/XMLSchema#boolean> .
<http://www.w3.org/ns/shacl#MinExclusiveConstraintComponent> <http://datashapes.org/dash#staticConstraint> "true"^^<http://www.w3.org/2001/XMLSchema#boolean> .
<http://www.w3.org/ns/shacl#MinInclusiveConstraintComponent> <http://datashapes.org/dash#staticConstraint> "true"^^<http://www.w3.org/2001/XMLSchema#boolean> .
<http://datashapes.org/dash#valueCount> <http://www.w3.org/ns/shacl#parameter> _:B485dc9d077951c4a981419e27a12efce .
_:B88430adc5caf16f7f8cd82bc8fb6a6f8 <http://www.w3.org/1999/02/22-rdf-syntax-ns#type> <http://www.w3.org/ns/shacl#SPARQLAskValidator> .
<http://datashapes.org/dash#AllObjectsTarget> <http://www.w3.org/ns/shacl#jsLibrary> <http://datashapes.org/dash#DASHJSLibrary> .
<http://datashapes.org/dash#uniqueValueForClass> <http://www.w3.org/2000/01/rdf-schema#label> "unique value for class" .
<http://datashapes.org/dash#FailureTestCaseResult> <http://www.w3.org/1999/02/22-rdf-syntax-ns#type> <http://www.w3.org/2000/01/rdf-schema#Class> .
<http://datashapes.org/dash#hasMinExclusive> <http://www.w3.org/ns/shacl#ask> "ASK { FILTER ($value > $minExclusive) }" .
<http://www.w3.org/ns/shacl#InConstraintComponent> <http://www.w3.org/ns/shacl#message> "Value is not in {$in}" .
_:B7f1ad1df154d5b4790aefb896d1c9fb8 <http://www.w3.org/1999/02/22-rdf-syntax-ns#type> <http://www.w3.org/ns/shacl#PropertyShape> .
<http://datashapes.org/dash#GraphUpdate> <http://www.w3.org/1999/02/22-rdf-syntax-ns#type> <http://www.w3.org/2000/01/rdf-schema#Class> .
_:B3b32abda9658f358f57cc4b5edac88b8 <http://www.w3.org/ns/shacl#description> "The expected inferred triples, represented by instances of rdfs:Statement." .
<http://www.w3.org/ns/shacl#MaxExclusiveConstraintComponent> <http://www.w3.org/ns/shacl#labelTemplate> "Value must be < {$maxExclusive}" .
<http://datashapes.org/dash#CoExistsWithConstraintComponent> <http://www.w3.org/ns/shacl#message> "Values must co-exist with values of {$coExistsWith}" .
<http://www.w3.org/ns/shacl#MinInclusiveConstraintComponent> <http://www.w3.org/ns/shacl#message> "Value is not >= {$minInclusive}" .
<http://www.w3.org/ns/shacl#LessThanConstraintComponent> <http://www.w3.org/ns/shacl#propertyValidator> _:B576b207887a27c8640d054dd19740272 .
<http://www.w3.org/ns/shacl#MinCountConstraintComponent> <http://www.w3.org/ns/shacl#labelTemplate> "Must have at least {$minCount} values" .
<http://www.w3.org/ns/shacl#MaxExclusiveConstraintComponent> <http://www.w3.org/ns/shacl#validator> <http://datashapes.org/dash#hasMaxExclusive> .
_:B0c0f328c69e13d06674f58bb5b4a9284 <http://www.w3.org/ns/shacl#group> <http://topbraid.org/tosh#StringBasedConstraintPropertyGroup> .
<http://datashapes.org/dash#testEnvironment> <http://www.w3.org/2000/01/rdf-schema#comment> "Can be used by TestCases to point at a resource with information on how to set up the execution environment prior to execution." .
<http://www.w3.org/ns/shacl#InConstraintComponent> <http://www.w3.org/ns/shacl#targetClass> <http://www.w3.org/ns/shacl#Shape> .
<http://datashapes.org/dash#hasMaxLength> <http://www.w3.org/ns/shacl#prefixes> <http://datashapes.org/dash> .
_:B77912faa4452655d39dee0cf876cb183 <http://www.w3.org/ns/shacl#jsFunctionName> "validateHasValueNode" .
<http://datashapes.org/dash#SymmetricConstraintComponent> <http://www.w3.org/ns/shacl#targetClass> <http://www.w3.org/ns/shacl#PropertyShape> .
<http://datashapes.org/dash#hasNodeKind> <http://www.w3.org/1999/02/22-rdf-syntax-ns#type> <http://www.w3.org/ns/shacl#SPARQLAskValidator> .
_:B5672337cd6b085d4efa2003d67fc0562 <http://www.w3.org/ns/shacl#name> "predicate" .
<http://datashapes.org/dash#Editor> <http://www.w3.org/2000/01/rdf-schema#label> "Editor" .
<http://datashapes.org/dash#GraphValidationTestCase> <http://www.w3.org/2000/01/rdf-schema#subClassOf> <http://datashapes.org/dash#ValidationTestCase> .
_:Bdad9596a4e29da75e0aa7a561275dd9f <http://www.w3.org/ns/shacl#jsLibrary> <http://datashapes.org/dash#DASHJSLibrary> .
<http://datashapes.org/dash#LiteralViewer> <http://www.w3.org/2000/01/rdf-schema#label> "Literal Viewer" .
_:B707d4e7635546fda18ee3fda129e9373 <http://www.w3.org/ns/shacl#jsFunctionName> "validateHasValueWithClass" .
<http://datashapes.org/dash#ValueTableViewer> <http://www.w3.org/2000/01/rdf-schema#comment> "A viewer that renders all values of a given property as a table, with one value per row, and the columns defined by the shape that is the sh:node or sh:class of the property." .
_:B1db6386c181b226090f5a502966d369b <http://www.w3.org/1999/02/22-rdf-syntax-ns#type> <http://www.w3.org/ns/shacl#JSValidator> .
<http://datashapes.org/dash#Widget> <http://www.w3.org/2000/01/rdf-schema#subClassOf> <http://www.w3.org/2000/01/rdf-schema#Resource> .
_:B1131591453602389668eae575a1a4693 <http://www.w3.org/ns/shacl#description> "The SPARQL SELECT query to execute." .
_:Bfe0a112f2951265152c632d9a5c70c7a <http://www.w3.org/ns/shacl#prefixes> <http://datashapes.org/dash> .
<http://www.w3.org/ns/shacl#LessThanOrEqualsConstraintComponent> <http://www.w3.org/ns/shacl#targetClass> <http://www.w3.org/ns/shacl#PropertyShape> .
<http://www.w3.org/ns/shacl#DatatypeConstraintComponent> <http://www.w3.org/ns/shacl#labelTemplate> "Values must have datatype {$datatype}" .
<http://datashapes.org/dash#includedExecutionPlatform> <http://www.w3.org/2000/01/rdf-schema#comment> "Can be used to state that one (subject) execution platform includes all features of another platform (object)." .
_:Ba94bb54840f7b2f2def8b93e306cd9bf <http://www.w3.org/ns/shacl#datatype> <http://www.w3.org/2001/XMLSchema#boolean> .
<http://datashapes.org/dash#DetailsViewer> <http://www.w3.org/1999/02/22-rdf-syntax-ns#type> <http://datashapes.org/dash#Viewer> .
_:Bbc6a3e0006c01fd1021e9a87d62d127a <http://www.w3.org/1999/02/22-rdf-syntax-ns#type> <http://www.w3.org/ns/shacl#PropertyShape> .
<http://datashapes.org/dash#hasMinExclusive> <http://www.w3.org/ns/shacl#prefixes> <http://datashapes.org/dash> .
<http://datashapes.org/dash#isNodeKindBlankNode> <http://www.w3.org/ns/shacl#prefixes> <http://datashapes.org/dash> .
<http://datashapes.org/dash#expectedResultIsJSON> <http://www.w3.org/2000/01/rdf-schema#label> "expected result is JSON" .
<http://datashapes.org/dash#applicableToClass> <http://www.w3.org/2000/01/rdf-schema#label> "applicable to class" .
<http://www.w3.org/ns/shacl#QualifiedMaxCountConstraintComponent> <http://www.w3.org/ns/shacl#labelTemplate> "No more than {$qualifiedMaxCount} values can have shape {$qualifiedValueShape}" .
_:Bf2df11d10c098c62248867b2af223317 <http://www.w3.org/ns/shacl#namespace> "http://www.w3.org/2001/XMLSchema#"^^<http://www.w3.org/2001/XMLSchema#anyURI> .
<http://datashapes.org/dash#AllSubjectsTarget> <http://www.w3.org/2000/01/rdf-schema#label> "All subjects target" .
_:Be4b7da0362b43f04fa717e3e11887a9e <http://www.w3.org/ns/shacl#select> "SELECT $this\nWHERE {\n\tFILTER NOT EXISTS {\n    \t$this $PATH ?value .\n\t\t?value a ?type .\n\t\t?type rdfs:subClassOf* ?hasValueWithClass .\n\t}\n}" .
_:B485dc9d077951c4a981419e27a12efce <http://www.w3.org/ns/shacl#class> <http://www.w3.org/2000/01/rdf-schema#Resource> .
_:B646fdae9066263aad8548980a9a6346d <http://www.w3.org/ns/shacl#jsLibrary> <http://datashapes.org/dash#DASHJSLibrary> .
<http://datashapes.org/dash#all> <http://www.w3.org/2000/01/rdf-schema#comment> "Represents all users/roles, for example as a possible value of the default view for role property." .
_:Bf0ecfeb376963097d84d425af13c3875 <http://www.w3.org/ns/shacl#namespace> "http://purl.org/dc/terms/"^^<http://www.w3.org/2001/XMLSchema#anyURI> .
<http://datashapes.org/dash#DASHJSLibrary> <http://www.w3.org/ns/shacl#jsLibrary> <http://datashapes.org/dash#RDFQueryJSLibrary> .
_:B474b201cX2D1114X2D493aX2Da90bX2D68fa0363bb24 <http://www.w3.org/1999/02/22-rdf-syntax-ns#first> _:B4d5234299127eb5252bb141a36ca256e .
<http://datashapes.org/dash#TestCaseResult> <http://www.w3.org/1999/02/22-rdf-syntax-ns#type> <http://www.w3.org/2000/01/rdf-schema#Class> .
<http://datashapes.org/dash#StringOrLangString> <http://www.w3.org/1999/02/22-rdf-syntax-ns#first> _:Bb2e5e8d47a4f14ae7e8ce2aaa0029c3f .
<http://datashapes.org/dash#PrimaryKeyConstraintComponent> <http://datashapes.org/dash#localConstraint> "true"^^<http://www.w3.org/2001/XMLSchema#boolean> .
<http://datashapes.org/dash#isNodeKindLiteral> <http://www.w3.org/ns/shacl#parameter> _:Bef4b4e661cf3b607381181797fae49a3 .
<http://datashapes.org/dash#SymmetricConstraintComponent> <http://www.w3.org/ns/shacl#parameter> <http://datashapes.org/dash#SymmetricConstraintComponent-symmetric> .
<http://datashapes.org/dash#NonRecursiveConstraintComponent-nonRecursive> <http://www.w3.org/1999/02/22-rdf-syntax-ns#type> <http://www.w3.org/ns/shacl#Parameter> .
<http://www.w3.org/ns/shacl#LessThanConstraintComponent> <http://datashapes.org/dash#localConstraint> "true"^^<http://www.w3.org/2001/XMLSchema#boolean> .
<http://www.w3.org/ns/shacl#OrConstraintComponent> <http://www.w3.org/ns/shacl#targetClass> <http://www.w3.org/ns/shacl#Shape> .
<http://datashapes.org/dash#isNodeKindBlankNode> <http://www.w3.org/2000/01/rdf-schema#label> "is NodeKind BlankNode" .
_:B2cb630d3ce6cc80fcb0af823135f42af <http://www.w3.org/ns/shacl#name> "expression" .
_:B0c0f328c69e13d06674f58bb5b4a9284 <http://www.w3.org/ns/shacl#datatype> <http://www.w3.org/2001/XMLSchema#boolean> .
<http://datashapes.org/dash#isNodeKindLiteral> <http://www.w3.org/1999/02/22-rdf-syntax-ns#type> <http://www.w3.org/ns/shacl#SPARQLFunction> .
_:B324a4eda45fae1908023e86a8b10dbdb <http://www.w3.org/1999/02/22-rdf-syntax-ns#type> <http://www.w3.org/ns/shacl#JSValidator> .
<http://datashapes.org/dash#ParameterConstraintComponent> <http://www.w3.org/2000/01/rdf-schema#label> "Parameter constraint component"@en .
<http://www.w3.org/ns/shacl#Target> <http://datashapes.org/dash#abstract> "true"^^<http://www.w3.org/2001/XMLSchema#boolean> .
<http://www.w3.org/ns/shacl#sparql> <http://datashapes.org/dash#defaultValueType> <http://www.w3.org/ns/shacl#SPARQLConstraint> .
_:Ba6e7b59cb1609800d73a83169cfb1050 <http://www.w3.org/ns/shacl#prefix> "dash" .
<http://datashapes.org/dash#cachable> <http://www.w3.org/2000/01/rdf-schema#domain> <http://www.w3.org/ns/shacl#Function> .
<http://www.w3.org/ns/shacl#not> <http://datashapes.org/dash#defaultValueType> <http://www.w3.org/ns/shacl#Shape> .
<http://www.w3.org/ns/shacl#LanguageInConstraintComponent> <http://www.w3.org/ns/shacl#targetClass> <http://www.w3.org/ns/shacl#Shape> .
<http://datashapes.org/dash#applicableToClass> <http://www.w3.org/1999/02/22-rdf-syntax-ns#type> <http://www.w3.org/1999/02/22-rdf-syntax-ns#Property> .
<http://datashapes.org/dash#HasValueWithClassConstraintComponent> <http://www.w3.org/ns/shacl#targetClass> <http://www.w3.org/ns/shacl#PropertyShape> .
_:B6a3dda78c1d1372a3ae27e96a10584b5 <http://www.w3.org/ns/shacl#prefix> "owl" .
<http://datashapes.org/dash#SubSetOfConstraintComponent> <http://www.w3.org/ns/shacl#targetClass> <http://www.w3.org/ns/shacl#PropertyShape> .
_:B12898dca29ca363f5ae4b1b4c90c363b <http://www.w3.org/ns/shacl#class> <http://datashapes.org/dash#TestCase> .
_:Bff9ecbe5a61b70becac46f6b4ddfdb03 <http://www.w3.org/ns/shacl#minCount> "1"^^<http://www.w3.org/2001/XMLSchema#integer> .
<http://datashapes.org/dash#SingleLineConstraintComponent> <http://www.w3.org/ns/shacl#validator> _:B88430adc5caf16f7f8cd82bc8fb6a6f8 .
<http://datashapes.org/dash#FailureTestCaseResult> <http://www.w3.org/2000/01/rdf-schema#comment> "Represents a failure of a test case." .
_:B7f1ad1df154d5b4790aefb896d1c9fb8 <http://www.w3.org/ns/shacl#path> <http://datashapes.org/dash#cachable> .
<http://www.w3.org/ns/shacl#MinExclusiveConstraintComponent> <http://www.w3.org/ns/shacl#labelTemplate> "Value must be > {$minExclusive}" .
_:B9f8708a030e28285db3efcfa7150f80b <http://www.w3.org/1999/02/22-rdf-syntax-ns#type> <http://www.w3.org/ns/shacl#JSValidator> .
<http://datashapes.org/dash#includedExecutionPlatform> <http://www.w3.org/2000/01/rdf-schema#range> <http://datashapes.org/dash#ExecutionPlatform> .
_:B31473064d8bd1e288bd70b63b0f116a3 <http://www.w3.org/ns/shacl#nodeKind> <http://www.w3.org/ns/shacl#IRI> .
<http://www.w3.org/ns/shacl#EqualsConstraintComponent> <http://www.w3.org/ns/shacl#message> "Must have same values as {$equals}" .
<http://datashapes.org/dash#HyperlinkViewer> <http://www.w3.org/1999/02/22-rdf-syntax-ns#type> <http://datashapes.org/dash#Viewer> .
_:B61f5442de5a071e03f0bc4b21b3752cc <http://www.w3.org/1999/02/22-rdf-syntax-ns#type> <http://www.w3.org/ns/shacl#SPARQLSelectValidator> .
_:Bd7d823a9ff3f41bf4f9c8b66d70cce69 <http://www.w3.org/1999/02/22-rdf-syntax-ns#type> <http://www.w3.org/ns/shacl#JSValidator> .
<http://datashapes.org/dash#hasValueWithClass> <http://www.w3.org/1999/02/22-rdf-syntax-ns#type> <http://www.w3.org/1999/02/22-rdf-syntax-ns#Property> .
_:B0cd35e055bd003648f8b9739d1d3297a <http://www.w3.org/ns/shacl#select> "\n\t\tSELECT $this\n\t\tWHERE {\n\t\t\t$this $PATH ?value .\n\t\t}\n\t\tGROUP BY $this\n\t\tHAVING (COUNT(DISTINCT ?value) > $maxCount)\n\t\t" .
<http://datashapes.org/dash#symmetric> <http://www.w3.org/2000/01/rdf-schema#label> "symmetric" .
_:Bb880e354f894466d96da68ac6732829f <http://www.w3.org/ns/shacl#jsFunctionName> "validateEqualsProperty" .
<http://datashapes.org/dash#ReifiableByConstraintComponent-reifiableBy> <http://www.w3.org/ns/shacl#class> <http://www.w3.org/ns/shacl#NodeShape> .
<http://datashapes.org/dash#expectedResult> <http://www.w3.org/2000/01/rdf-schema#comment> "The expected result(s) of a test case. The value range of this property is different for each kind of test cases." .
<http://datashapes.org/dash#hasMaxInclusive> <http://www.w3.org/ns/shacl#ask> "ASK { FILTER ($value <= $maxInclusive) }" .
<http://datashapes.org/dash#SPARQLSelectTemplate> <http://www.w3.org/1999/02/22-rdf-syntax-ns#type> <http://www.w3.org/2000/01/rdf-schema#Class> .
<http://datashapes.org/dash#subSetOf> <http://www.w3.org/2000/01/rdf-schema#label> "sub set of" .
<http://www.w3.org/ns/shacl#UniqueLangConstraintComponent> <http://www.w3.org/ns/shacl#message> "Language \"{?lang}\" used more than once" .
_:B3b39cb9aee43fa574acdbcdac62b381f <http://www.w3.org/1999/02/22-rdf-syntax-ns#type> <http://www.w3.org/ns/shacl#JSValidator> .
_:B6431ca200460b7f86c096adcb4867b07 <http://www.w3.org/1999/02/22-rdf-syntax-ns#type> <http://www.w3.org/ns/shacl#PropertyShape> .
<http://datashapes.org/dash#AllSubjectsTarget> <http://www.w3.org/2000/01/rdf-schema#subClassOf> <http://www.w3.org/ns/shacl#Target> .
<http://datashapes.org/dash#CoExistsWithConstraintComponent> <http://www.w3.org/1999/02/22-rdf-syntax-ns#type> <http://www.w3.org/ns/shacl#ConstraintComponent> .
<http://datashapes.org/dash#AllObjectsTarget> <http://www.w3.org/ns/shacl#select> "SELECT DISTINCT ?this\nWHERE {\n    ?anyS ?anyP ?this .\n}" .
<http://datashapes.org/dash#hasMinInclusive> <http://www.w3.org/ns/shacl#prefixes> <http://datashapes.org/dash> .
_:B0501804cef6c59c65c932d30353a449b <http://www.w3.org/ns/shacl#select> "SELECT DISTINCT $this ?value ?other\nWHERE {\n\t{\n    \t$this $PATH ?value .\n\t\t?other $PATH ?value .\n\t\tFILTER (?other != $this) .\n\t}\n\t?other a ?type .\n\t?type rdfs:subClassOf* $uniqueValueForClass .\n}" .
<http://datashapes.org/dash#ValidationTestCase> <http://www.w3.org/1999/02/22-rdf-syntax-ns#type> <http://www.w3.org/2000/01/rdf-schema#Class> .
<http://datashapes.org/dash#SingleLineConstraintComponent> <http://www.w3.org/1999/02/22-rdf-syntax-ns#type> <http://www.w3.org/ns/shacl#ConstraintComponent> .
<http://datashapes.org/dash#suggestionGroup> <http://www.w3.org/2000/01/rdf-schema#comment> "Can be used to link a suggestion with the group identifier to which it belongs. By default this is a link to the dash:SuggestionGenerator, but in principle this could be any value." .
<http://www.w3.org/ns/shacl#Function> <http://www.w3.org/ns/shacl#property> _:B7f1ad1df154d5b4790aefb896d1c9fb8 .
<http://datashapes.org/dash#Editor> <http://www.w3.org/1999/02/22-rdf-syntax-ns#type> <http://www.w3.org/2000/01/rdf-schema#Class> .
<http://www.w3.org/ns/shacl#NotConstraintComponent> <http://www.w3.org/ns/shacl#message> "Value does have shape {$not}" .
_:B12898dca29ca363f5ae4b1b4c90c363b <http://www.w3.org/ns/shacl#path> <http://datashapes.org/dash#testCase> .
<http://datashapes.org/dash#SuggestionGenerator> <http://www.w3.org/2000/01/rdf-schema#comment> "Base class of objects that can generate suggestions (added or deleted triples) for a validation result of a given constraint component." .
<http://datashapes.org/dash#TestCase> <http://www.w3.org/2000/01/rdf-schema#subClassOf> <http://www.w3.org/2000/01/rdf-schema#Resource> .
_:B1131591453602389668eae575a1a4693 <http://www.w3.org/ns/shacl#maxCount> "1"^^<http://www.w3.org/2001/XMLSchema#integer> .
<http://datashapes.org/dash#JSTestCase> <http://www.w3.org/ns/shacl#property> _:Bd5a64ddffc0079f527ee5678e81011df .
<http://datashapes.org/dash#SPARQLConstructTemplate> <http://www.w3.org/2000/01/rdf-schema#subClassOf> <http://www.w3.org/ns/shacl#SPARQLConstructExecutable> .
<http://datashapes.org/dash#hasPattern> <http://www.w3.org/2000/01/rdf-schema#label> "has pattern" .
<http://datashapes.org/dash#editor> <http://www.w3.org/1999/02/22-rdf-syntax-ns#type> <http://www.w3.org/1999/02/22-rdf-syntax-ns#Property> .
<http://datashapes.org/dash#RootClassConstraintComponent-rootClass> <http://www.w3.org/ns/shacl#description> "The root class." .
<http://datashapes.org/dash#composite> <http://www.w3.org/2000/01/rdf-schema#label> "composite" .
<http://www.w3.org/ns/shacl#MinInclusiveConstraintComponent> <http://www.w3.org/ns/shacl#validator> <http://datashapes.org/dash#hasMinInclusive> .
_:Bbd150169a34ef6489542c2938b3e8f67 <http://www.w3.org/ns/shacl#hasValue> <http://www.w3.org/1999/02/22-rdf-syntax-ns#nil> .
<http://datashapes.org/dash#testModifiesEnvironment> <http://www.w3.org/2000/01/rdf-schema#label> "test modifies environment" .
_:Bf0deb4dbfedca171cbc3d5e34c7d597d <http://www.w3.org/ns/shacl#path> <http://www.w3.org/1999/02/22-rdf-syntax-ns#rest> .
<http://datashapes.org/dash#UniqueValueForClassConstraintComponent-uniqueValueForClass> <http://www.w3.org/ns/shacl#path> <http://datashapes.org/dash#uniqueValueForClass> .
<http://datashapes.org/dash#detailsEndpoint> <http://www.w3.org/1999/02/22-rdf-syntax-ns#type> <http://www.w3.org/1999/02/22-rdf-syntax-ns#Property> .
<http://datashapes.org/dash#defaultViewForRole> <http://www.w3.org/2000/01/rdf-schema#domain> <http://www.w3.org/ns/shacl#NodeShape> .
_:Bef4b4e661cf3b607381181797fae49a3 <http://www.w3.org/ns/shacl#nodeKind> <http://www.w3.org/ns/shacl#IRI> .
<http://www.w3.org/ns/shacl#qualifiedValueShape> <http://datashapes.org/dash#defaultValueType> <http://www.w3.org/ns/shacl#Shape> .
<http://datashapes.org/dash#coExistsWith> <http://www.w3.org/2000/01/rdf-schema#comment> "Specifies a property that must have a value whenever the property path has a value, and must have no value whenever the property path has no value." .
<http://datashapes.org/dash#isNodeKindLiteral> <http://www.w3.org/2000/01/rdf-schema#comment> "Checks if a given sh:NodeKind is one that includes Literals." .
_:B77912faa4452655d39dee0cf876cb183 <http://www.w3.org/ns/shacl#message> "Value must be {$hasValue}" .
<http://datashapes.org/dash#AllSubjectsTarget> <http://www.w3.org/ns/shacl#prefixes> <http://datashapes.org/dash> .
<http://datashapes.org/dash#hidden> <http://www.w3.org/2000/01/rdf-schema#comment> "Properties marked as readOnly do not appear in user interfaces, yet remain part of the shape for other purposes such as validation and GraphQL schemas." .
<http://datashapes.org/dash#ParameterConstraintComponent> <http://www.w3.org/1999/02/22-rdf-syntax-ns#type> <http://www.w3.org/ns/shacl#ConstraintComponent> .
_:B3198ee9db9f046c7a63785bb62bb0766 <http://www.w3.org/1999/02/22-rdf-syntax-ns#type> <http://www.w3.org/ns/shacl#JSValidator> .
_:B2cb630d3ce6cc80fcb0af823135f42af <http://www.w3.org/1999/02/22-rdf-syntax-ns#type> <http://www.w3.org/ns/shacl#PropertyShape> .
<http://datashapes.org/dash#AllObjectsTarget> <http://www.w3.org/ns/shacl#jsFunctionName> "dash_allObjects" .
_:B8137cd87d692f6f1ad4d374873d42a49 <http://www.w3.org/ns/shacl#jsLibrary> <http://datashapes.org/dash#DASHJSLibrary> .
_:B42c37f93cbd4d4c68e68cfec1631af95 <http://www.w3.org/ns/shacl#message> "Value node must not also be one of the values of {$disjoint}" .
<http://datashapes.org/dash#AutoCompleteEditor> <http://www.w3.org/1999/02/22-rdf-syntax-ns#type> <http://datashapes.org/dash#Editor> .
<http://www.w3.org/ns/shacl#AndConstraintComponent> <http://www.w3.org/ns/shacl#targetClass> <http://www.w3.org/ns/shacl#Shape> .
_:B54c36a3353a36f7de1eb49377ffde112 <http://www.w3.org/ns/shacl#prefix> "rdfs" .
<http://datashapes.org/dash#SubSetOfConstraintComponent-subSetOf> <http://www.w3.org/ns/shacl#class> <http://www.w3.org/1999/02/22-rdf-syntax-ns#Property> .
<http://datashapes.org/dash#expectedResultIsJSON> <http://www.w3.org/1999/02/22-rdf-syntax-ns#type> <http://www.w3.org/1999/02/22-rdf-syntax-ns#Property> .
_:B567e621e200ca5c599b5f14c17b0e7b3 <http://www.w3.org/ns/shacl#jsLibrary> <http://datashapes.org/dash#DASHJSLibrary> .
<http://datashapes.org/dash#HTMLOrStringOrLangString> <http://www.w3.org/2000/01/rdf-schema#label> "HTML or string or langString" .
<http://datashapes.org/dash#x> <http://www.w3.org/2000/01/rdf-schema#comment> "The x position." .
_:B1131591453602389668eae575a1a4693 <http://www.w3.org/ns/shacl#name> "SPARQL query" .
_:B9fe7602a489f48a08b22e99931d59d35 <http://www.w3.org/ns/shacl#datatype> <http://www.w3.org/2001/XMLSchema#string> .
_:Bbc6a3e0006c01fd1021e9a87d62d127a <http://www.w3.org/ns/shacl#name> "uri" .
<http://www.w3.org/ns/shacl#LanguageInConstraintComponent> <http://www.w3.org/ns/shacl#validator> _:B1db6386c181b226090f5a502966d369b .
<http://datashapes.org/dash#isDeactivated> <http://www.w3.org/ns/shacl#ask> "ASK {\n    ?constraintOrShape sh:deactivated true .\n}" .
<http://datashapes.org/dash#propertySuggestionGenerator> <http://www.w3.org/2000/01/rdf-schema#comment> "Links the constraint component with instances of dash:SuggestionGenerator that may be used to produce suggestions for a given validation result that was produced by a property constraint." .
<http://datashapes.org/dash#toString> <http://www.w3.org/2000/01/rdf-schema#comment> "Returns a literal with datatype xsd:string that has the input value as its string. If the input value is an (URI) resource then its URI will be used." .
<http://datashapes.org/dash#isDeactivated> <http://www.w3.org/2000/01/rdf-schema#label> "is deactivated" .
_:B8791b3a24b8675de3fe6cea3980f416f <http://www.w3.org/ns/shacl#message> "Property must not share any values with {$disjoint}" .
_:B881d49f14342613394c38418a3e2b26e <http://www.w3.org/ns/shacl#select> "\n\t\tSELECT $this\n\t\tWHERE {\n\t\t\tOPTIONAL {\n\t\t\t\t$this $PATH ?value .\n\t\t\t}\n\t\t}\n\t\tGROUP BY $this\n\t\tHAVING (COUNT(DISTINCT ?value) < $minCount)\n\t\t" .
_:B21421ade4ccc7092969f52bbcc0d7484 <http://www.w3.org/ns/shacl#jsFunctionName> "validateMinInclusive" .
_:B3198ee9db9f046c7a63785bb62bb0766 <http://www.w3.org/ns/shacl#jsLibrary> <http://datashapes.org/dash#DASHJSLibrary> .
_:B8137cd87d692f6f1ad4d374873d42a49 <http://www.w3.org/1999/02/22-rdf-syntax-ns#type> <http://www.w3.org/ns/shacl#JSValidator> .
<http://datashapes.org/dash#height> <http://www.w3.org/2000/01/rdf-schema#comment> "The height." .
<http://www.w3.org/ns/shacl#ClassConstraintComponent> <http://www.w3.org/ns/shacl#validator> <http://datashapes.org/dash#hasClass> .
<http://datashapes.org/dash#RootClassConstraintComponent> <http://www.w3.org/2000/01/rdf-schema#comment> "A constraint component defining the parameter dash:rootClass, which restricts the values to be either the root class itself or one of its subclasses. This is typically used in conjunction with properties that have rdfs:Class as their type." .
<http://datashapes.org/dash#ReifiableByConstraintComponent-reifiableBy> <http://www.w3.org/ns/shacl#description> "Can be used to specify the node shape that may be applied to reified statements produced by a property shape. The property shape must have a URI resource as its sh:path. The values of this property must be node shapes. User interfaces can use this information to determine which properties to present to users when reified statements are explored or edited. Also, SHACL validators can use it to determine how to validate reified triples. Use dash:None to indicate that no reification should be permitted." .
_:B567e621e200ca5c599b5f14c17b0e7b3 <http://www.w3.org/1999/02/22-rdf-syntax-ns#type> <http://www.w3.org/ns/shacl#JSValidator> .
_:B307f48b773a26646f04807f63f4f7218 <http://www.w3.org/ns/shacl#datatype> <http://www.w3.org/1999/02/22-rdf-syntax-ns#langString> .
<http://datashapes.org/dash#RichTextEditor> <http://www.w3.org/1999/02/22-rdf-syntax-ns#type> <http://datashapes.org/dash#Editor> .
<http://datashapes.org/dash#abstract> <http://www.w3.org/2000/01/rdf-schema#comment> "Indicates that a class is \"abstract\" and cannot be used in asserted rdf:type triples. Only non-abstract subclasses of abstract classes should be instantiated directly." .
<http://www.w3.org/ns/shacl#LanguageInConstraintComponent> <http://www.w3.org/ns/shacl#message> "Language does not match any of {$languageIn}" .
<http://datashapes.org/dash#RootClassConstraintComponent> <http://www.w3.org/ns/shacl#validator> _:B646fdae9066263aad8548980a9a6346d .
_:Bb2e5e8d47a4f14ae7e8ce2aaa0029c3f <http://www.w3.org/ns/shacl#datatype> <http://www.w3.org/2001/XMLSchema#string> .
_:B23e1001b72de7da857c5cf60a846810f <http://www.w3.org/ns/shacl#jsFunctionName> "validateNot" .
<http://datashapes.org/dash#viewer> <http://www.w3.org/1999/02/22-rdf-syntax-ns#type> <http://www.w3.org/1999/02/22-rdf-syntax-ns#Property> .
<http://datashapes.org/dash#y> <http://www.w3.org/1999/02/22-rdf-syntax-ns#type> <http://www.w3.org/1999/02/22-rdf-syntax-ns#Property> .
<http://www.w3.org/ns/shacl#MinExclusiveConstraintComponent> <http://www.w3.org/ns/shacl#validator> _:Bd79d8623d532452c0b9fb0617219aa16 .
<http://datashapes.org/dash#Widget> <http://datashapes.org/dash#abstract> "true"^^<http://www.w3.org/2001/XMLSchema#boolean> .
_:B6d4cbc3d992ff864f2dac864d1480fb8 <http://www.w3.org/ns/shacl#maxCount> "1"^^<http://www.w3.org/2001/XMLSchema#integer> .
<http://www.w3.org/ns/shacl#InConstraintComponent> <http://www.w3.org/ns/shacl#labelTemplate> "Value must be in {$in}" .
<http://datashapes.org/dash#x> <http://www.w3.org/1999/02/22-rdf-syntax-ns#type> <http://www.w3.org/1999/02/22-rdf-syntax-ns#Property> .
<http://datashapes.org/dash#deletedTriple> <http://www.w3.org/2000/01/rdf-schema#label> "deleted triple" .
<http://datashapes.org/dash#NonRecursiveConstraintComponent> <http://www.w3.org/ns/shacl#propertyValidator> _:B8911ff43e060d96ba77f70561fffd26e .
<http://datashapes.org/dash#SuccessResult> <http://www.w3.org/2000/01/rdf-schema#subClassOf> <http://www.w3.org/ns/shacl#AbstractResult> .
<http://datashapes.org/dash#isNodeKindIRI> <http://www.w3.org/ns/shacl#prefixes> <http://datashapes.org/dash> .
_:B12898dca29ca363f5ae4b1b4c90c363b <http://www.w3.org/ns/shacl#description> "The dash:TestCase that was executed." .
<http://datashapes.org/dash#UniqueValueForClassConstraintComponent> <http://www.w3.org/1999/02/22-rdf-syntax-ns#type> <http://www.w3.org/ns/shacl#ConstraintComponent> .
<http://datashapes.org/dash#hasRootClass> <http://www.w3.org/ns/shacl#prefixes> <http://datashapes.org/dash> .
<http://datashapes.org/dash#isDeactivated> <http://www.w3.org/ns/shacl#parameter> _:B96cb50ba954aab266bfb44f5557bd78e .
_:B0cd35e055bd003648f8b9739d1d3297a <http://www.w3.org/1999/02/22-rdf-syntax-ns#type> <http://www.w3.org/ns/shacl#SPARQLSelectValidator> .
<http://datashapes.org/dash#hasMinInclusive> <http://www.w3.org/2000/01/rdf-schema#comment> "Checks whether a given node (?value) has value greater than or equal to (>=) the provided ?minInclusive. Returns false if this cannot be determined, e.g. because values do not have comparable types." .
_:Bcb38cdae1cd4f5c0b1a9201bb0062cdf <http://www.w3.org/ns/shacl#maxCount> "1"^^<http://www.w3.org/2001/XMLSchema#integer> .
_:B9fe7602a489f48a08b22e99931d59d35 <http://www.w3.org/ns/shacl#minCount> "1"^^<http://www.w3.org/2001/XMLSchema#integer> .
<http://datashapes.org/dash#HTMLViewer> <http://www.w3.org/1999/02/22-rdf-syntax-ns#type> <http://datashapes.org/dash#Viewer> .
<http://datashapes.org/dash#SuggestionResult> <http://www.w3.org/2000/01/rdf-schema#subClassOf> <http://www.w3.org/ns/shacl#AbstractResult> .
<http://datashapes.org/dash#CoExistsWithConstraintComponent> <http://www.w3.org/ns/shacl#propertyValidator> _:B9c8553d682def0269e89fe21a9181cad .
_:B192ffa056ee292f9513e19adb943a589 <http://www.w3.org/ns/shacl#jsFunctionName> "validateSymmetric" .
<http://www.w3.org/ns/shacl#InConstraintComponent> <http://datashapes.org/dash#localConstraint> "true"^^<http://www.w3.org/2001/XMLSchema#boolean> .
<http://www.w3.org/ns/shacl#property> <http://datashapes.org/dash#defaultValueType> <http://www.w3.org/ns/shacl#PropertyShape> .
_:B28e99018c21492355cbeb7ce9c303876 <http://www.w3.org/ns/shacl#jsFunctionName> "validateMaxInclusive" .
_:B3b39cb9aee43fa574acdbcdac62b381f <http://www.w3.org/ns/shacl#jsLibrary> <http://datashapes.org/dash#DASHJSLibrary> .
_:Bbc6a3e0006c01fd1021e9a87d62d127a <http://www.w3.org/ns/shacl#description> "The URI of the graph to load." .
<http://datashapes.org/dash#NonRecursiveConstraintComponent-nonRecursive> <http://www.w3.org/ns/shacl#maxCount> "1"^^<http://www.w3.org/2001/XMLSchema#integer> .
_:Baf7234052e57bdd00025c4c0de812c1d <http://www.w3.org/ns/shacl#prefixes> <http://datashapes.org/dash> .
_:B88430adc5caf16f7f8cd82bc8fb6a6f8 <http://www.w3.org/ns/shacl#ask> "ASK {\n    FILTER (!$singleLine || !isLiteral($value) || (!contains(str($value), '\\n') && !contains(str($value), '\\r')))\n}" .
<http://datashapes.org/dash#closedByTypes> <http://www.w3.org/2000/01/rdf-schema#label> "closed by types" .
<http://www.w3.org/ns/shacl#MinLengthConstraintComponent> <http://www.w3.org/ns/shacl#message> "Value has less than {$minLength} characters" .
<http://datashapes.org/dash#expectedResultIsTTL> <http://www.w3.org/2000/01/rdf-schema#domain> <http://datashapes.org/dash#TestCase> .
<http://datashapes.org/dash#validateShapes> <http://www.w3.org/2000/01/rdf-schema#label> "validate shapes" .
<http://datashapes.org/dash#NonRecursiveConstraintComponent> <http://www.w3.org/1999/02/22-rdf-syntax-ns#type> <http://www.w3.org/ns/shacl#ConstraintComponent> .
<http://datashapes.org/dash#PrimaryKeyConstraintComponent> <http://www.w3.org/ns/shacl#parameter> <http://datashapes.org/dash#PrimaryKeyConstraintComponent-uriStart> .
<http://datashapes.org/dash#StemConstraintComponent> <http://www.w3.org/ns/shacl#parameter> <http://datashapes.org/dash#StemConstraintComponent-stem> .
<http://datashapes.org/dash#ExecutionPlatform> <http://www.w3.org/1999/02/22-rdf-syntax-ns#type> <http://www.w3.org/2000/01/rdf-schema#Class> .
_:Bd5a64ddffc0079f527ee5678e81011df <http://www.w3.org/1999/02/22-rdf-syntax-ns#type> <http://www.w3.org/ns/shacl#PropertyShape> .
<http://datashapes.org/dash#AutoCompleteEditor> <http://www.w3.org/2000/01/rdf-schema#label> "Auto-complete editor" .
_:B4f9dd044b748456b76262d5363cb5a94 <http://www.w3.org/1999/02/22-rdf-syntax-ns#type> <http://www.w3.org/ns/shacl#SPARQLSelectValidator> .
_:Bd7d823a9ff3f41bf4f9c8b66d70cce69 <http://www.w3.org/ns/shacl#jsLibrary> <http://datashapes.org/dash#DASHJSLibrary> .
_:B6df3b0d09d638883ddc7eaf55d1a9646 <http://www.w3.org/1999/02/22-rdf-syntax-ns#type> <http://www.w3.org/ns/shacl#PropertyShape> .
<http://www.w3.org/ns/shacl#ClassConstraintComponent> <http://www.w3.org/ns/shacl#targetClass> <http://www.w3.org/ns/shacl#Shape> .
<http://www.w3.org/ns/shacl#LanguageInConstraintComponent> <http://datashapes.org/dash#localConstraint> "true"^^<http://www.w3.org/2001/XMLSchema#boolean> .
_:B5ea6cb49b4f6b98c242342a8a98d3388 <http://www.w3.org/ns/shacl#property> _:Bf0deb4dbfedca171cbc3d5e34c7d597d .
_:B2bc3ad21d29b4bdb3981840c7e38c769 <http://www.w3.org/ns/shacl#hasValue> <http://www.w3.org/1999/02/22-rdf-syntax-ns#nil> .
<http://datashapes.org/dash#defaultValueType> <http://www.w3.org/2000/01/rdf-schema#label> "default value type" .
<http://www.w3.org/ns/shacl#MaxExclusiveConstraintComponent> <http://www.w3.org/ns/shacl#targetClass> <http://www.w3.org/ns/shacl#Shape> .
<http://datashapes.org/dash#reifiableBy> <http://www.w3.org/2000/01/rdf-schema#label> "reifiable by" .
<http://datashapes.org/dash#valueCount> <http://www.w3.org/2000/01/rdf-schema#comment> "Computes the number of objects for a given subject/predicate combination." .
_:B64037a34fda104980e7dda281bd2bc45 <http://www.w3.org/ns/shacl#maxCount> "1"^^<http://www.w3.org/2001/XMLSchema#integer> .
<http://datashapes.org/dash#toString> <http://www.w3.org/ns/shacl#prefixes> <http://datashapes.org/dash> .
<http://datashapes.org/dash#readOnly> <http://www.w3.org/1999/02/22-rdf-syntax-ns#type> <http://www.w3.org/1999/02/22-rdf-syntax-ns#Property> .
<http://datashapes.org/dash#LangStringViewer> <http://www.w3.org/1999/02/22-rdf-syntax-ns#type> <http://datashapes.org/dash#Viewer> .
_:Bd048027623bcc6288ff18f5d0dfbb126 <http://www.w3.org/ns/shacl#select> "\n\t\tSELECT DISTINCT $this ?value\n\t\tWHERE {\n\t\t\t{\n\t\t\t\tFILTER NOT EXISTS { $this $equals $this }\n\t\t\t\tBIND ($this AS ?value) .\n\t\t\t}\n\t\t\tUNION\n\t\t\t{\n\t\t\t\t$this $equals ?value .\n\t\t\t\tFILTER (?value != $this) .\n\t\t\t}\n\t\t}\n\t\t" .
<http://datashapes.org/dash#hasMaxExclusive> <http://www.w3.org/2000/01/rdf-schema#comment> "Checks whether a given node (?value) has a value less than (<) the provided ?maxExclusive. Returns false if this cannot be determined, e.g. because values do not have comparable types." .
_:B80b7e2f9fc1f404e1d9d214172e0e1b3 <http://www.w3.org/1999/02/22-rdf-syntax-ns#type> <http://www.w3.org/ns/shacl#SPARQLAskValidator> .
<http://datashapes.org/dash#symmetric> <http://www.w3.org/2000/01/rdf-schema#comment> "True to declare that the associated property path is symmetric." .
<http://www.w3.org/ns/shacl#ClassConstraintComponent> <http://www.w3.org/ns/shacl#validator> _:B2a3499b11e685d3ad17286d18e230c41 .
<http://www.w3.org/ns/shacl#MaxCountConstraintComponent> <http://www.w3.org/ns/shacl#propertyValidator> _:B0cd35e055bd003648f8b9739d1d3297a .
_:B817d3310X2D8c48X2D4ff6X2Da801X2D06febce45863 <http://www.w3.org/1999/02/22-rdf-syntax-ns#first> _:B307f48b773a26646f04807f63f4f7218 .
<http://datashapes.org/dash#valueCount> <http://www.w3.org/1999/02/22-rdf-syntax-ns#type> <http://www.w3.org/ns/shacl#SPARQLFunction> .
_:B44ba6ca913112e299d99b54732ce1509 <http://www.w3.org/ns/shacl#prefixes> <http://datashapes.org/dash> .
<http://www.w3.org/ns/shacl#PatternConstraintComponent> <http://www.w3.org/ns/shacl#targetClass> <http://www.w3.org/ns/shacl#Shape> .
<http://datashapes.org/dash#RootClassConstraintComponent> <http://www.w3.org/ns/shacl#targetClass> <http://www.w3.org/ns/shacl#PropertyShape> .
<http://datashapes.org/dash#CoExistsWithConstraintComponent> <http://www.w3.org/2000/01/rdf-schema#label> "Co-exists-with constraint component" .
_:B31473064d8bd1e288bd70b63b0f116a3 <http://www.w3.org/ns/shacl#class> <http://www.w3.org/ns/shacl#NodeKind> .
