<http://www.w3.org/ns/auth/rsa> <http://xmlns.com/foaf/0.1/maker> <http://bblfish.net/people/henry/card#me> .
<http://www.w3.org/ns/auth/rsa#RSAPublicKey> <http://www.w3.org/2000/01/rdf-schema#subClassOf> <http://www.w3.org/ns/auth/rsa#RSAKey> .
<http://www.w3.org/ns/auth/rsa#private_exponent> <http://www.w3.org/1999/02/22-rdf-syntax-ns#type> <http://www.w3.org/2002/07/owl#DatatypeProperty> .
<http://www.w3.org/ns/auth/rsa#RSAKey> <http://www.w3.org/2000/01/rdf-schema#comment> "\n    The union of the public and private components of an RSAKey.\n    Usually those pieces are not kept together\n    "@en .
<http://www.w3.org/ns/auth/rsa#RSAPublicKey> <http://www.w3.org/2000/01/rdf-schema#subClassOf> <http://www.w3.org/ns/auth/cert#PublicKey> .
<http://www.w3.org/ns/auth/rsa#modulus> <http://www.w3.org/2000/01/rdf-schema#domain> <http://www.w3.org/ns/auth/rsa#RSAKey> .
<http://www.w3.org/ns/auth/rsa#private_exponent> <http://www.w3.org/2000/01/rdf-schema#range> <http://www.w3.org/ns/auth/cert#int> .
<http://www.w3.org/ns/auth/rsa#private_exponent> <http://www.w3.org/2000/01/rdf-schema#domain> <http://www.w3.org/ns/auth/rsa#RSAPrivateKey> .
<http://www.w3.org/ns/auth/rsa> <http://www.w3.org/2000/01/rdf-schema#seeAlso> <http://en.wikipedia.org/wiki/RSA> .
<http://www.w3.org/ns/auth/rsa#RSAKey> <http://www.w3.org/1999/02/22-rdf-syntax-ns#type> <http://www.w3.org/2002/07/owl#Class> .
<http://www.w3.org/ns/auth/rsa#modulus> <http://www.w3.org/2000/01/rdf-schema#comment> "    \n   The modulus of an RSA public and private key. \n   This is defined as n = p*q\n   "@en .
<http://www.w3.org/ns/auth/rsa#public_exponent> <http://www.w3.org/2000/01/rdf-schema#comment> "\n       The exponent used to encrypt the message. Number chosen between\n       1 and the totient(p*q). Often named 'e' .\n    "@en .
_:B83a74783X2D2702X2D40eeX2Daba3X2Da677c414615d <http://xmlns.com/foaf/0.1/homepage> <http://ii.uwb.edu.pl/~dtomaszuk/card> .
<http://www.w3.org/ns/auth/rsa#public_exponent> <http://www.w3.org/2000/01/rdf-schema#range> <http://www.w3.org/ns/auth/cert#int> .
<http://www.w3.org/ns/auth/rsa#RSAPrivateKey> <http://www.w3.org/1999/02/22-rdf-syntax-ns#type> <http://www.w3.org/2002/07/owl#Class> .
<http://www.w3.org/ns/auth/rsa#RSAPublicKey> <http://www.w3.org/2000/01/rdf-schema#comment> "\n    The RSA public key.  Padded message m are encrypted by applying the function\n      modulus(power(m,exponent),modulus)\n    "@en .
<http://www.w3.org/ns/auth/rsa#RSAPrivateKey> <http://www.w3.org/2000/01/rdf-schema#seeAlso> <http://en.wikipedia.org/wiki/RSA> .
<http://www.w3.org/ns/auth/rsa#modulus> <http://www.w3.org/2003/06/sw-vocab-status/ns#term_status> "unstable" .
<http://www.w3.org/ns/auth/rsa#RSAKey> <http://www.w3.org/2000/01/rdf-schema#label> "RSA Key"@en .
<http://www.w3.org/ns/auth/rsa#public_exponent> <http://www.w3.org/1999/02/22-rdf-syntax-ns#type> <http://www.w3.org/2002/07/owl#DatatypeProperty> .
<http://www.w3.org/ns/auth/rsa#RSAPrivateKey> <http://www.w3.org/2000/01/rdf-schema#comment> "\n    A Private Key in the RSA framework \n    "@en .
<http://www.w3.org/ns/auth/rsa#RSAPrivateKey> <http://www.w3.org/2000/01/rdf-schema#label> "RSA Private Key"@en .
<http://www.w3.org/ns/auth/rsa#RSAPublicKey> <http://www.w3.org/2003/06/sw-vocab-status/ns#term_status> "unstable" .
<http://www.w3.org/ns/auth/rsa#RSAPublicKey> <http://www.w3.org/2000/01/rdf-schema#seeAlso> <http://en.wikipedia.org/wiki/RSA> .
<http://www.w3.org/ns/auth/rsa#RSAPublicKey> <http://www.w3.org/1999/02/22-rdf-syntax-ns#type> <http://www.w3.org/2002/07/owl#Class> .
<http://www.w3.org/ns/auth/rsa#RSAKey> <http://www.w3.org/2000/01/rdf-schema#subClassOf> <http://www.w3.org/ns/auth/cert#Key> .
<http://www.w3.org/ns/auth/rsa#RSAPrivateKey> <http://www.w3.org/2003/06/sw-vocab-status/ns#term_status> "unstable" .
<http://www.w3.org/ns/auth/rsa#modulus> <http://www.w3.org/2000/01/rdf-schema#label> "modulus"@en .
<http://www.w3.org/ns/auth/rsa> <http://purl.org/dc/terms/contributor> _:B83a74783X2D2702X2D40eeX2Daba3X2Da677c414615d .
<http://www.w3.org/ns/auth/rsa#private_exponent> <http://www.w3.org/2000/01/rdf-schema#label> "private"@en .
<http://www.w3.org/ns/auth/rsa> <http://purl.org/dc/terms/created> "2008-11-13"^^<http://www.w3.org/2001/XMLSchema#date> .
<http://www.w3.org/ns/auth/rsa> <http://www.w3.org/2003/06/sw-vocab-status/ns#term_status> "unstable" .
<http://www.w3.org/ns/auth/rsa#public_exponent> <http://www.w3.org/2000/01/rdf-schema#domain> <http://www.w3.org/ns/auth/rsa#RSAPublicKey> .
<http://www.w3.org/ns/auth/rsa> <http://www.w3.org/2000/01/rdf-schema#comment> "ontology for the RSA public private keys "@en .
<http://www.w3.org/ns/auth/rsa#RSAKey> <http://www.w3.org/2003/06/sw-vocab-status/ns#term_status> "unstable" .
<http://www.w3.org/ns/auth/rsa#private_exponent> <http://www.w3.org/2003/06/sw-vocab-status/ns#term_status> "unstable" .
<http://www.w3.org/ns/auth/rsa#modulus> <http://www.w3.org/1999/02/22-rdf-syntax-ns#type> <http://www.w3.org/2002/07/owl#DatatypeProperty> .
<http://www.w3.org/ns/auth/rsa#RSAPrivateKey> <http://www.w3.org/2000/01/rdf-schema#subClassOf> <http://www.w3.org/ns/auth/cert#PrivateKey> .
<http://www.w3.org/ns/auth/rsa#public_exponent> <http://www.w3.org/2000/01/rdf-schema#label> "public_exponent"@en .
<http://www.w3.org/ns/auth/rsa#public_exponent> <http://www.w3.org/2003/06/sw-vocab-status/ns#term_status> "unstable" .
<http://www.w3.org/ns/auth/rsa#modulus> <http://www.w3.org/2000/01/rdf-schema#range> <http://www.w3.org/ns/auth/cert#int> .
<http://www.w3.org/ns/auth/rsa#private_exponent> <http://www.w3.org/2000/01/rdf-schema#comment> "\n       The exponent used to decrypt the message\n       calculated as \n          public_exponent*private_exponent = 1 modulo totient(p*q)\n       The private exponent is often named 'd'\n    "@en .
<http://www.w3.org/ns/auth/rsa#RSAPublicKey> <http://www.w3.org/2000/01/rdf-schema#label> "RSA Public Key"@en .
<http://www.w3.org/ns/auth/rsa> <http://www.w3.org/2000/01/rdf-schema#seeAlso> <http://www.w3.org/ns/auth/X509Uml.svg> .
<http://www.w3.org/ns/auth/rsa> <http://www.w3.org/1999/02/22-rdf-syntax-ns#type> <http://www.w3.org/2002/07/owl#Ontology> .
<http://www.w3.org/ns/auth/rsa> <http://www.w3.org/2000/01/rdf-schema#seeAlso> <http://lists.foaf-project.org/mailman/listinfo/foaf-protocols> .
<http://www.w3.org/ns/auth/rsa#RSAPrivateKey> <http://www.w3.org/2000/01/rdf-schema#subClassOf> <http://www.w3.org/ns/auth/rsa#RSAKey> .
